<?xml version="1.0"?>
<rdf:RDF xmlns="http://w3id.org/dcri-ont/vocabulary/"
     xml:base="http://w3id.org/dcri-ont/vocabulary/"
     xmlns:owl="http://www.w3.org/2002/07/owl#"
     xmlns:rdf="http://www.w3.org/1999/02/22-rdf-syntax-ns#"
     xmlns:xml="http://www.w3.org/XML/1998/namespace"
     xmlns:xsd="http://www.w3.org/2001/XMLSchema#"
     xmlns:rdfs="http://www.w3.org/2000/01/rdf-schema#"
     xmlns:skos="http://www.w3.org/2004/02/skos/core#"
     xmlns:terms="http://purl.org/dc/terms/">
    <owl:Ontology rdf:about="http://w3id.org/dcri-ont/vocabulary/">
        <owl:imports rdf:resource="http://www.w3.org/2004/02/skos/core"/>
        <terms:creator xml:lang="en">Efthymia Moraitou</terms:creator>
        <terms:description xml:lang="en">DCRIO Vocabulary is a vocabulary of terms related to conservation and restoration interventions.</terms:description>
        <terms:title xml:lang="en">DCRIO Vocabulary</terms:title>
        <rdfs:comment xml:lang="en">DCRIO Vocabulary is a vocabulary of terms related to conservation and restoration interventions. It includes specialised terminology about intervnetion materials, techniques and equipment, as well as their characteristics.

The main objective of CRIO Vocabulary is the representation of specialised terminology which can be integrated to a formal ontology about conservation and restoration interventions, namely Decision of Conservation and Restoration Intervention Ontology.

A secondary objective of the vocabulary is the development of a vocabulary for the domain of conservation and restoration interventions exploiting Semantic Web technologies, which can be reused in other applications of conservation data management and organisation.</rdfs:comment>
        <rdfs:label xml:lang="en">DCRIO Vocabulary</rdfs:label>
        <owl:versionInfo>1.0</owl:versionInfo>
    </owl:Ontology>
    


    <!-- 
    ///////////////////////////////////////////////////////////////////////////////////////
    //
    // Annotation properties
    //
    ///////////////////////////////////////////////////////////////////////////////////////
     -->


    


    <!-- http://purl.org/dc/terms/creator -->


    <owl:AnnotationProperty rdf:about="http://purl.org/dc/terms/creator"/>
    


    <!-- http://purl.org/dc/terms/description -->


    <owl:AnnotationProperty rdf:about="http://purl.org/dc/terms/description"/>
    


    <!-- http://purl.org/dc/terms/title -->


    <owl:AnnotationProperty rdf:about="http://purl.org/dc/terms/title"/>
    


    <!-- http://www.w3.org/2004/02/skos/core#altLabel -->


    <owl:AnnotationProperty rdf:about="http://www.w3.org/2004/02/skos/core#altLabel">
        <rdfs:comment xml:lang="en">The range of skos:altLabel is the class of RDF plain literals.</rdfs:comment>
        <rdfs:comment xml:lang="en">skos:prefLabel, skos:altLabel and skos:hiddenLabel are pairwise disjoint properties.</rdfs:comment>
        <rdfs:isDefinedBy rdf:resource="http://www.w3.org/2004/02/skos/core"/>
        <rdfs:label xml:lang="en">alternative label</rdfs:label>
        <skos:definition xml:lang="en">An alternative lexical label for a resource.</skos:definition>
        <skos:example xml:lang="en">Acronyms, abbreviations, spelling variants, and irregular plural/singular forms may be included among the alternative labels for a concept. Mis-spelled terms are normally included as hidden labels (see skos:hiddenLabel).</skos:example>
        <rdfs:subPropertyOf rdf:resource="http://www.w3.org/2000/01/rdf-schema#label"/>
    </owl:AnnotationProperty>
    


    <!-- http://www.w3.org/2004/02/skos/core#changeNote -->


    <owl:AnnotationProperty rdf:about="http://www.w3.org/2004/02/skos/core#changeNote">
        <rdfs:isDefinedBy rdf:resource="http://www.w3.org/2004/02/skos/core"/>
        <rdfs:label xml:lang="en">change note</rdfs:label>
        <skos:definition xml:lang="en">A note about a modification to a concept.</skos:definition>
        <rdfs:subPropertyOf rdf:resource="http://www.w3.org/2004/02/skos/core#note"/>
    </owl:AnnotationProperty>
    


    <!-- http://www.w3.org/2004/02/skos/core#definition -->


    <owl:AnnotationProperty rdf:about="http://www.w3.org/2004/02/skos/core#definition">
        <rdfs:isDefinedBy rdf:resource="http://www.w3.org/2004/02/skos/core"/>
        <rdfs:label xml:lang="en">definition</rdfs:label>
        <skos:definition xml:lang="en">A statement or formal explanation of the meaning of a concept.</skos:definition>
        <rdfs:subPropertyOf rdf:resource="http://www.w3.org/2004/02/skos/core#note"/>
    </owl:AnnotationProperty>
    


    <!-- http://www.w3.org/2004/02/skos/core#editorialNote -->


    <owl:AnnotationProperty rdf:about="http://www.w3.org/2004/02/skos/core#editorialNote">
        <rdfs:isDefinedBy rdf:resource="http://www.w3.org/2004/02/skos/core"/>
        <rdfs:label xml:lang="en">editorial note</rdfs:label>
        <skos:definition xml:lang="en">A note for an editor, translator or maintainer of the vocabulary.</skos:definition>
        <rdfs:subPropertyOf rdf:resource="http://www.w3.org/2004/02/skos/core#note"/>
    </owl:AnnotationProperty>
    


    <!-- http://www.w3.org/2004/02/skos/core#example -->


    <owl:AnnotationProperty rdf:about="http://www.w3.org/2004/02/skos/core#example">
        <rdfs:isDefinedBy rdf:resource="http://www.w3.org/2004/02/skos/core"/>
        <rdfs:label xml:lang="en">example</rdfs:label>
        <skos:definition xml:lang="en">An example of the use of a concept.</skos:definition>
        <rdfs:subPropertyOf rdf:resource="http://www.w3.org/2004/02/skos/core#note"/>
    </owl:AnnotationProperty>
    


    <!-- http://www.w3.org/2004/02/skos/core#hiddenLabel -->


    <owl:AnnotationProperty rdf:about="http://www.w3.org/2004/02/skos/core#hiddenLabel">
        <rdfs:comment xml:lang="en">The range of skos:hiddenLabel is the class of RDF plain literals.</rdfs:comment>
        <rdfs:comment xml:lang="en">skos:prefLabel, skos:altLabel and skos:hiddenLabel are pairwise disjoint properties.</rdfs:comment>
        <rdfs:isDefinedBy rdf:resource="http://www.w3.org/2004/02/skos/core"/>
        <rdfs:label xml:lang="en">hidden label</rdfs:label>
        <skos:definition xml:lang="en">A lexical label for a resource that should be hidden when generating visual displays of the resource, but should still be accessible to free text search operations.</skos:definition>
        <rdfs:subPropertyOf rdf:resource="http://www.w3.org/2000/01/rdf-schema#label"/>
    </owl:AnnotationProperty>
    


    <!-- http://www.w3.org/2004/02/skos/core#historyNote -->


    <owl:AnnotationProperty rdf:about="http://www.w3.org/2004/02/skos/core#historyNote">
        <rdfs:isDefinedBy rdf:resource="http://www.w3.org/2004/02/skos/core"/>
        <rdfs:label xml:lang="en">history note</rdfs:label>
        <skos:definition xml:lang="en">A note about the past state/use/meaning of a concept.</skos:definition>
        <rdfs:subPropertyOf rdf:resource="http://www.w3.org/2004/02/skos/core#note"/>
    </owl:AnnotationProperty>
    


    <!-- http://www.w3.org/2004/02/skos/core#note -->


    <owl:AnnotationProperty rdf:about="http://www.w3.org/2004/02/skos/core#note">
        <rdfs:isDefinedBy rdf:resource="http://www.w3.org/2004/02/skos/core"/>
        <rdfs:label xml:lang="en">note</rdfs:label>
        <skos:definition xml:lang="en">A general note, for any purpose.</skos:definition>
        <skos:scopeNote xml:lang="en">This property may be used directly, or as a super-property for more specific note types.</skos:scopeNote>
    </owl:AnnotationProperty>
    


    <!-- http://www.w3.org/2004/02/skos/core#prefLabel -->


    <owl:AnnotationProperty rdf:about="http://www.w3.org/2004/02/skos/core#prefLabel">
        <rdfs:comment xml:lang="en">A resource has no more than one value of skos:prefLabel per language tag, and no more than one value of skos:prefLabel without language tag.</rdfs:comment>
        <rdfs:comment xml:lang="en">The range of skos:prefLabel is the class of RDF plain literals.</rdfs:comment>
        <rdfs:comment xml:lang="en">skos:prefLabel, skos:altLabel and skos:hiddenLabel are pairwise
      disjoint properties.</rdfs:comment>
        <rdfs:isDefinedBy rdf:resource="http://www.w3.org/2004/02/skos/core"/>
        <rdfs:label xml:lang="en">preferred label</rdfs:label>
        <skos:definition xml:lang="en">The preferred lexical label for a resource, in a given language.</skos:definition>
        <rdfs:subPropertyOf rdf:resource="http://www.w3.org/2000/01/rdf-schema#label"/>
    </owl:AnnotationProperty>
    


    <!-- http://www.w3.org/2004/02/skos/core#scopeNote -->


    <owl:AnnotationProperty rdf:about="http://www.w3.org/2004/02/skos/core#scopeNote">
        <rdfs:isDefinedBy rdf:resource="http://www.w3.org/2004/02/skos/core"/>
        <rdfs:label xml:lang="en">scope note</rdfs:label>
        <skos:definition xml:lang="en">A note that helps to clarify the meaning and/or the use of a concept.</skos:definition>
        <rdfs:subPropertyOf rdf:resource="http://www.w3.org/2004/02/skos/core#note"/>
    </owl:AnnotationProperty>
    


    <!-- 
    ///////////////////////////////////////////////////////////////////////////////////////
    //
    // Object Properties
    //
    ///////////////////////////////////////////////////////////////////////////////////////
     -->


    


    <!-- http://www.w3.org/2004/02/skos/core#broadMatch -->


    <owl:ObjectProperty rdf:about="http://www.w3.org/2004/02/skos/core#broadMatch">
        <rdfs:subPropertyOf rdf:resource="http://www.w3.org/2004/02/skos/core#broader"/>
        <rdfs:subPropertyOf rdf:resource="http://www.w3.org/2004/02/skos/core#mappingRelation"/>
        <owl:inverseOf rdf:resource="http://www.w3.org/2004/02/skos/core#narrowMatch"/>
        <rdfs:isDefinedBy rdf:resource="http://www.w3.org/2004/02/skos/core"/>
        <rdfs:label xml:lang="en">has broader match</rdfs:label>
        <skos:definition xml:lang="en">skos:broadMatch is used to state a hierarchical mapping link between two conceptual resources in different concept schemes.</skos:definition>
    </owl:ObjectProperty>
    


    <!-- http://www.w3.org/2004/02/skos/core#broader -->


    <owl:ObjectProperty rdf:about="http://www.w3.org/2004/02/skos/core#broader">
        <rdfs:subPropertyOf rdf:resource="http://www.w3.org/2004/02/skos/core#broaderTransitive"/>
        <rdfs:comment xml:lang="en">Broader concepts are typically rendered as parents in a concept hierarchy (tree).</rdfs:comment>
        <rdfs:isDefinedBy rdf:resource="http://www.w3.org/2004/02/skos/core"/>
        <rdfs:label xml:lang="en">has broader</rdfs:label>
        <skos:definition xml:lang="en">Relates a concept to a concept that is more general in meaning.</skos:definition>
        <skos:scopeNote xml:lang="en">By convention, skos:broader is only used to assert an immediate (i.e. direct) hierarchical link between two conceptual resources.</skos:scopeNote>
    </owl:ObjectProperty>
    


    <!-- http://www.w3.org/2004/02/skos/core#broaderTransitive -->


    <owl:ObjectProperty rdf:about="http://www.w3.org/2004/02/skos/core#broaderTransitive">
        <rdfs:subPropertyOf rdf:resource="http://www.w3.org/2004/02/skos/core#semanticRelation"/>
        <owl:inverseOf rdf:resource="http://www.w3.org/2004/02/skos/core#narrowerTransitive"/>
        <rdf:type rdf:resource="http://www.w3.org/2002/07/owl#TransitiveProperty"/>
        <rdfs:isDefinedBy rdf:resource="http://www.w3.org/2004/02/skos/core"/>
        <rdfs:label xml:lang="en">has broader transitive</rdfs:label>
        <skos:definition>skos:broaderTransitive is a transitive superproperty of skos:broader.</skos:definition>
        <skos:scopeNote xml:lang="en">By convention, skos:broaderTransitive is not used to make assertions. Rather, the properties can be used to draw inferences about the transitive closure of the hierarchical relation, which is useful e.g. when implementing a simple query expansion algorithm in a search application.</skos:scopeNote>
    </owl:ObjectProperty>
    


    <!-- http://www.w3.org/2004/02/skos/core#closeMatch -->


    <owl:ObjectProperty rdf:about="http://www.w3.org/2004/02/skos/core#closeMatch">
        <rdfs:subPropertyOf rdf:resource="http://www.w3.org/2004/02/skos/core#mappingRelation"/>
        <rdf:type rdf:resource="http://www.w3.org/2002/07/owl#SymmetricProperty"/>
        <rdfs:isDefinedBy rdf:resource="http://www.w3.org/2004/02/skos/core"/>
        <rdfs:label xml:lang="en">has close match</rdfs:label>
        <skos:definition xml:lang="en">skos:closeMatch is used to link two concepts that are sufficiently similar that they can be used interchangeably in some information retrieval applications. In order to avoid the possibility of &quot;compound errors&quot; when combining mappings across more than two concept schemes, skos:closeMatch is not declared to be a transitive property.</skos:definition>
    </owl:ObjectProperty>
    


    <!-- http://www.w3.org/2004/02/skos/core#exactMatch -->


    <owl:ObjectProperty rdf:about="http://www.w3.org/2004/02/skos/core#exactMatch">
        <rdfs:subPropertyOf rdf:resource="http://www.w3.org/2004/02/skos/core#closeMatch"/>
        <rdf:type rdf:resource="http://www.w3.org/2002/07/owl#SymmetricProperty"/>
        <rdf:type rdf:resource="http://www.w3.org/2002/07/owl#TransitiveProperty"/>
        <rdfs:comment xml:lang="en">skos:exactMatch is disjoint with each of the properties skos:broadMatch and skos:relatedMatch.</rdfs:comment>
        <rdfs:isDefinedBy rdf:resource="http://www.w3.org/2004/02/skos/core"/>
        <rdfs:label xml:lang="en">has exact match</rdfs:label>
        <skos:definition xml:lang="en">skos:exactMatch is used to link two concepts, indicating a high degree of confidence that the concepts can be used interchangeably across a wide range of information retrieval applications. skos:exactMatch is a transitive property, and is a sub-property of skos:closeMatch.</skos:definition>
    </owl:ObjectProperty>
    


    <!-- http://www.w3.org/2004/02/skos/core#hasTopConcept -->


    <owl:ObjectProperty rdf:about="http://www.w3.org/2004/02/skos/core#hasTopConcept">
        <owl:inverseOf rdf:resource="http://www.w3.org/2004/02/skos/core#topConceptOf"/>
        <rdfs:domain rdf:resource="http://www.w3.org/2004/02/skos/core#ConceptScheme"/>
        <rdfs:range rdf:resource="http://www.w3.org/2004/02/skos/core#Concept"/>
        <rdfs:isDefinedBy rdf:resource="http://www.w3.org/2004/02/skos/core"/>
        <rdfs:label xml:lang="en">has top concept</rdfs:label>
        <skos:definition xml:lang="en">Relates, by convention, a concept scheme to a concept which is topmost in the broader/narrower concept hierarchies for that scheme, providing an entry point to these hierarchies.</skos:definition>
    </owl:ObjectProperty>
    


    <!-- http://www.w3.org/2004/02/skos/core#inScheme -->


    <owl:ObjectProperty rdf:about="http://www.w3.org/2004/02/skos/core#inScheme">
        <rdfs:range rdf:resource="http://www.w3.org/2004/02/skos/core#ConceptScheme"/>
        <rdfs:isDefinedBy rdf:resource="http://www.w3.org/2004/02/skos/core"/>
        <rdfs:label xml:lang="en">is in scheme</rdfs:label>
        <skos:definition xml:lang="en">Relates a resource (for example a concept) to a concept scheme in which it is included.</skos:definition>
        <skos:scopeNote xml:lang="en">A concept may be a member of more than one concept scheme.</skos:scopeNote>
    </owl:ObjectProperty>
    


    <!-- http://www.w3.org/2004/02/skos/core#mappingRelation -->


    <owl:ObjectProperty rdf:about="http://www.w3.org/2004/02/skos/core#mappingRelation">
        <rdfs:subPropertyOf rdf:resource="http://www.w3.org/2004/02/skos/core#semanticRelation"/>
        <rdfs:comment xml:lang="en">These concept mapping relations mirror semantic relations, and the data model defined below is similar (with the exception of skos:exactMatch) to the data model defined for semantic relations. A distinct vocabulary is provided for concept mapping relations, to provide a convenient way to differentiate links within a concept scheme from links between concept schemes. However, this pattern of usage is not a formal requirement of the SKOS data model, and relies on informal definitions of best practice.</rdfs:comment>
        <rdfs:isDefinedBy rdf:resource="http://www.w3.org/2004/02/skos/core"/>
        <rdfs:label xml:lang="en">is in mapping relation with</rdfs:label>
        <skos:definition xml:lang="en">Relates two concepts coming, by convention, from different schemes, and that have comparable meanings</skos:definition>
    </owl:ObjectProperty>
    


    <!-- http://www.w3.org/2004/02/skos/core#member -->


    <owl:ObjectProperty rdf:about="http://www.w3.org/2004/02/skos/core#member">
        <rdfs:domain rdf:resource="http://www.w3.org/2004/02/skos/core#Collection"/>
        <rdfs:range>
            <owl:Class>
                <owl:unionOf rdf:parseType="Collection">
                    <rdf:Description rdf:about="http://www.w3.org/2004/02/skos/core#Collection"/>
                    <rdf:Description rdf:about="http://www.w3.org/2004/02/skos/core#Concept"/>
                </owl:unionOf>
            </owl:Class>
        </rdfs:range>
        <rdfs:isDefinedBy rdf:resource="http://www.w3.org/2004/02/skos/core"/>
        <rdfs:label xml:lang="en">has member</rdfs:label>
        <skos:definition xml:lang="en">Relates a collection to one of its members.</skos:definition>
    </owl:ObjectProperty>
    


    <!-- http://www.w3.org/2004/02/skos/core#memberList -->


    <owl:ObjectProperty rdf:about="http://www.w3.org/2004/02/skos/core#memberList">
        <rdf:type rdf:resource="http://www.w3.org/2002/07/owl#FunctionalProperty"/>
        <rdfs:domain rdf:resource="http://www.w3.org/2004/02/skos/core#OrderedCollection"/>
        <rdfs:range rdf:resource="http://www.w3.org/1999/02/22-rdf-syntax-ns#List"/>
        <rdfs:comment xml:lang="en">For any resource, every item in the list given as the value of the
      skos:memberList property is also a value of the skos:member property.</rdfs:comment>
        <rdfs:isDefinedBy rdf:resource="http://www.w3.org/2004/02/skos/core"/>
        <rdfs:label xml:lang="en">has member list</rdfs:label>
        <skos:definition xml:lang="en">Relates an ordered collection to the RDF list containing its members.</skos:definition>
    </owl:ObjectProperty>
    


    <!-- http://www.w3.org/2004/02/skos/core#narrowMatch -->


    <owl:ObjectProperty rdf:about="http://www.w3.org/2004/02/skos/core#narrowMatch">
        <rdfs:subPropertyOf rdf:resource="http://www.w3.org/2004/02/skos/core#mappingRelation"/>
        <rdfs:subPropertyOf rdf:resource="http://www.w3.org/2004/02/skos/core#narrower"/>
        <rdfs:isDefinedBy rdf:resource="http://www.w3.org/2004/02/skos/core"/>
        <rdfs:label xml:lang="en">has narrower match</rdfs:label>
        <skos:definition xml:lang="en">skos:narrowMatch is used to state a hierarchical mapping link between two conceptual resources in different concept schemes.</skos:definition>
    </owl:ObjectProperty>
    


    <!-- http://www.w3.org/2004/02/skos/core#narrower -->


    <owl:ObjectProperty rdf:about="http://www.w3.org/2004/02/skos/core#narrower">
        <rdfs:subPropertyOf rdf:resource="http://www.w3.org/2004/02/skos/core#narrowerTransitive"/>
        <owl:inverseOf rdf:resource="http://www.w3.org/2004/02/skos/core#broader"/>
        <rdfs:comment xml:lang="en">Narrower concepts are typically rendered as children in a concept hierarchy (tree).</rdfs:comment>
        <rdfs:isDefinedBy rdf:resource="http://www.w3.org/2004/02/skos/core"/>
        <rdfs:label xml:lang="en">has narrower</rdfs:label>
        <skos:definition xml:lang="en">Relates a concept to a concept that is more specific in meaning.</skos:definition>
        <skos:scopeNote xml:lang="en">By convention, skos:broader is only used to assert an immediate (i.e. direct) hierarchical link between two conceptual resources.</skos:scopeNote>
    </owl:ObjectProperty>
    


    <!-- http://www.w3.org/2004/02/skos/core#narrowerTransitive -->


    <owl:ObjectProperty rdf:about="http://www.w3.org/2004/02/skos/core#narrowerTransitive">
        <rdfs:subPropertyOf rdf:resource="http://www.w3.org/2004/02/skos/core#semanticRelation"/>
        <rdf:type rdf:resource="http://www.w3.org/2002/07/owl#TransitiveProperty"/>
        <rdfs:isDefinedBy rdf:resource="http://www.w3.org/2004/02/skos/core"/>
        <rdfs:label xml:lang="en">has narrower transitive</rdfs:label>
        <skos:definition>skos:narrowerTransitive is a transitive superproperty of skos:narrower.</skos:definition>
        <skos:scopeNote xml:lang="en">By convention, skos:narrowerTransitive is not used to make assertions. Rather, the properties can be used to draw inferences about the transitive closure of the hierarchical relation, which is useful e.g. when implementing a simple query expansion algorithm in a search application.</skos:scopeNote>
    </owl:ObjectProperty>
    


    <!-- http://www.w3.org/2004/02/skos/core#related -->


    <owl:ObjectProperty rdf:about="http://www.w3.org/2004/02/skos/core#related">
        <rdfs:subPropertyOf rdf:resource="http://www.w3.org/2004/02/skos/core#semanticRelation"/>
        <rdf:type rdf:resource="http://www.w3.org/2002/07/owl#SymmetricProperty"/>
        <rdfs:comment xml:lang="en">skos:related is disjoint with skos:broaderTransitive</rdfs:comment>
        <rdfs:isDefinedBy rdf:resource="http://www.w3.org/2004/02/skos/core"/>
        <rdfs:label xml:lang="en">has related</rdfs:label>
        <skos:definition xml:lang="en">Relates a concept to a concept with which there is an associative semantic relationship.</skos:definition>
    </owl:ObjectProperty>
    


    <!-- http://www.w3.org/2004/02/skos/core#relatedMatch -->


    <owl:ObjectProperty rdf:about="http://www.w3.org/2004/02/skos/core#relatedMatch">
        <rdfs:subPropertyOf rdf:resource="http://www.w3.org/2004/02/skos/core#mappingRelation"/>
        <rdfs:subPropertyOf rdf:resource="http://www.w3.org/2004/02/skos/core#related"/>
        <rdf:type rdf:resource="http://www.w3.org/2002/07/owl#SymmetricProperty"/>
        <rdfs:isDefinedBy rdf:resource="http://www.w3.org/2004/02/skos/core"/>
        <rdfs:label xml:lang="en">has related match</rdfs:label>
        <skos:definition xml:lang="en">skos:relatedMatch is used to state an associative mapping link between two conceptual resources in different concept schemes.</skos:definition>
    </owl:ObjectProperty>
    


    <!-- http://www.w3.org/2004/02/skos/core#semanticRelation -->


    <owl:ObjectProperty rdf:about="http://www.w3.org/2004/02/skos/core#semanticRelation">
        <rdfs:domain rdf:resource="http://www.w3.org/2004/02/skos/core#Concept"/>
        <rdfs:range rdf:resource="http://www.w3.org/2004/02/skos/core#Concept"/>
        <rdfs:isDefinedBy rdf:resource="http://www.w3.org/2004/02/skos/core"/>
        <rdfs:label xml:lang="en">is in semantic relation with</rdfs:label>
        <skos:definition xml:lang="en">Links a concept to a concept related by meaning.</skos:definition>
        <skos:scopeNote xml:lang="en">This property should not be used directly, but as a super-property for all properties denoting a relationship of meaning between concepts.</skos:scopeNote>
    </owl:ObjectProperty>
    


    <!-- http://www.w3.org/2004/02/skos/core#topConceptOf -->


    <owl:ObjectProperty rdf:about="http://www.w3.org/2004/02/skos/core#topConceptOf">
        <rdfs:subPropertyOf rdf:resource="http://www.w3.org/2004/02/skos/core#inScheme"/>
        <rdfs:domain rdf:resource="http://www.w3.org/2004/02/skos/core#Concept"/>
        <rdfs:range rdf:resource="http://www.w3.org/2004/02/skos/core#ConceptScheme"/>
        <rdfs:isDefinedBy rdf:resource="http://www.w3.org/2004/02/skos/core"/>
        <rdfs:label xml:lang="en">is top concept in scheme</rdfs:label>
        <skos:definition xml:lang="en">Relates a concept to the concept scheme that it is a top level concept of.</skos:definition>
    </owl:ObjectProperty>
    


    <!-- 
    ///////////////////////////////////////////////////////////////////////////////////////
    //
    // Data properties
    //
    ///////////////////////////////////////////////////////////////////////////////////////
     -->


    


    <!-- http://www.w3.org/2004/02/skos/core#notation -->


    <owl:DatatypeProperty rdf:about="http://www.w3.org/2004/02/skos/core#notation">
        <rdfs:isDefinedBy rdf:resource="http://www.w3.org/2004/02/skos/core"/>
        <rdfs:label xml:lang="en">notation</rdfs:label>
        <skos:definition xml:lang="en">A notation, also known as classification code, is a string of characters such as &quot;T58.5&quot; or &quot;303.4833&quot; used to uniquely identify a concept within the scope of a given concept scheme.</skos:definition>
        <skos:scopeNote xml:lang="en">By convention, skos:notation is used with a typed literal in the object position of the triple.</skos:scopeNote>
    </owl:DatatypeProperty>
    


    <!-- 
    ///////////////////////////////////////////////////////////////////////////////////////
    //
    // Classes
    //
    ///////////////////////////////////////////////////////////////////////////////////////
     -->


    


    <!-- http://www.w3.org/2004/02/skos/core#Collection -->


    <owl:Class rdf:about="http://www.w3.org/2004/02/skos/core#Collection">
        <owl:disjointWith rdf:resource="http://www.w3.org/2004/02/skos/core#Concept"/>
        <owl:disjointWith rdf:resource="http://www.w3.org/2004/02/skos/core#ConceptScheme"/>
        <rdfs:isDefinedBy rdf:resource="http://www.w3.org/2004/02/skos/core"/>
        <rdfs:label xml:lang="en">Collection</rdfs:label>
        <skos:definition xml:lang="en">A meaningful collection of concepts.</skos:definition>
        <skos:scopeNote xml:lang="en">Labelled collections can be used where you would like a set of concepts to be displayed under a &apos;node label&apos; in the hierarchy.</skos:scopeNote>
    </owl:Class>
    


    <!-- http://www.w3.org/2004/02/skos/core#Concept -->


    <owl:Class rdf:about="http://www.w3.org/2004/02/skos/core#Concept">
        <owl:disjointWith rdf:resource="http://www.w3.org/2004/02/skos/core#ConceptScheme"/>
        <rdfs:isDefinedBy rdf:resource="http://www.w3.org/2004/02/skos/core"/>
        <rdfs:label xml:lang="en">Concept</rdfs:label>
        <skos:definition xml:lang="en">An idea or notion; a unit of thought.</skos:definition>
    </owl:Class>
    


    <!-- http://www.w3.org/2004/02/skos/core#ConceptScheme -->


    <owl:Class rdf:about="http://www.w3.org/2004/02/skos/core#ConceptScheme">
        <rdfs:isDefinedBy rdf:resource="http://www.w3.org/2004/02/skos/core"/>
        <rdfs:label xml:lang="en">Concept Scheme</rdfs:label>
        <skos:definition xml:lang="en">A set of concepts, optionally including statements about semantic relationships between those concepts.</skos:definition>
        <skos:example xml:lang="en">Thesauri, classification schemes, subject heading lists, taxonomies, &apos;folksonomies&apos;, and other types of controlled vocabulary are all examples of concept schemes. Concept schemes are also embedded in glossaries and terminologies.</skos:example>
        <skos:scopeNote xml:lang="en">A concept scheme may be defined to include concepts from different sources.</skos:scopeNote>
    </owl:Class>
    


    <!-- http://www.w3.org/2004/02/skos/core#OrderedCollection -->


    <owl:Class rdf:about="http://www.w3.org/2004/02/skos/core#OrderedCollection">
        <rdfs:subClassOf rdf:resource="http://www.w3.org/2004/02/skos/core#Collection"/>
        <rdfs:isDefinedBy rdf:resource="http://www.w3.org/2004/02/skos/core"/>
        <rdfs:label xml:lang="en">Ordered Collection</rdfs:label>
        <skos:definition xml:lang="en">An ordered collection of concepts, where both the grouping and the ordering are meaningful.</skos:definition>
        <skos:scopeNote xml:lang="en">Ordered collections can be used where you would like a set of concepts to be displayed in a specific order, and optionally under a &apos;node label&apos;.</skos:scopeNote>
    </owl:Class>
    


    <!-- 
    ///////////////////////////////////////////////////////////////////////////////////////
    //
    // Individuals
    //
    ///////////////////////////////////////////////////////////////////////////////////////
     -->


    


    <!-- http://w3id.org/dcri-ont/vocabulary/concept_00002 -->


    <owl:NamedIndividual rdf:about="http://w3id.org/dcri-ont/vocabulary/concept_00002">
        <rdf:type rdf:resource="http://www.w3.org/2004/02/skos/core#Concept"/>
        <skos:broader rdf:resource="http://w3id.org/dcri-ont/vocabulary/concept_00228"/>
        <skos:inScheme rdf:resource="http://w3id.org/dcri-ont/vocabulary/conceptscheme"/>
        <rdfs:comment xml:lang="en">It refers to the extent on which an intervention procedure is applied.</rdfs:comment>
        <rdfs:comment xml:lang="el">Αναφέρεται στην έκταση στην οποία εφαρμόζεται μια διαδικασία επέμβασης.</rdfs:comment>
        <rdfs:label xml:lang="en">Application extent</rdfs:label>
        <rdfs:label xml:lang="el">Έκταση εφαρμογής</rdfs:label>
        <skos:definition xml:lang="en">It refers to the extent on which an intervention procedure is applied.</skos:definition>
        <skos:definition xml:lang="el">Αναφέρεται στην έκταση στην οποία εφαρμόζεται μια διαδικασία επέμβασης.</skos:definition>
        <skos:prefLabel xml:lang="en">Application extent</skos:prefLabel>
        <skos:prefLabel xml:lang="el">Έκταση εφαρμογής</skos:prefLabel>
    </owl:NamedIndividual>
    


    <!-- http://w3id.org/dcri-ont/vocabulary/concept_00014 -->


    <owl:NamedIndividual rdf:about="http://w3id.org/dcri-ont/vocabulary/concept_00014">
        <rdf:type rdf:resource="http://www.w3.org/2004/02/skos/core#Concept"/>
        <skos:broader rdf:resource="http://w3id.org/dcri-ont/vocabulary/concept_00228"/>
        <skos:inScheme rdf:resource="http://w3id.org/dcri-ont/vocabulary/conceptscheme"/>
        <rdfs:comment xml:lang="en">It refers to the abundance of a constituent (solute) divided by the total volume of a mixture (solution).</rdfs:comment>
        <rdfs:comment xml:lang="el">Αναφέρεται στην ποσότητα ενός συστατικού (διαλυμένης ουσίας) διαιρούμενης με τον συνολικό όγκο ενός μείγματος (διαλύματος).</rdfs:comment>
        <rdfs:label xml:lang="en">Concentration</rdfs:label>
        <rdfs:label xml:lang="el">Συγκέντρωση</rdfs:label>
        <skos:definition xml:lang="en">It refers to the abundance of a constituent (solute) divided by the total volume of a mixture (solution).</skos:definition>
        <skos:definition xml:lang="el">Αναφέρεται στην ποσότητα ενός συστατικού (διαλυμένης ουσίας) διαιρούμενης με τον συνολικό όγκο ενός μείγματος (διαλύματος).</skos:definition>
        <skos:prefLabel xml:lang="en">Concentration</skos:prefLabel>
        <skos:prefLabel xml:lang="el">Συγκέντρωση</skos:prefLabel>
    </owl:NamedIndividual>
    


    <!-- http://w3id.org/dcri-ont/vocabulary/concept_00018 -->


    <owl:NamedIndividual rdf:about="http://w3id.org/dcri-ont/vocabulary/concept_00018">
        <rdf:type rdf:resource="http://www.w3.org/2004/02/skos/core#Concept"/>
        <skos:broader rdf:resource="http://w3id.org/dcri-ont/vocabulary/concept_00225"/>
        <skos:inScheme rdf:resource="http://w3id.org/dcri-ont/vocabulary/conceptscheme"/>
        <rdfs:comment xml:lang="en">It refers to the re-establishment of mechanical strength, improvment of the internal cohesion and generally stabilisation of degraded or weakend areas or layers by introducing or attaching adhesive products that will hold the areas or layers together.</rdfs:comment>
        <rdfs:comment xml:lang="el">Αναφέρεται στην επαναφορά της μηχανικής στερεότητας, στην βελτίωση της εσωτερικής συνοχής και την γενική σταθεροποίηση φθαρμένων ή αδύναμων περιοχών ή στρωμάτων εισάγοντας ή προσαρτώντας συγκολλητικά υλικά τα οποία θα συγκρατήσουν τις περιοχές ή τα στρώματα μεταξύ τους.</rdfs:comment>
        <rdfs:label xml:lang="en">Consolidation</rdfs:label>
        <rdfs:label xml:lang="el">Στερέωση</rdfs:label>
        <skos:definition xml:lang="en">It refers to the re-establishment of mechanical strength, improvment of the internal cohesion and generally stabilisation of degraded or weakend areas or layers by introducing or attaching adhesive products that will hold the areas or layers together.</skos:definition>
        <skos:definition xml:lang="el">Αναφέρεται στην επαναφορά της μηχανικής στερεότητας, στην βελτίωση της εσωτερικής συνοχής και την γενική σταθεροποίηση φθαρμένων ή αδύναμων περιοχών ή στρωμάτων εισάγοντας ή προσαρτώντας συγκολλητικά υλικά τα οποία θα συγκρατήσουν τις περιοχές ή τα στρώματα μεταξύ τους.</skos:definition>
        <skos:prefLabel xml:lang="en">Consolidation</skos:prefLabel>
        <skos:prefLabel xml:lang="el">Στερέωση</skos:prefLabel>
    </owl:NamedIndividual>
    


    <!-- http://w3id.org/dcri-ont/vocabulary/concept_00019 -->


    <owl:NamedIndividual rdf:about="http://w3id.org/dcri-ont/vocabulary/concept_00019">
        <rdf:type rdf:resource="http://www.w3.org/2004/02/skos/core#Concept"/>
        <skos:broader rdf:resource="http://w3id.org/dcri-ont/vocabulary/concept_00225"/>
        <skos:inScheme rdf:resource="http://w3id.org/dcri-ont/vocabulary/conceptscheme"/>
        <rdfs:comment xml:lang="en">It refers to the making of an area or surface of a conservation object firm and stable.</rdfs:comment>
        <rdfs:comment xml:lang="el">Αναφέρεται στο να καταστεί μια περιοχή ή επιφάνεια ενός αντικειμένου συντήρησης σταθερή.</rdfs:comment>
        <rdfs:label xml:lang="en">Fixing</rdfs:label>
        <rdfs:label xml:lang="el">Στερέωση</rdfs:label>
        <skos:definition xml:lang="en">It refers to the making of an area or surface of a conservation object firm and stable.</skos:definition>
        <skos:definition xml:lang="el">Αναφέρεται στο να καταστεί μια περιοχή ή επιφάνεια ενός αντικειμένου συντήρησης σταθερή.</skos:definition>
        <skos:prefLabel xml:lang="en">Fixing</skos:prefLabel>
        <skos:prefLabel xml:lang="el">Στερέωση</skos:prefLabel>
    </owl:NamedIndividual>
    


    <!-- http://w3id.org/dcri-ont/vocabulary/concept_00020 -->


    <owl:NamedIndividual rdf:about="http://w3id.org/dcri-ont/vocabulary/concept_00020">
        <rdf:type rdf:resource="http://www.w3.org/2004/02/skos/core#Concept"/>
        <skos:broader rdf:resource="http://w3id.org/dcri-ont/vocabulary/concept_00225"/>
        <skos:inScheme rdf:resource="http://w3id.org/dcri-ont/vocabulary/conceptscheme"/>
        <skos:narrower rdf:resource="http://w3id.org/dcri-ont/vocabulary/concept_00021"/>
        <skos:narrower rdf:resource="http://w3id.org/dcri-ont/vocabulary/concept_00023"/>
        <skos:narrower rdf:resource="http://w3id.org/dcri-ont/vocabulary/concept_00025"/>
        <skos:narrower rdf:resource="http://w3id.org/dcri-ont/vocabulary/concept_00026"/>
        <skos:narrower rdf:resource="http://w3id.org/dcri-ont/vocabulary/concept_00027"/>
        <rdfs:comment xml:lang="en">It refers to the process of removing dirt, foreign matter, products of alteration, surface coatings, discolorations, or other undesired matter from a substrate.</rdfs:comment>
        <rdfs:comment xml:lang="el">Αναφέρεται στην διαδικασία απομάκρυνσης βρωμιάς, ξένου υλικού, προιόντων αλλοίωσης, επικαλυπτικών υλικών, δυσχρωμιών ή οποιουδήποτε μη επιθυμητού υλικού από μια επιφάνεια.</rdfs:comment>
        <rdfs:label xml:lang="en">Cleaning</rdfs:label>
        <rdfs:label xml:lang="el">Καθαρισμός</rdfs:label>
        <skos:definition xml:lang="en">It refers to the process of removing dirt, foreign matter, products of alteration, surface coatings, discolorations, or other undesired matter from a substrate.</skos:definition>
        <skos:definition xml:lang="el">Αναφέρεται στην διαδικασία απομάκρυνσης βρωμιάς, ξένου υλικού, προιόντων αλλοίωσης, επικαλυπτικών υλικών, δυσχρωμιών ή οποιουδήποτε μη επιθυμητού υλικού από μια επιφάνεια.</skos:definition>
        <skos:prefLabel xml:lang="en">Cleaning</skos:prefLabel>
        <skos:prefLabel xml:lang="el">Καθαρισμός</skos:prefLabel>
    </owl:NamedIndividual>
    


    <!-- http://w3id.org/dcri-ont/vocabulary/concept_00021 -->


    <owl:NamedIndividual rdf:about="http://w3id.org/dcri-ont/vocabulary/concept_00021">
        <rdf:type rdf:resource="http://www.w3.org/2004/02/skos/core#Concept"/>
        <skos:broader rdf:resource="http://w3id.org/dcri-ont/vocabulary/concept_00020"/>
        <skos:inScheme rdf:resource="http://w3id.org/dcri-ont/vocabulary/conceptscheme"/>
        <skos:narrower rdf:resource="http://w3id.org/dcri-ont/vocabulary/concept_00022"/>
        <rdfs:comment xml:lang="en">It refers to a cleaning category, during which the removing of undesired matter from a substrate is achieved through forces that break the bonds between the undesired matter and the substrate. The forces exertion is done mannually with various tools or with the aid of equipment.</rdfs:comment>
        <rdfs:comment xml:lang="el">Αναφέρεται σε μια κατηγορία καθαρισμού, κατά την οποία η απομάκρυνση του μη επιθυμητού υλικού από μια επιφάνεια επιτυγχάνεται με την άσκηση δύναμης ώστε να σπάσει ο δεσμός μεταξύ του μη επιθυμητού υλικού και της επιφάνειας. Η άσκηση της δύναμης γίνεται χειροκίνητα, με την χρήση εργαλείων (π.χ. πινέλο, σπάτουλα) ή την βοήθεια άλλου εξοπλισμού (π.χ. φυσητήρας, πουάρ).</rdfs:comment>
        <rdfs:label xml:lang="en">Mechanical cleaning</rdfs:label>
        <rdfs:label xml:lang="el">Μηχανικός καθαρισμός</rdfs:label>
        <skos:definition xml:lang="en">It refers to a cleaning category, during which the removing of undesired matter from a substrate is achieved through forces that break the bonds between the undesired matter and the substrate. The forces exertion is done mannually with various tools or with the aid of equipment.</skos:definition>
        <skos:definition xml:lang="el">Αναφέρεται σε μια κατηγορία καθαρισμού, κατά την οποία η απομάκρυνση του μη επιθυμητού υλικού από μια επιφάνεια επιτυγχάνεται με την άσκηση δύναμης ώστε να σπάσει ο δεσμός μεταξύ του μη επιθυμητού υλικού και της επιφάνειας. Η άσκηση της δύναμης γίνεται χειροκίνητα, με την χρήση εργαλείων (π.χ. πινέλο, σπάτουλα) ή την βοήθεια άλλου εξοπλισμού (π.χ. φυσητήρας, πουάρ).</skos:definition>
        <skos:prefLabel xml:lang="en">Mechanical cleaning</skos:prefLabel>
        <skos:prefLabel xml:lang="el">Μηχανικός καθαρισμός</skos:prefLabel>
    </owl:NamedIndividual>
    


    <!-- http://w3id.org/dcri-ont/vocabulary/concept_00022 -->


    <owl:NamedIndividual rdf:about="http://w3id.org/dcri-ont/vocabulary/concept_00022">
        <rdf:type rdf:resource="http://www.w3.org/2004/02/skos/core#Concept"/>
        <skos:broader rdf:resource="http://w3id.org/dcri-ont/vocabulary/concept_00021"/>
        <skos:inScheme rdf:resource="http://w3id.org/dcri-ont/vocabulary/conceptscheme"/>
        <skos:narrower rdf:resource="http://w3id.org/dcri-ont/vocabulary/concept_00032"/>
        <rdfs:comment xml:lang="en">It refers to a mechanical cleaning category, which aim to reduce or remove superficial deposits (e.g. dust, soil, insect droppings). In the context of paper conservation the term describes more particulalrly cleaning with the use of erasers, brush, cloth, vacuum or blower.</rdfs:comment>
        <rdfs:comment xml:lang="el">Αναφέρεται σε μια κατηγορία μηχανικού καθαρισμού, η οποία στοχεύει στην μείωση ή απομάκρυνση των επιφανειακών επικαθίσεων (π.χ. σκόνη, χώμα, περιττώματα εντόμων). Στο πλαίσιο της συντήρησης χαρτιού ο όρος χρησιμοποιείται για να περιγράψει τον καθαρισμό πιο συγκεκριμένα με την χρήση γόμας, πινέλου, υφάσματος, απορροφητικής σκούπας ή φυσητήρα.</rdfs:comment>
        <rdfs:label xml:lang="en">Dry cleaning (paper)</rdfs:label>
        <rdfs:label xml:lang="el">Ξηρός καθαρισμός (χαρτί)</rdfs:label>
        <skos:altLabel xml:lang="en">Surface cleaning</skos:altLabel>
        <skos:altLabel xml:lang="el">Επιφανειακός καθαρισμός</skos:altLabel>
        <skos:definition xml:lang="en">It refers to a mechanical cleaning category, which aim to reduce or remove superficial deposits (e.g. dust, soil, insect droppings). In the context of paper conservation the term describes more particulalrly cleaning with the use of erasers, brush, cloth, vacuum or blower.</skos:definition>
        <skos:definition xml:lang="el">Αναφέρεται σε μια κατηγορία μηχανικού καθαρισμού, η οποία στοχεύει στην μείωση ή απομάκρυνση των επιφανειακών επικαθίσεων (π.χ. σκόνη, χώμα, περιττώματα εντόμων). Στο πλαίσιο της συντήρησης χαρτιού ο όρος χρησιμοποιείται για να περιγράψει τον καθαρισμό πιο συγκεκριμένα με την χρήση γόμας, πινέλου, υφάσματος, απορροφητικής σκούπας ή φυσητήρα.</skos:definition>
        <skos:prefLabel xml:lang="en">Dry cleaning (paper)</skos:prefLabel>
        <skos:prefLabel xml:lang="el">Ξηρός καθαρισμός (χαρτί)</skos:prefLabel>
    </owl:NamedIndividual>
    


    <!-- http://w3id.org/dcri-ont/vocabulary/concept_00023 -->


    <owl:NamedIndividual rdf:about="http://w3id.org/dcri-ont/vocabulary/concept_00023">
        <rdf:type rdf:resource="http://www.w3.org/2004/02/skos/core#Concept"/>
        <skos:broader rdf:resource="http://w3id.org/dcri-ont/vocabulary/concept_00020"/>
        <skos:inScheme rdf:resource="http://w3id.org/dcri-ont/vocabulary/conceptscheme"/>
        <skos:narrower rdf:resource="http://w3id.org/dcri-ont/vocabulary/concept_00024"/>
        <rdfs:comment xml:lang="en">It refers to a cleaning category, during which the removing of undesired matter from a substrate is achieved through its dissolutions by means of organic solvents, water and/or chemical reagents.</rdfs:comment>
        <rdfs:comment xml:lang="el">Αναφέρεται σε μια κατηγορία καθαρισμού, κατά την οποία η απομάκρυνση του μη επιθυμητού υλικού από μια επιφάνεια επιτυγχάνεται με την διάλυσή του με την χρήση οργανικών διαλυτών, νερού και/ή χημικών αντιδραστηρίων.</rdfs:comment>
        <rdfs:label xml:lang="en">Physico-chemical cleaning</rdfs:label>
        <rdfs:label xml:lang="el">Φυσικοχημικός καθαρισμός</rdfs:label>
        <skos:definition xml:lang="en">It refers to a cleaning category, during which the removing of undesired matter from a substrate is achieved through its dissolutions by means of organic solvents, water and/or chemical reagents.</skos:definition>
        <skos:definition xml:lang="el">Αναφέρεται σε μια κατηγορία καθαρισμού, κατά την οποία η απομάκρυνση του μη επιθυμητού υλικού από μια επιφάνεια επιτυγχάνεται με την διάλυσή του με την χρήση οργανικών διαλυτών, νερού και/ή χημικών αντιδραστηρίων.</skos:definition>
        <skos:prefLabel xml:lang="en">Physico-chemical cleaning</skos:prefLabel>
        <skos:prefLabel xml:lang="el">Φυσικοχημικός καθαρισμός</skos:prefLabel>
    </owl:NamedIndividual>
    


    <!-- http://w3id.org/dcri-ont/vocabulary/concept_00024 -->


    <owl:NamedIndividual rdf:about="http://w3id.org/dcri-ont/vocabulary/concept_00024">
        <rdf:type rdf:resource="http://www.w3.org/2004/02/skos/core#Concept"/>
        <skos:broader rdf:resource="http://w3id.org/dcri-ont/vocabulary/concept_00023"/>
        <skos:inScheme rdf:resource="http://w3id.org/dcri-ont/vocabulary/conceptscheme"/>
        <rdfs:comment xml:lang="en">It refers to a physico-chemical cleaning category, during which the removing of undesired matter from a substrate is achieved through the use of aqueous medium.</rdfs:comment>
        <rdfs:comment xml:lang="el">Αναφέρεται σε μια κατηγορία φυσικοχημικού καθαρισμού, κατά την οποία η απομάκρυνση του μη επιθυμητού υλικού από μια επιφάνεια επιτυγχάνεται με την χρήση υδατικού μέσου.</rdfs:comment>
        <rdfs:label xml:lang="en">Wet cleaning</rdfs:label>
        <rdfs:label xml:lang="el">Υγρός καθαρισμός</rdfs:label>
        <skos:altLabel xml:lang="el">Υδατικός καθαρισμός</skos:altLabel>
        <skos:definition xml:lang="en">It refers to a physico-chemical cleaning category, during which the removing of undesired matter from a substrate is achieved through the use of aqueous medium.</skos:definition>
        <skos:definition xml:lang="el">Αναφέρεται σε μια κατηγορία φυσικοχημικού καθαρισμού, κατά την οποία η απομάκρυνση του μη επιθυμητού υλικού από μια επιφάνεια επιτυγχάνεται με την χρήση υδατικού μέσου.</skos:definition>
        <skos:prefLabel xml:lang="en">Wet cleaning</skos:prefLabel>
        <skos:prefLabel xml:lang="el">Υγρός καθαρισμός</skos:prefLabel>
    </owl:NamedIndividual>
    


    <!-- http://w3id.org/dcri-ont/vocabulary/concept_00025 -->


    <owl:NamedIndividual rdf:about="http://w3id.org/dcri-ont/vocabulary/concept_00025">
        <rdf:type rdf:resource="http://www.w3.org/2004/02/skos/core#Concept"/>
        <skos:broader rdf:resource="http://w3id.org/dcri-ont/vocabulary/concept_00020"/>
        <skos:inScheme rdf:resource="http://w3id.org/dcri-ont/vocabulary/conceptscheme"/>
        <rdfs:comment xml:lang="en">It refers to a cleaning category, during which the removing of undesired matter from a substrate is achieved through the use of equipment of laser technology.</rdfs:comment>
        <rdfs:comment xml:lang="el">Αναφέρεται σε μια κατηγορία καθαρισμού, κατά την οποία η απομάκρυνση του μη επιθυμητού υλικού από μια επιφάνεια επιτυγχάνεται με την χρήση εξοπλισμού τεχνολογίας laser.</rdfs:comment>
        <rdfs:label xml:lang="en">Laser cleaning</rdfs:label>
        <rdfs:label xml:lang="el">Καθαρισμός με laser</rdfs:label>
        <skos:definition xml:lang="en">It refers to a cleaning category, during which the removing of undesired matter from a substrate is achieved through the use of equipment of laser technology.</skos:definition>
        <skos:definition xml:lang="el">Αναφέρεται σε μια κατηγορία καθαρισμού, κατά την οποία η απομάκρυνση του μη επιθυμητού υλικού από μια επιφάνεια επιτυγχάνεται με την χρήση εξοπλισμού τεχνολογίας laser.</skos:definition>
        <skos:prefLabel xml:lang="en">Laser cleaning</skos:prefLabel>
        <skos:prefLabel xml:lang="el">Καθαρισμός με laser</skos:prefLabel>
    </owl:NamedIndividual>
    


    <!-- http://w3id.org/dcri-ont/vocabulary/concept_00026 -->


    <owl:NamedIndividual rdf:about="http://w3id.org/dcri-ont/vocabulary/concept_00026">
        <rdf:type rdf:resource="http://www.w3.org/2004/02/skos/core#Concept"/>
        <skos:broader rdf:resource="http://w3id.org/dcri-ont/vocabulary/concept_00020"/>
        <skos:inScheme rdf:resource="http://w3id.org/dcri-ont/vocabulary/conceptscheme"/>
        <rdfs:comment xml:lang="en">It refers to a cleaning category, during which the removing of undesired matter from a substrate is achieved through the use of living organisms and/or their enzymes as cleaning agents by controlled reproduction of their metabolic processes.</rdfs:comment>
        <rdfs:comment xml:lang="el">Αναφέρεται σε μια κατηγορία καθαρισμού, κατά την οποία η απομάκρυνση του μη επιθυμητού υλικού από μια επιφάνεια επιτυγχάνεται με την χρήση έμβιων οργανισμών και/ή των ενζύμων τους ως μέσα καθαρισμού με την ελεγχόμενη αναπαραγωγή των μεταβολικών τους διαδικασιών.</rdfs:comment>
        <rdfs:label xml:lang="en">Biological cleaning</rdfs:label>
        <rdfs:label xml:lang="el">Βιολογικός καθαρισμός</rdfs:label>
        <skos:altLabel xml:lang="en">Biocleaning</skos:altLabel>
        <skos:definition xml:lang="en">It refers to a cleaning category, during which the removing of undesired matter from a substrate is achieved through the use of living organisms and/or their enzymes as cleaning agents by controlled reproduction of their metabolic processes.</skos:definition>
        <skos:definition xml:lang="el">Αναφέρεται σε μια κατηγορία καθαρισμού, κατά την οποία η απομάκρυνση του μη επιθυμητού υλικού από μια επιφάνεια επιτυγχάνεται με την χρήση έμβιων οργανισμών και/ή των ενζύμων τους ως μέσα καθαρισμού με την ελεγχόμενη αναπαραγωγή των μεταβολικών τους διαδικασιών.</skos:definition>
        <skos:prefLabel xml:lang="en">Biological cleaning</skos:prefLabel>
        <skos:prefLabel xml:lang="el">Βιολογικός καθαρισμός</skos:prefLabel>
    </owl:NamedIndividual>
    


    <!-- http://w3id.org/dcri-ont/vocabulary/concept_00027 -->


    <owl:NamedIndividual rdf:about="http://w3id.org/dcri-ont/vocabulary/concept_00027">
        <rdf:type rdf:resource="http://www.w3.org/2004/02/skos/core#Concept"/>
        <skos:broader rdf:resource="http://w3id.org/dcri-ont/vocabulary/concept_00020"/>
        <skos:inScheme rdf:resource="http://w3id.org/dcri-ont/vocabulary/conceptscheme"/>
        <rdfs:comment xml:lang="en">It refers to a cleaning category, during which the removing of undesired matter from a substrate is achieved through the use of equipment of gels.</rdfs:comment>
        <rdfs:comment xml:lang="el">Αναφέρεται σε μια κατηγορία καθαρισμού, κατά την οποία η απομάκρυνση του μη επιθυμητού υλικού από μια επιφάνεια επιτυγχάνεται με την χρήση γελών.</rdfs:comment>
        <rdfs:label xml:lang="en">Gel cleaning</rdfs:label>
        <rdfs:label xml:lang="el">Καθαρισμός με γέλη</rdfs:label>
        <skos:definition xml:lang="en">It refers to a cleaning category, during which the removing of undesired matter from a substrate is achieved through the use of equipment of gels.</skos:definition>
        <skos:definition xml:lang="el">Αναφέρεται σε μια κατηγορία καθαρισμού, κατά την οποία η απομάκρυνση του μη επιθυμητού υλικού από μια επιφάνεια επιτυγχάνεται με την χρήση γελών.</skos:definition>
        <skos:prefLabel xml:lang="en">Gel cleaning</skos:prefLabel>
        <skos:prefLabel xml:lang="el">Καθαρισμός με γέλη</skos:prefLabel>
    </owl:NamedIndividual>
    


    <!-- http://w3id.org/dcri-ont/vocabulary/concept_00028 -->


    <owl:NamedIndividual rdf:about="http://w3id.org/dcri-ont/vocabulary/concept_00028">
        <rdf:type rdf:resource="http://www.w3.org/2004/02/skos/core#Concept"/>
        <skos:broader rdf:resource="http://w3id.org/dcri-ont/vocabulary/concept_00228"/>
        <skos:inScheme rdf:resource="http://w3id.org/dcri-ont/vocabulary/conceptscheme"/>
        <rdfs:comment xml:lang="en">It refers to the distance from which an intervention procedure is applied.</rdfs:comment>
        <rdfs:comment xml:lang="el">Αναφέρεται στην απόσταση από την οποία εφαρμόζεται μια διαδικασία επέμβασης.</rdfs:comment>
        <rdfs:label xml:lang="en">Application distance</rdfs:label>
        <rdfs:label xml:lang="el">Απόσταση εφαρμογής</rdfs:label>
        <skos:definition xml:lang="en">It refers to the distance from which an intervention procedure is applied.</skos:definition>
        <skos:definition xml:lang="el">Αναφέρεται στην απόσταση από την οποία εφαρμόζεται μια διαδικασία επέμβασης.</skos:definition>
        <skos:prefLabel xml:lang="en">Application distance</skos:prefLabel>
        <skos:prefLabel xml:lang="el">Απόσταση εφαρμογής</skos:prefLabel>
    </owl:NamedIndividual>
    


    <!-- http://w3id.org/dcri-ont/vocabulary/concept_00029 -->


    <owl:NamedIndividual rdf:about="http://w3id.org/dcri-ont/vocabulary/concept_00029">
        <rdf:type rdf:resource="http://www.w3.org/2004/02/skos/core#Concept"/>
        <skos:broader rdf:resource="http://w3id.org/dcri-ont/vocabulary/concept_00228"/>
        <skos:inScheme rdf:resource="http://w3id.org/dcri-ont/vocabulary/conceptscheme"/>
        <rdfs:comment xml:lang="en">It refers to the speed with which an intervention procedure is performed - how quickly can be performed.</rdfs:comment>
        <rdfs:comment xml:lang="el">Αναφέρεται στην ταχύτητα με την οποία εκτελείται μια διαδικασία επέμβασης - πόσο γρήγορη μπορεί να εκτελεστεί.</rdfs:comment>
        <rdfs:label xml:lang="en">Performance speed</rdfs:label>
        <rdfs:label xml:lang="el">Ταχύτητα ετέλεσης</rdfs:label>
        <skos:definition xml:lang="en">It refers to the speed with which an intervention procedure is performed - how quickly can be performed.</skos:definition>
        <skos:definition xml:lang="el">Αναφέρεται στην ταχύτητα με την οποία εκτελείται μια διαδικασία επέμβασης - πόσο γρήγορη μπορεί να εκτελεστεί.</skos:definition>
        <skos:prefLabel xml:lang="en">Performance speed</skos:prefLabel>
        <skos:prefLabel xml:lang="el">Ταχύτητα ετέλεσης</skos:prefLabel>
    </owl:NamedIndividual>
    


    <!-- http://w3id.org/dcri-ont/vocabulary/concept_00030 -->


    <owl:NamedIndividual rdf:about="http://w3id.org/dcri-ont/vocabulary/concept_00030">
        <rdf:type rdf:resource="http://www.w3.org/2004/02/skos/core#Concept"/>
        <skos:broader rdf:resource="http://w3id.org/dcri-ont/vocabulary/concept_00228"/>
        <skos:inScheme rdf:resource="http://w3id.org/dcri-ont/vocabulary/conceptscheme"/>
        <rdfs:comment xml:lang="en">It refers to the air velocity, provided by an intervention equipment.</rdfs:comment>
        <rdfs:comment xml:lang="el">Αναφέρεται στην ένταση αέρα την οποία παρέχει ο εξοπλισμός επέμβασης.</rdfs:comment>
        <rdfs:label xml:lang="en">Air velocity</rdfs:label>
        <rdfs:label xml:lang="el">Ένταση αέρα</rdfs:label>
        <skos:definition xml:lang="en">It refers to the air velocity, provided by an intervention equipment.</skos:definition>
        <skos:definition xml:lang="el">Αναφέρεται στην ένταση αέρα την οποία παρέχει ο εξοπλισμός επέμβασης.</skos:definition>
        <skos:prefLabel xml:lang="en">Air velocity</skos:prefLabel>
        <skos:prefLabel xml:lang="el">Ένταση αέρα</skos:prefLabel>
    </owl:NamedIndividual>
    


    <!-- http://w3id.org/dcri-ont/vocabulary/concept_00031 -->


    <owl:NamedIndividual rdf:about="http://w3id.org/dcri-ont/vocabulary/concept_00031">
        <rdf:type rdf:resource="http://www.w3.org/2004/02/skos/core#Concept"/>
        <skos:broader rdf:resource="http://w3id.org/dcri-ont/vocabulary/concept_00068"/>
        <skos:inScheme rdf:resource="http://w3id.org/dcri-ont/vocabulary/conceptscheme"/>
        <rdfs:comment xml:lang="en">Textile made in various weights, usually of flax, hemp, jute, or cotton, used especially as a support for oil and other paintings.</rdfs:comment>
        <rdfs:comment xml:lang="el">Ύφασμα φτιαγμένο σε ποικίλα βάρη, συνήθως από λινάρι, κάνναβη, γιούτα ή βαμβάκι, που χρησιμοποιείται ειδικά ως υποστήριγμα για ελαιογραφίες ή άλλους πίνακες.</rdfs:comment>
        <rdfs:label xml:lang="en">Canvas</rdfs:label>
        <rdfs:label xml:lang="el">Καμβάς</rdfs:label>
        <skos:definition xml:lang="en">Textile made in various weights, usually of flax, hemp, jute, or cotton, used especially as a support for oil and other paintings.</skos:definition>
        <skos:definition xml:lang="el">Ύφασμα φτιαγμένο σε ποικίλα βάρη, συνήθως από λινάρι, κάνναβη, γιούτα ή βαμβάκι, που χρησιμοποιείται ειδικά ως υποστήριγμα για ελαιογραφίες ή άλλους πίνακες.</skos:definition>
        <skos:prefLabel xml:lang="en">Canvas</skos:prefLabel>
        <skos:prefLabel xml:lang="el">Καμβάς</skos:prefLabel>
    </owl:NamedIndividual>
    


    <!-- http://w3id.org/dcri-ont/vocabulary/concept_00032 -->


    <owl:NamedIndividual rdf:about="http://w3id.org/dcri-ont/vocabulary/concept_00032">
        <rdf:type rdf:resource="http://www.w3.org/2004/02/skos/core#Concept"/>
        <skos:broader rdf:resource="http://w3id.org/dcri-ont/vocabulary/concept_00022"/>
        <skos:inScheme rdf:resource="http://w3id.org/dcri-ont/vocabulary/conceptscheme"/>
        <rdfs:comment xml:lang="en">It refers to a mechanical cleaning category, which aim to reduce or remove superficial deposits (e.g. dust, soil, insect droppings) using vacuum.</rdfs:comment>
        <rdfs:comment xml:lang="el">Αναφέρεται σε μια κατηγορία μηχανικού καθαρισμού, η οποία στοχεύει στην μείωση ή απομάκρυνση των επιφανειακών επικαθίσεων (π.χ. σκόνη, χώμα, περιττώματα εντόμων) χρησιμοποιώντας απορροφητική σκούπα.</rdfs:comment>
        <rdfs:label xml:lang="en">Vacuum cleaning</rdfs:label>
        <rdfs:label xml:lang="el">Καθαρισμός με απορροφητική σκούπα</rdfs:label>
        <skos:definition xml:lang="en">It refers to a mechanical cleaning category, which aim to reduce or remove superficial deposits (e.g. dust, soil, insect droppings) using vacuum.</skos:definition>
        <skos:definition xml:lang="el">Αναφέρεται σε μια κατηγορία μηχανικού καθαρισμού, η οποία στοχεύει στην μείωση ή απομάκρυνση των επιφανειακών επικαθίσεων (π.χ. σκόνη, χώμα, περιττώματα εντόμων) χρησιμοποιώντας απορροφητική σκούπα.</skos:definition>
        <skos:prefLabel xml:lang="en">Vacuum cleaning</skos:prefLabel>
        <skos:prefLabel xml:lang="el">Καθαρισμός με απορροφητική σκούπα</skos:prefLabel>
    </owl:NamedIndividual>
    


    <!-- http://w3id.org/dcri-ont/vocabulary/concept_00033 -->


    <owl:NamedIndividual rdf:about="http://w3id.org/dcri-ont/vocabulary/concept_00033">
        <rdf:type rdf:resource="http://www.w3.org/2004/02/skos/core#Concept"/>
        <skos:broader rdf:resource="http://w3id.org/dcri-ont/vocabulary/concept_00228"/>
        <skos:inScheme rdf:resource="http://w3id.org/dcri-ont/vocabulary/conceptscheme"/>
        <rdfs:comment xml:lang="en">It refers to the air flow, suction or blowing, that an intervention equipment provides.</rdfs:comment>
        <rdfs:comment xml:lang="el">Αναφέρεται στην ροή αέρα, απορρόφηση ή εκτόξευση, την οποία παρέχει ο εξοπλισμός επέμβασης.</rdfs:comment>
        <rdfs:label xml:lang="en">Air flow</rdfs:label>
        <rdfs:label xml:lang="el">Ροή αέρα</rdfs:label>
        <skos:definition xml:lang="en">It refers to the air flow, suction or blowing, that an intervention equipment provides.</skos:definition>
        <skos:definition xml:lang="el">Αναφέρεται στην ροή αέρα, απορρόφηση ή εκτόξευση, την οποία παρέχει ο εξοπλισμός επέμβασης.</skos:definition>
        <skos:prefLabel xml:lang="en">Air flow</skos:prefLabel>
        <skos:prefLabel xml:lang="el">Ροή αέρα</skos:prefLabel>
    </owl:NamedIndividual>
    


    <!-- http://w3id.org/dcri-ont/vocabulary/concept_00039 -->


    <owl:NamedIndividual rdf:about="http://w3id.org/dcri-ont/vocabulary/concept_00039">
        <rdf:type rdf:resource="http://www.w3.org/2004/02/skos/core#Concept"/>
        <skos:broader rdf:resource="http://w3id.org/dcri-ont/vocabulary/concept_00228"/>
        <skos:inScheme rdf:resource="http://w3id.org/dcri-ont/vocabulary/conceptscheme"/>
        <rdfs:comment xml:lang="en">It refers to the ability of an intervention material to preserve its optical properties through the time.</rdfs:comment>
        <rdfs:comment xml:lang="el">Αναφέρεται στην ικανότητα ενός υλικού επέμβασης να διατηρεί τις οπτικές του ιδιότητες στο πέρασμα του χρόνου.</rdfs:comment>
        <rdfs:label xml:lang="en">Optical stability</rdfs:label>
        <rdfs:label xml:lang="el">Οπτική σταθερότητα</rdfs:label>
        <skos:definition xml:lang="en">It refers to the ability of an intervention material to preserve its optical properties through the time.</skos:definition>
        <skos:definition xml:lang="el">Αναφέρεται στην ικανότητα ενός υλικού επέμβασης να διατηρεί τις οπτικές του ιδιότητες στο πέρασμα του χρόνου.</skos:definition>
        <skos:prefLabel xml:lang="en">Optical stability</skos:prefLabel>
        <skos:prefLabel xml:lang="el">Οπτική σταθερότητα</skos:prefLabel>
    </owl:NamedIndividual>
    


    <!-- http://w3id.org/dcri-ont/vocabulary/concept_00040 -->


    <owl:NamedIndividual rdf:about="http://w3id.org/dcri-ont/vocabulary/concept_00040">
        <rdf:type rdf:resource="http://www.w3.org/2004/02/skos/core#Concept"/>
        <skos:broader rdf:resource="http://w3id.org/dcri-ont/vocabulary/concept_00228"/>
        <skos:inScheme rdf:resource="http://w3id.org/dcri-ont/vocabulary/conceptscheme"/>
        <rdfs:comment xml:lang="en">It refers to the space in which an intervention procedure can be performed.</rdfs:comment>
        <rdfs:comment xml:lang="el">Αναφέρεται στον χώρο στον οποίο μπορεί να εκτελεστεί μια διαδικασία επέμβασης.</rdfs:comment>
        <rdfs:label xml:lang="en">Performance space</rdfs:label>
        <rdfs:label xml:lang="el">Χώρος εκτέλεσης</rdfs:label>
        <skos:definition xml:lang="en">It refers to the space in which an intervention procedure can be performed.</skos:definition>
        <skos:definition xml:lang="el">Αναφέρεται στον χώρο στον οποίο μπορεί να εκτελεστεί μια διαδικασία επέμβασης.</skos:definition>
        <skos:prefLabel xml:lang="en">Performance space</skos:prefLabel>
        <skos:prefLabel xml:lang="el">Χώρος εκτέλεσης</skos:prefLabel>
    </owl:NamedIndividual>
    


    <!-- http://w3id.org/dcri-ont/vocabulary/concept_00041 -->


    <owl:NamedIndividual rdf:about="http://w3id.org/dcri-ont/vocabulary/concept_00041">
        <rdf:type rdf:resource="http://www.w3.org/2004/02/skos/core#Concept"/>
        <skos:broader rdf:resource="http://w3id.org/dcri-ont/vocabulary/concept_00228"/>
        <skos:inScheme rdf:resource="http://w3id.org/dcri-ont/vocabulary/conceptscheme"/>
        <rdfs:comment xml:lang="en">It refers to the ability of an intervention supply to be moved from one location to another.</rdfs:comment>
        <rdfs:comment xml:lang="el">Αναφέρεται στην ικανότητα ενός εξαρτήματος επέμβασης να μεταφέρεται από μια τοποθεσία σε μια άλλη</rdfs:comment>
        <rdfs:label xml:lang="en">Portability</rdfs:label>
        <rdfs:label xml:lang="el">Φορητότητα</rdfs:label>
        <skos:definition xml:lang="en">It refers to the ability of an intervention supply to be moved from one location to another.</skos:definition>
        <skos:definition xml:lang="el">Αναφέρεται στην ικανότητα ενός εξαρτήματος επέμβασης να μεταφέρεται από μια τοποθεσία σε μια άλλη</skos:definition>
        <skos:prefLabel xml:lang="en">Portability</skos:prefLabel>
        <skos:prefLabel xml:lang="el">Φορητότητα</skos:prefLabel>
    </owl:NamedIndividual>
    


    <!-- http://w3id.org/dcri-ont/vocabulary/concept_00042 -->


    <owl:NamedIndividual rdf:about="http://w3id.org/dcri-ont/vocabulary/concept_00042">
        <rdf:type rdf:resource="http://www.w3.org/2004/02/skos/core#Concept"/>
        <skos:broader rdf:resource="http://w3id.org/dcri-ont/vocabulary/concept_00228"/>
        <skos:inScheme rdf:resource="http://w3id.org/dcri-ont/vocabulary/conceptscheme"/>
        <rdfs:comment xml:lang="en">It refers to the power supply that an interventino equipment needs in order to be functional.</rdfs:comment>
        <rdfs:comment xml:lang="el">Αναφέρεται στην ενέργεια που χρειάζεται ο εξοπλισμός επέμβασης για να λειτουργήσει.</rdfs:comment>
        <rdfs:label xml:lang="en">Power supply</rdfs:label>
        <rdfs:label xml:lang="el">Χρήση ενέργειας</rdfs:label>
        <skos:definition xml:lang="en">It refers to the power supply that an interventino equipment needs in order to be functional.</skos:definition>
        <skos:definition xml:lang="el">Αναφέρεται στην ενέργεια που χρειάζεται ο εξοπλισμός επέμβασης για να λειτουργήσει.</skos:definition>
        <skos:prefLabel xml:lang="en">Power supply</skos:prefLabel>
        <skos:prefLabel xml:lang="el">Χρήση ενέργειας</skos:prefLabel>
    </owl:NamedIndividual>
    


    <!-- http://w3id.org/dcri-ont/vocabulary/concept_00046 -->


    <owl:NamedIndividual rdf:about="http://w3id.org/dcri-ont/vocabulary/concept_00046">
        <rdf:type rdf:resource="http://www.w3.org/2004/02/skos/core#Concept"/>
        <skos:broader rdf:resource="http://w3id.org/dcri-ont/vocabulary/concept_00228"/>
        <skos:inScheme rdf:resource="http://w3id.org/dcri-ont/vocabulary/conceptscheme"/>
        <rdfs:comment xml:lang="en">It refers to the property of an intervention material to dissolve in a solvent.</rdfs:comment>
        <rdfs:comment xml:lang="el">Αναφέρεται στην ιδιότητα ενός υλικού επέμβασης να διαλύεται σε έναν διαλύτη.</rdfs:comment>
        <rdfs:label xml:lang="en">Solubility in solvent</rdfs:label>
        <rdfs:label xml:lang="el">Διαλυτότητα σε διαλύτη</rdfs:label>
        <skos:definition xml:lang="en">It refers to the property of an intervention material to dissolve in a solvent.</skos:definition>
        <skos:definition xml:lang="el">Αναφέρεται στην ιδιότητα ενός υλικού επέμβασης να διαλύεται σε έναν διαλύτη.</skos:definition>
        <skos:prefLabel xml:lang="en">Solubility in solvent</skos:prefLabel>
        <skos:prefLabel xml:lang="el">Διαλυτότητα σε διαλύτη</skos:prefLabel>
    </owl:NamedIndividual>
    


    <!-- http://w3id.org/dcri-ont/vocabulary/concept_00047 -->


    <owl:NamedIndividual rdf:about="http://w3id.org/dcri-ont/vocabulary/concept_00047">
        <rdf:type rdf:resource="http://www.w3.org/2004/02/skos/core#Concept"/>
        <skos:broader rdf:resource="http://w3id.org/dcri-ont/vocabulary/concept_00223"/>
        <skos:inScheme rdf:resource="http://w3id.org/dcri-ont/vocabulary/conceptscheme"/>
        <rdfs:comment xml:lang="en">A tool used for cleaning, consisting of a handle onto which feathers (e.g. ostrich feathers) are wound. It is used in the context of conservation interventions related to surface cleaning or removal of loose deposits (e.g. dust) from the surfaces of movable Cultural Heritage items.</rdfs:comment>
        <rdfs:comment xml:lang="el">Εργαλείο καθαρισμού, αποτελούμενο από μια λαβή πάνω στην οποία είναι στερεωμένα φτερά (π.χ. φτερά στρουθοκαμήλου). Χρησιμοποιείται στο πλαίσιο επεμβάσεων συντήρησης που αφορούν στον επιφανειακό καθαρισμό ή την απομάκρυνση χαλαρών επικαθίσεων (π.χ. σκόνης) από τις επιφάνειες κινητών αντικειμένων της Πολιτιστικής Κληρονομιάς.</rdfs:comment>
        <rdfs:label xml:lang="en">Feather duster</rdfs:label>
        <rdfs:label xml:lang="el">Φτερό ξεσκονίσματος</rdfs:label>
        <skos:altLabel xml:lang="el">Φτερό</skos:altLabel>
        <skos:definition xml:lang="en">A tool used for cleaning, consisting of a handle onto which feathers (e.g. ostrich feathers) are wound. It is used in the context of conservation interventions related to surface cleaning or removal of loose deposits (e.g. dust) from the surfaces of movable Cultural Heritage items.</skos:definition>
        <skos:definition xml:lang="el">Εργαλείο καθαρισμού, αποτελούμενο από μια λαβή πάνω στην οποία είναι στερεωμένα φτερά (π.χ. φτερά στρουθοκαμήλου). Χρησιμοποιείται στο πλαίσιο επεμβάσεων συντήρησης που αφορούν στον επιφανειακό καθαρισμό ή την απομάκρυνση χαλαρών επικαθίσεων (π.χ. σκόνης) από τις επιφάνειες κινητών αντικειμένων της Πολιτιστικής Κληρονομιάς.</skos:definition>
        <skos:prefLabel xml:lang="en">Feather duster</skos:prefLabel>
        <skos:prefLabel xml:lang="el">Φτερό ξεσκονίσματος</skos:prefLabel>
    </owl:NamedIndividual>
    


    <!-- http://w3id.org/dcri-ont/vocabulary/concept_00048 -->


    <owl:NamedIndividual rdf:about="http://w3id.org/dcri-ont/vocabulary/concept_00048">
        <rdf:type rdf:resource="http://www.w3.org/2004/02/skos/core#Concept"/>
        <skos:broader rdf:resource="http://w3id.org/dcri-ont/vocabulary/concept_00223"/>
        <skos:inScheme rdf:resource="http://w3id.org/dcri-ont/vocabulary/conceptscheme"/>
        <rdfs:label xml:lang="en">Swiffer duster</rdfs:label>
        <rdfs:label xml:lang="el">Πανί ξεσκονίσματος Swiffer</rdfs:label>
        <skos:prefLabel xml:lang="en">Swiffer duster</skos:prefLabel>
        <skos:prefLabel xml:lang="el">Πανί ξεσκονίσματος Swiffer</skos:prefLabel>
    </owl:NamedIndividual>
    


    <!-- http://w3id.org/dcri-ont/vocabulary/concept_00049 -->


    <owl:NamedIndividual rdf:about="http://w3id.org/dcri-ont/vocabulary/concept_00049">
        <rdf:type rdf:resource="http://www.w3.org/2004/02/skos/core#Concept"/>
        <skos:broader rdf:resource="http://w3id.org/dcri-ont/vocabulary/concept_00223"/>
        <skos:inScheme rdf:resource="http://w3id.org/dcri-ont/vocabulary/conceptscheme"/>
        <rdfs:comment xml:lang="en">Paper which absorb liquid substances.  It is used in the context of conservation interventions related to surface cleaning or removal of loose deposits (e.g. dust) from the surfaces of movable Cultural Heritage items. Particularly, it facilitates the application of some type of liquid cleanser and the removal of the undesireable deposits.</rdfs:comment>
        <rdfs:comment xml:lang="el">Χαρτί το οποίο απορροφά υλικά σε υγρή/ρευστή μορφή. Χρησιμοποιείται στο πλαίσιο επεμβάσεων συντήρησης που αφορούν στον επιφανειακό καθαρισμό ή την απομάκρυνση χαλαρών επικαθίσεων (π.χ. σκόνης) από τις επιφάνειες κινητών αντικειμένων της Πολιτιστικής Κληρονομιάς. Συγκεκριμένα, διευκολύνουν την εφαρμογή κάποιου υγρού καθαριστικού και την απομακρύνουν τις μη επιθυμητές επικαθίσεις.</rdfs:comment>
        <rdfs:label xml:lang="en">Absorbent paper</rdfs:label>
        <rdfs:label xml:lang="el">Απορροφητικό χαρτί</rdfs:label>
        <skos:definition xml:lang="en">Paper which absorb liquid substances.  It is used in the context of conservation interventions related to surface cleaning or removal of loose deposits (e.g. dust) from the surfaces of movable Cultural Heritage items. Particularly, it facilitates the application of some type of liquid cleanser and the removal of the undesireable deposits.</skos:definition>
        <skos:definition xml:lang="el">Χαρτί το οποίο απορροφά υλικά σε υγρή/ρευστή μορφή. Χρησιμοποιείται στο πλαίσιο επεμβάσεων συντήρησης που αφορούν στον επιφανειακό καθαρισμό ή την απομάκρυνση χαλαρών επικαθίσεων (π.χ. σκόνης) από τις επιφάνειες κινητών αντικειμένων της Πολιτιστικής Κληρονομιάς. Συγκεκριμένα, διευκολύνουν την εφαρμογή κάποιου υγρού καθαριστικού και την απομακρύνουν τις μη επιθυμητές επικαθίσεις.</skos:definition>
        <skos:prefLabel xml:lang="en">Absorbent paper</skos:prefLabel>
        <skos:prefLabel xml:lang="el">Απορροφητικό χαρτί</skos:prefLabel>
    </owl:NamedIndividual>
    


    <!-- http://w3id.org/dcri-ont/vocabulary/concept_00050 -->


    <owl:NamedIndividual rdf:about="http://w3id.org/dcri-ont/vocabulary/concept_00050">
        <rdf:type rdf:resource="http://www.w3.org/2004/02/skos/core#Concept"/>
        <skos:broader rdf:resource="http://w3id.org/dcri-ont/vocabulary/concept_00223"/>
        <skos:inScheme rdf:resource="http://w3id.org/dcri-ont/vocabulary/conceptscheme"/>
        <rdfs:comment xml:lang="en">Pieces of textile which is used for cleaning.  It is used in the context of conservation interventions related to surface cleaning or removal of loose deposits (e.g. dust) from the surfaces of movable Cultural Heritage items.</rdfs:comment>
        <rdfs:comment xml:lang="el">Τμήματα/κομάτια υφάσματος τα οποία χρησιμοποιούνται για καθάρισμα. Χρησιμοποιείται στο πλαίσιο επεμβάσεων συντήρησης που αφορούν στον επιφανειακό καθαρισμό ή την απομάκρυνση χαλαρών επικαθίσεων (π.χ. σκόνης) από τις επιφάνειες κινητών αντικειμένων της Πολιτιστικής Κληρονομιάς.</rdfs:comment>
        <rdfs:label xml:lang="en">Dust cloth</rdfs:label>
        <rdfs:label xml:lang="el">Ξεσκονόπανο</rdfs:label>
        <skos:altLabel xml:lang="en">Cloth for dusting</skos:altLabel>
        <skos:altLabel xml:lang="el">Πανί για ξεσκόνισμα</skos:altLabel>
        <skos:definition xml:lang="en">Pieces of textile which is used for cleaning.  It is used in the context of conservation interventions related to surface cleaning or removal of loose deposits (e.g. dust) from the surfaces of movable Cultural Heritage items.</skos:definition>
        <skos:definition xml:lang="el">Τμήματα/κομάτια υφάσματος τα οποία χρησιμοποιούνται για καθάρισμα. Χρησιμοποιείται στο πλαίσιο επεμβάσεων συντήρησης που αφορούν στον επιφανειακό καθαρισμό ή την απομάκρυνση χαλαρών επικαθίσεων (π.χ. σκόνης) από τις επιφάνειες κινητών αντικειμένων της Πολιτιστικής Κληρονομιάς.</skos:definition>
        <skos:prefLabel xml:lang="en">Dust cloth</skos:prefLabel>
        <skos:prefLabel xml:lang="el">Ξεσκονόπανο</skos:prefLabel>
    </owl:NamedIndividual>
    


    <!-- http://w3id.org/dcri-ont/vocabulary/concept_00051 -->


    <owl:NamedIndividual rdf:about="http://w3id.org/dcri-ont/vocabulary/concept_00051">
        <rdf:type rdf:resource="http://www.w3.org/2004/02/skos/core#Concept"/>
        <skos:broader rdf:resource="http://w3id.org/dcri-ont/vocabulary/concept_00223"/>
        <skos:inScheme rdf:resource="http://w3id.org/dcri-ont/vocabulary/conceptscheme"/>
        <rdfs:comment xml:lang="en">A tool used for cleaning, having a rubber bulblike piece which produces vacuum suction when squeezed. The bulb was an opening at one end and often a tube is adjusted on this opening. It is used in the context of conservation interventions related to surface cleaning or removal of loose deposits (e.g. dust) from the surfaces of movable Cultural Heritage items.</rdfs:comment>
        <rdfs:comment xml:lang="el">Εργαλείο καθαρισμού, αποτελούμενο από ένα λαστιχένιο κομμάτι που μοιάζει με βολβό το οποίο παράγει απορρόφηση κενού αέρος όταν πιεστεί. Το κομμάτι αυτό διαθέτει ένα άνοιγμα στην μια πλευρά του, στο οποίο προσαρμόζεται κάποιος σωλήνας. Χρησιμοποιείται στο πλαίσιο επεμβάσεων συντήρησης που αφορούν στον επιφανειακό καθαρισμό ή την απομάκρυνση χαλαρών επικαθίσεων (π.χ. σκόνης) από τις επιφάνειες κινητών αντικειμένων της Πολιτιστικής Κληρονομιάς.</rdfs:comment>
        <rdfs:label xml:lang="en">Dust bulb</rdfs:label>
        <rdfs:label xml:lang="el">Πουάρ</rdfs:label>
        <skos:altLabel xml:lang="en">Bulb duster</skos:altLabel>
        <skos:altLabel xml:lang="en">Rubber bulb</skos:altLabel>
        <skos:definition xml:lang="en">A tool used for cleaning, having a rubber bulblike piece which produces vacuum suction when squeezed. The bulb was an opening at one end and often a tube is adjusted on this opening. It is used in the context of conservation interventions related to surface cleaning or removal of loose deposits (e.g. dust) from the surfaces of movable Cultural Heritage items.</skos:definition>
        <skos:definition xml:lang="el">Εργαλείο καθαρισμού, αποτελούμενο από ένα λαστιχένιο κομμάτι που μοιάζει με βολβό το οποίο παράγει απορρόφηση κενού αέρος όταν πιεστεί. Το κομμάτι αυτό διαθέτει ένα άνοιγμα στην μια πλευρά του, στο οποίο προσαρμόζεται κάποιος σωλήνας. Χρησιμοποιείται στο πλαίσιο επεμβάσεων συντήρησης που αφορούν στον επιφανειακό καθαρισμό ή την απομάκρυνση χαλαρών επικαθίσεων (π.χ. σκόνης) από τις επιφάνειες κινητών αντικειμένων της Πολιτιστικής Κληρονομιάς.</skos:definition>
        <skos:prefLabel xml:lang="en">Dust bulb</skos:prefLabel>
        <skos:prefLabel xml:lang="el">Πουάρ</skos:prefLabel>
    </owl:NamedIndividual>
    


    <!-- http://w3id.org/dcri-ont/vocabulary/concept_00052 -->


    <owl:NamedIndividual rdf:about="http://w3id.org/dcri-ont/vocabulary/concept_00052">
        <rdf:type rdf:resource="http://www.w3.org/2004/02/skos/core#Concept"/>
        <skos:broader rdf:resource="http://w3id.org/dcri-ont/vocabulary/concept_00223"/>
        <skos:inScheme rdf:resource="http://w3id.org/dcri-ont/vocabulary/conceptscheme"/>
        <skos:narrower rdf:resource="http://w3id.org/dcri-ont/vocabulary/concept_00053"/>
        <rdfs:comment xml:lang="en">A tool used for cleaning, consisting of a handle onto which bristles are wound. It is used in the context of conservation interventions related to surface cleaning or removal of loose deposits (e.g. dust) from the surfaces of movable Cultural Heritage items.</rdfs:comment>
        <rdfs:comment xml:lang="el">Εργαλείο καθαρισμού, αποτελούμενο από μια λαβή πάνω στην οποία είναι στερεωμένες τρίχες. Χρησιμοποιείται στο πλαίσιο επεμβάσεων συντήρησης που αφορούν στον επιφανειακό καθαρισμό ή την απομάκρυνση χαλαρών επικαθίσεων (π.χ. σκόνης) από τις επιφάνειες κινητών αντικειμένων της Πολιτιστικής Κληρονομιάς.</rdfs:comment>
        <rdfs:label xml:lang="en">Dusting brush</rdfs:label>
        <rdfs:label xml:lang="el">Πινέλο ξεσκονίσματος</rdfs:label>
        <skos:definition xml:lang="en">A tool used for cleaning, consisting of a handle onto which bristles are wound. It is used in the context of conservation interventions related to surface cleaning or removal of loose deposits (e.g. dust) from the surfaces of movable Cultural Heritage items.</skos:definition>
        <skos:definition xml:lang="el">Εργαλείο καθαρισμού, αποτελούμενο από μια λαβή πάνω στην οποία είναι στερεωμένες τρίχες. Χρησιμοποιείται στο πλαίσιο επεμβάσεων συντήρησης που αφορούν στον επιφανειακό καθαρισμό ή την απομάκρυνση χαλαρών επικαθίσεων (π.χ. σκόνης) από τις επιφάνειες κινητών αντικειμένων της Πολιτιστικής Κληρονομιάς.</skos:definition>
        <skos:prefLabel xml:lang="en">Dusting brush</skos:prefLabel>
        <skos:prefLabel xml:lang="el">Πινέλο ξεσκονίσματος</skos:prefLabel>
    </owl:NamedIndividual>
    


    <!-- http://w3id.org/dcri-ont/vocabulary/concept_00053 -->


    <owl:NamedIndividual rdf:about="http://w3id.org/dcri-ont/vocabulary/concept_00053">
        <rdf:type rdf:resource="http://www.w3.org/2004/02/skos/core#Concept"/>
        <skos:broader rdf:resource="http://w3id.org/dcri-ont/vocabulary/concept_00052"/>
        <skos:inScheme rdf:resource="http://w3id.org/dcri-ont/vocabulary/conceptscheme"/>
        <rdfs:comment xml:lang="en">A dusting brush which has soft bristles.</rdfs:comment>
        <rdfs:comment xml:lang="el">Ένα πινέλο ξεσκονίσματος με μαλακές τρίχες.</rdfs:comment>
        <rdfs:label xml:lang="en">Soft dusting brush</rdfs:label>
        <rdfs:label xml:lang="el">Μαλακό πινέλο ξεσκονίσματος</rdfs:label>
        <skos:definition xml:lang="en">A dusting brush which has soft bristles.</skos:definition>
        <skos:definition xml:lang="el">Ένα πινέλο ξεσκονίσματος με μαλακές τρίχες.</skos:definition>
        <skos:prefLabel xml:lang="en">Soft dusting brush</skos:prefLabel>
        <skos:prefLabel xml:lang="el">Μαλακό πινέλο ξεσκονίσματος</skos:prefLabel>
    </owl:NamedIndividual>
    


    <!-- http://w3id.org/dcri-ont/vocabulary/concept_00054 -->


    <owl:NamedIndividual rdf:about="http://w3id.org/dcri-ont/vocabulary/concept_00054">
        <rdf:type rdf:resource="http://www.w3.org/2004/02/skos/core#Concept"/>
        <skos:broader rdf:resource="http://w3id.org/dcri-ont/vocabulary/concept_00054"/>
        <skos:inScheme rdf:resource="http://w3id.org/dcri-ont/vocabulary/conceptscheme"/>
        <skos:narrower rdf:resource="http://w3id.org/dcri-ont/vocabulary/concept_00055"/>
        <skos:narrower rdf:resource="http://w3id.org/dcri-ont/vocabulary/concept_00056"/>
        <skos:narrower rdf:resource="http://w3id.org/dcri-ont/vocabulary/concept_00057"/>
        <rdfs:comment xml:lang="en">Device which is used for cleaning by sunction. It is used in the context of conservation interventions related to surface cleaning or removal of loose deposits (e.g. dust) from the surfaces of movable Cultural Heritage items or sections of immovable Cultural Heritage.</rdfs:comment>
        <rdfs:comment xml:lang="el">Συσκευή καθαρισμού με απορρόφηση αέρα. Χρησιμοποιείται στο πλαίσιο επεμβάσεων συντήρησης που αφορούν στον επιφανειακό καθαρισμό ή την απομάκρυνση χαλαρών επικαθίσεων (π.χ. σκόνης) από τις επιφάνειες κινητών αντικειμένων της Πολιτιστικής Κληρονομιάς ή από τμήματα/μέρη της μη κινητής Πολιτιστικής Κληρονομιάς.</rdfs:comment>
        <rdfs:label xml:lang="en">Vacuum cleaner</rdfs:label>
        <rdfs:label xml:lang="el">Απορροφητική σκούπα</rdfs:label>
        <skos:definition xml:lang="en">Device which is used for cleaning by sunction. It is used in the context of conservation interventions related to surface cleaning or removal of loose deposits (e.g. dust) from the surfaces of movable Cultural Heritage items or sections of immovable Cultural Heritage.</skos:definition>
        <skos:definition xml:lang="el">Συσκευή καθαρισμού με απορρόφηση αέρα. Χρησιμοποιείται στο πλαίσιο επεμβάσεων συντήρησης που αφορούν στον επιφανειακό καθαρισμό ή την απομάκρυνση χαλαρών επικαθίσεων (π.χ. σκόνης) από τις επιφάνειες κινητών αντικειμένων της Πολιτιστικής Κληρονομιάς ή από τμήματα/μέρη της μη κινητής Πολιτιστικής Κληρονομιάς.</skos:definition>
        <skos:prefLabel xml:lang="en">Vacuum cleaner</skos:prefLabel>
        <skos:prefLabel xml:lang="el">Απορροφητική σκούπα</skos:prefLabel>
    </owl:NamedIndividual>
    


    <!-- http://w3id.org/dcri-ont/vocabulary/concept_00055 -->


    <owl:NamedIndividual rdf:about="http://w3id.org/dcri-ont/vocabulary/concept_00055">
        <rdf:type rdf:resource="http://www.w3.org/2004/02/skos/core#Concept"/>
        <skos:broader rdf:resource="http://w3id.org/dcri-ont/vocabulary/concept_00054"/>
        <skos:inScheme rdf:resource="http://w3id.org/dcri-ont/vocabulary/conceptscheme"/>
        <rdfs:comment xml:lang="en">An electric vacuum cleaner which can reach high volumes of sunction.</rdfs:comment>
        <rdfs:comment xml:lang="el">Ηλεκτρική απορροφητική σκούπα που μπορεί να πετύχει απορρόφηση υψηλών εντάσεων.</rdfs:comment>
        <rdfs:label xml:lang="en">Professional vacuum cleaner</rdfs:label>
        <rdfs:label xml:lang="el">Επαγγελματική απορροφητική σκούπα</rdfs:label>
        <skos:definition xml:lang="en">An electric vacuum cleaner which can reach high volumes of sunction.</skos:definition>
        <skos:definition xml:lang="el">Ηλεκτρική απορροφητική σκούπα που μπορεί να πετύχει απορρόφηση υψηλών εντάσεων.</skos:definition>
        <skos:prefLabel xml:lang="en">Professional vacuum cleaner</skos:prefLabel>
        <skos:prefLabel xml:lang="el">Επαγγελματική απορροφητική σκούπα</skos:prefLabel>
    </owl:NamedIndividual>
    


    <!-- http://w3id.org/dcri-ont/vocabulary/concept_00056 -->


    <owl:NamedIndividual rdf:about="http://w3id.org/dcri-ont/vocabulary/concept_00056">
        <rdf:type rdf:resource="http://www.w3.org/2004/02/skos/core#Concept"/>
        <skos:broader rdf:resource="http://w3id.org/dcri-ont/vocabulary/concept_00054"/>
        <skos:inScheme rdf:resource="http://w3id.org/dcri-ont/vocabulary/conceptscheme"/>
        <rdfs:comment xml:lang="en">An electric vacuum cleaner which can reach medium to very low volumes of sunction.</rdfs:comment>
        <rdfs:comment xml:lang="el">Ηλεκτρική απορροφητική σκούπα που μπορεί να πετύχει απορρόφηση μέτριων έως πολύ χαμηλών υψηλών εντάσεων.</rdfs:comment>
        <rdfs:label xml:lang="en">Museum vacuum cleaner</rdfs:label>
        <rdfs:label xml:lang="el">Απορροφητική σκούπα μουσείου</rdfs:label>
        <skos:definition xml:lang="en">An electric vacuum cleaner which can reach medium to very low volumes of sunction.</skos:definition>
        <skos:definition xml:lang="el">Ηλεκτρική απορροφητική σκούπα που μπορεί να πετύχει απορρόφηση μέτριων έως πολύ χαμηλών υψηλών εντάσεων.</skos:definition>
        <skos:prefLabel xml:lang="en">Museum vacuum cleaner</skos:prefLabel>
        <skos:prefLabel xml:lang="el">Απορροφητική σκούπα μουσείου</skos:prefLabel>
    </owl:NamedIndividual>
    


    <!-- http://w3id.org/dcri-ont/vocabulary/concept_00057 -->


    <owl:NamedIndividual rdf:about="http://w3id.org/dcri-ont/vocabulary/concept_00057">
        <rdf:type rdf:resource="http://www.w3.org/2004/02/skos/core#Concept"/>
        <skos:broader rdf:resource="http://w3id.org/dcri-ont/vocabulary/concept_00054"/>
        <skos:inScheme rdf:resource="http://w3id.org/dcri-ont/vocabulary/conceptscheme"/>
        <rdfs:label xml:lang="en">Battery vacuum cleaner</rdfs:label>
        <rdfs:label xml:lang="el">Απορροφητική σκούπα μπαταρίας</rdfs:label>
        <skos:prefLabel xml:lang="en">Battery vacuum cleaner</skos:prefLabel>
        <skos:prefLabel xml:lang="el">Απορροφητική σκούπα μπαταρίας</skos:prefLabel>
    </owl:NamedIndividual>
    


    <!-- http://w3id.org/dcri-ont/vocabulary/concept_00058 -->


    <owl:NamedIndividual rdf:about="http://w3id.org/dcri-ont/vocabulary/concept_00058">
        <rdf:type rdf:resource="http://www.w3.org/2004/02/skos/core#Concept"/>
        <skos:broader rdf:resource="http://w3id.org/dcri-ont/vocabulary/concept_00223"/>
        <skos:inScheme rdf:resource="http://w3id.org/dcri-ont/vocabulary/conceptscheme"/>
        <skos:narrower rdf:resource="http://w3id.org/dcri-ont/vocabulary/concept_00059"/>
        <skos:narrower rdf:resource="http://w3id.org/dcri-ont/vocabulary/concept_00060"/>
        <skos:narrower rdf:resource="http://w3id.org/dcri-ont/vocabulary/concept_00061"/>
        <rdfs:comment xml:lang="en">Device which is used for cleaning by blowing air. It is used in the context of conservation interventions related to surface cleaning or removal of loose deposits (e.g. dust) from the surfaces of movable Cultural Heritage items or sections of immovable Cultural Heritage.</rdfs:comment>
        <rdfs:comment xml:lang="el">Συσκευή καθαρισμού με εκτόξευση αέρα. Χρησιμοποιείται στο πλαίσιο επεμβάσεων συντήρησης που αφορούν στον επιφανειακό καθαρισμό ή την απομάκρυνση χαλαρών επικαθίσεων (π.χ. σκόνης) από τις επιφάνειες κινητών αντικειμένων της Πολιτιστικής Κληρονομιάς ή από τμήματα/μέρη της μη κινητής Πολιτιστικής Κληρονομιάς.</rdfs:comment>
        <rdfs:label xml:lang="en">Air blower</rdfs:label>
        <rdfs:label xml:lang="el">Φυσητήρας</rdfs:label>
        <skos:definition xml:lang="en">Device which is used for cleaning by blowing air. It is used in the context of conservation interventions related to surface cleaning or removal of loose deposits (e.g. dust) from the surfaces of movable Cultural Heritage items or sections of immovable Cultural Heritage.</skos:definition>
        <skos:definition xml:lang="el">Συσκευή καθαρισμού με εκτόξευση αέρα. Χρησιμοποιείται στο πλαίσιο επεμβάσεων συντήρησης που αφορούν στον επιφανειακό καθαρισμό ή την απομάκρυνση χαλαρών επικαθίσεων (π.χ. σκόνης) από τις επιφάνειες κινητών αντικειμένων της Πολιτιστικής Κληρονομιάς ή από τμήματα/μέρη της μη κινητής Πολιτιστικής Κληρονομιάς.</skos:definition>
        <skos:prefLabel xml:lang="en">Air blower</skos:prefLabel>
        <skos:prefLabel xml:lang="el">Φυσητήρας</skos:prefLabel>
    </owl:NamedIndividual>
    


    <!-- http://w3id.org/dcri-ont/vocabulary/concept_00059 -->


    <owl:NamedIndividual rdf:about="http://w3id.org/dcri-ont/vocabulary/concept_00059">
        <rdf:type rdf:resource="http://www.w3.org/2004/02/skos/core#Concept"/>
        <skos:broader rdf:resource="http://w3id.org/dcri-ont/vocabulary/concept_00058"/>
        <skos:inScheme rdf:resource="http://w3id.org/dcri-ont/vocabulary/conceptscheme"/>
        <rdfs:comment xml:lang="en">Air blower which can reach high volumes of air blowing. It usually used for leaf blowing in outdoor spaces and gardening. It also is used in the context of conservation interventions related to surface cleaning or removal of loose deposits (e.g. dust) from sections of immovable Cultural Heritage.</rdfs:comment>
        <rdfs:comment xml:lang="el">Φυσητήρας που μπορεί να πετύχει εκτόξευση αέρα υψηλών εντάσεων. Συνήθωας χρησιμοποιείται για το φύσιμα φύλλων σε εξωτερικού χώρους και την κηπουρική. Επίσης, χρησιμοποιείται στο πλαίσιο επεμβάσεων συντήρησης που αφορούν στον επιφανειακό καθαρισμό ή την απομάκρυνση χαλαρών επικαθίσεων (π.χ. σκόνης) από τμήματα/μέρη της μη κινητής Πολιτιστικής Κληρονομιάς.</rdfs:comment>
        <rdfs:label xml:lang="en">Leaf blower</rdfs:label>
        <rdfs:label xml:lang="el">Φυσητήρας φύλλων</rdfs:label>
        <skos:definition xml:lang="en">Air blower which can reach high volumes of air blowing. It usually used for leaf blowing in outdoor spaces and gardening. It also is used in the context of conservation interventions related to surface cleaning or removal of loose deposits (e.g. dust) from sections of immovable Cultural Heritage.</skos:definition>
        <skos:definition xml:lang="el">Φυσητήρας που μπορεί να πετύχει εκτόξευση αέρα υψηλών εντάσεων. Συνήθωας χρησιμοποιείται για το φύσιμα φύλλων σε εξωτερικού χώρους και την κηπουρική. Επίσης, χρησιμοποιείται στο πλαίσιο επεμβάσεων συντήρησης που αφορούν στον επιφανειακό καθαρισμό ή την απομάκρυνση χαλαρών επικαθίσεων (π.χ. σκόνης) από τμήματα/μέρη της μη κινητής Πολιτιστικής Κληρονομιάς.</skos:definition>
        <skos:prefLabel xml:lang="en">Leaf blower</skos:prefLabel>
        <skos:prefLabel xml:lang="el">Φυσητήρας φύλλων</skos:prefLabel>
    </owl:NamedIndividual>
    


    <!-- http://w3id.org/dcri-ont/vocabulary/concept_00060 -->


    <owl:NamedIndividual rdf:about="http://w3id.org/dcri-ont/vocabulary/concept_00060">
        <rdf:type rdf:resource="http://www.w3.org/2004/02/skos/core#Concept"/>
        <skos:broader rdf:resource="http://w3id.org/dcri-ont/vocabulary/concept_00058"/>
        <skos:inScheme rdf:resource="http://w3id.org/dcri-ont/vocabulary/conceptscheme"/>
        <rdfs:label xml:lang="en">Air blow gun</rdfs:label>
        <rdfs:label xml:lang="el">Πιστόλι εκτόξευσης αέρα</rdfs:label>
        <skos:prefLabel xml:lang="en">Air blow gun</skos:prefLabel>
        <skos:prefLabel xml:lang="el">Πιστόλι εκτόξευσης αέρα</skos:prefLabel>
    </owl:NamedIndividual>
    


    <!-- http://w3id.org/dcri-ont/vocabulary/concept_00061 -->


    <owl:NamedIndividual rdf:about="http://w3id.org/dcri-ont/vocabulary/concept_00061">
        <rdf:type rdf:resource="http://www.w3.org/2004/02/skos/core#Concept"/>
        <skos:broader rdf:resource="http://w3id.org/dcri-ont/vocabulary/concept_00058"/>
        <skos:inScheme rdf:resource="http://w3id.org/dcri-ont/vocabulary/conceptscheme"/>
        <rdfs:label xml:lang="en">Battery air blower</rdfs:label>
        <rdfs:label xml:lang="el">Φυσητήρας μπαταρίας</rdfs:label>
        <skos:prefLabel xml:lang="en">Battery air blower</skos:prefLabel>
        <skos:prefLabel xml:lang="el">Φυσητήρας μπαταρίας</skos:prefLabel>
    </owl:NamedIndividual>
    


    <!-- http://w3id.org/dcri-ont/vocabulary/concept_00062 -->


    <owl:NamedIndividual rdf:about="http://w3id.org/dcri-ont/vocabulary/concept_00062">
        <rdf:type rdf:resource="http://www.w3.org/2004/02/skos/core#Concept"/>
        <skos:broader rdf:resource="http://w3id.org/dcri-ont/vocabulary/concept_00158"/>
        <skos:inScheme rdf:resource="http://w3id.org/dcri-ont/vocabulary/conceptscheme"/>
        <rdfs:label xml:lang="en">Ethanol</rdfs:label>
        <rdfs:label xml:lang="el">Αιθανόλη</rdfs:label>
        <skos:altLabel xml:lang="el">Οινόπνευμα</skos:altLabel>
        <skos:prefLabel xml:lang="en">Ethanol</skos:prefLabel>
        <skos:prefLabel xml:lang="el">Αιθανόλη</skos:prefLabel>
    </owl:NamedIndividual>
    


    <!-- http://w3id.org/dcri-ont/vocabulary/concept_00063 -->


    <owl:NamedIndividual rdf:about="http://w3id.org/dcri-ont/vocabulary/concept_00063">
        <rdf:type rdf:resource="http://www.w3.org/2004/02/skos/core#Concept"/>
        <skos:broader rdf:resource="http://w3id.org/dcri-ont/vocabulary/concept_00158"/>
        <skos:inScheme rdf:resource="http://w3id.org/dcri-ont/vocabulary/conceptscheme"/>
        <rdfs:label xml:lang="en">Water</rdfs:label>
        <rdfs:label xml:lang="el">Νερό</rdfs:label>
        <skos:prefLabel xml:lang="en">Water</skos:prefLabel>
        <skos:prefLabel xml:lang="el">Νερό</skos:prefLabel>
    </owl:NamedIndividual>
    


    <!-- http://w3id.org/dcri-ont/vocabulary/concept_00064 -->


    <owl:NamedIndividual rdf:about="http://w3id.org/dcri-ont/vocabulary/concept_00064">
        <rdf:type rdf:resource="http://www.w3.org/2004/02/skos/core#Concept"/>
        <skos:inScheme rdf:resource="http://w3id.org/dcri-ont/vocabulary/conceptscheme"/>
        <skos:topConceptOf rdf:resource="http://w3id.org/dcri-ont/vocabulary/conceptscheme"/>
        <rdfs:label xml:lang="en">Window cleaner</rdfs:label>
        <rdfs:label xml:lang="el">Καθαριστικό τζαμιών</rdfs:label>
        <skos:altLabel xml:lang="en">Glass cleaner</skos:altLabel>
        <skos:prefLabel xml:lang="en">Window cleaner</skos:prefLabel>
        <skos:prefLabel xml:lang="el">Καθαριστικό τζαμιών</skos:prefLabel>
    </owl:NamedIndividual>
    


    <!-- http://w3id.org/dcri-ont/vocabulary/concept_00065 -->


    <owl:NamedIndividual rdf:about="http://w3id.org/dcri-ont/vocabulary/concept_00065">
        <rdf:type rdf:resource="http://www.w3.org/2004/02/skos/core#Concept"/>
        <skos:broader rdf:resource="http://w3id.org/dcri-ont/vocabulary/concept_00222"/>
        <skos:inScheme rdf:resource="http://w3id.org/dcri-ont/vocabulary/conceptscheme"/>
        <skos:narrower rdf:resource="http://w3id.org/dcri-ont/vocabulary/concept_00174"/>
        <skos:narrower rdf:resource="http://w3id.org/dcri-ont/vocabulary/concept_00175"/>
        <rdfs:comment xml:lang="en">Thin and dry sheets or webs of fiber formed and dried on a fine screen from a pulpy water suspension. The fibers may be animal (e.g., hair, silk or wool), mineral (e.g., asbestos), synthetic or cellulosic plant (e.g., wood pulp, grass, cotton, linen, and straw).</rdfs:comment>
        <rdfs:comment xml:lang="el">Λεπτά και ξηρά φύλλα ή πλέγματα ινών τα οποία έχουν σχηματιστεί από την ξήρανση εναιωρήματος πολτού και νερού πάνω σε λεπτή σίτα. Οι ίνες μπορεί να είναι ζωικές (π.χ., μαλλιά, μετάξι, μαλλί), ορυκτές (π.χ., άσβεστος), συνθετικές ή κυτταρινικών φυτών (π.χ., ξυλοπολτός, γρασίδι, βαμβάκι, λινό, άχυρο).</rdfs:comment>
        <rdfs:label xml:lang="en">Paper</rdfs:label>
        <rdfs:label xml:lang="el">Χαρτί</rdfs:label>
        <skos:definition xml:lang="en">Thin and dry sheets or webs of fiber formed and dried on a fine screen from a pulpy water suspension. The fibers may be animal (e.g., hair, silk or wool), mineral (e.g., asbestos), synthetic or cellulosic plant (e.g., wood pulp, grass, cotton, linen, and straw).</skos:definition>
        <skos:definition xml:lang="el">Λεπτά και ξηρά φύλλα ή πλέγματα ινών τα οποία έχουν σχηματιστεί από την ξήρανση εναιωρήματος πολτού και νερού πάνω σε λεπτή σίτα. Οι ίνες μπορεί να είναι ζωικές (π.χ., μαλλιά, μετάξι, μαλλί), ορυκτές (π.χ., άσβεστος), συνθετικές ή κυτταρινικών φυτών (π.χ., ξυλοπολτός, γρασίδι, βαμβάκι, λινό, άχυρο).</skos:definition>
        <skos:prefLabel xml:lang="en">Paper</skos:prefLabel>
        <skos:prefLabel xml:lang="el">Χαρτί</skos:prefLabel>
    </owl:NamedIndividual>
    


    <!-- http://w3id.org/dcri-ont/vocabulary/concept_00066 -->


    <owl:NamedIndividual rdf:about="http://w3id.org/dcri-ont/vocabulary/concept_00066">
        <rdf:type rdf:resource="http://www.w3.org/2004/02/skos/core#Concept"/>
        <skos:broader rdf:resource="http://w3id.org/dcri-ont/vocabulary/concept_00155"/>
        <skos:inScheme rdf:resource="http://w3id.org/dcri-ont/vocabulary/conceptscheme"/>
        <rdfs:comment xml:lang="en">A black, porous carbonaceous material comprising the carbon-containing residue from burned wood or other organic containing materials (e.g., bone, plants, animals).</rdfs:comment>
        <rdfs:comment xml:lang="el">Μαύρο πορώδες υλικό το οποίο περιλαμβάνει κατάλοιπα άνθρακα από καμμένο ξύλο ή άλλα οργανικά υλικά (π.χ., οστά, φυτά, ζώα).</rdfs:comment>
        <rdfs:label xml:lang="en">Charcoal</rdfs:label>
        <rdfs:label xml:lang="el">Κάρβουνο</rdfs:label>
        <skos:definition xml:lang="en">A black, porous carbonaceous material comprising the carbon-containing residue from burned wood or other organic containing materials (e.g., bone, plants, animals).</skos:definition>
        <skos:definition xml:lang="el">Μαύρο πορώδες υλικό το οποίο περιλαμβάνει κατάλοιπα άνθρακα από καμμένο ξύλο ή άλλα οργανικά υλικά (π.χ., οστά, φυτά, ζώα).</skos:definition>
        <skos:prefLabel xml:lang="en">Charcoal</skos:prefLabel>
        <skos:prefLabel xml:lang="el">Κάρβουνο</skos:prefLabel>
    </owl:NamedIndividual>
    


    <!-- http://w3id.org/dcri-ont/vocabulary/concept_00067 -->


    <owl:NamedIndividual rdf:about="http://w3id.org/dcri-ont/vocabulary/concept_00067">
        <rdf:type rdf:resource="http://www.w3.org/2004/02/skos/core#Concept"/>
        <skos:broader rdf:resource="http://w3id.org/dcri-ont/vocabulary/concept_00156"/>
        <skos:inScheme rdf:resource="http://w3id.org/dcri-ont/vocabulary/conceptscheme"/>
        <skos:narrower rdf:resource="http://w3id.org/dcri-ont/vocabulary/concept_00172"/>
        <skos:narrower rdf:resource="http://w3id.org/dcri-ont/vocabulary/concept_00176"/>
        <skos:narrower rdf:resource="http://w3id.org/dcri-ont/vocabulary/concept_00177"/>
        <skos:narrower rdf:resource="http://w3id.org/dcri-ont/vocabulary/concept_00178"/>
        <skos:narrower rdf:resource="http://w3id.org/dcri-ont/vocabulary/concept_00229"/>
        <rdfs:comment xml:lang="en">Any dispersion of pigment in a liquid binder. Paint is applied with a brush, roller, sprayer, or by dipping and dries to form a decorative or protective film.</rdfs:comment>
        <rdfs:comment xml:lang="el">Διεσπαρμένη χρωστική σε κάποιο ρευστό συνδετικό μέσο. Το χρώμα εφαρμόζεται με πινέλο, ρόλερ, σπρέυ ή τίναγμα και στεγνώνει ώστε να δημιουργήσει ένα διακοσμητικό ή προστατευτικό φίλμ.</rdfs:comment>
        <rdfs:label xml:lang="en">Paint</rdfs:label>
        <rdfs:label xml:lang="el">Χρώμα</rdfs:label>
        <skos:altLabel xml:lang="el">Μπογιά</skos:altLabel>
        <skos:definition xml:lang="en">Any dispersion of pigment in a liquid binder. Paint is applied with a brush, roller, sprayer, or by dipping and dries to form a decorative or protective film.</skos:definition>
        <skos:definition xml:lang="el">Διεσπαρμένη χρωστική σε κάποιο ρευστό συνδετικό μέσο. Το χρώμα εφαρμόζεται με πινέλο, ρόλερ, σπρέυ ή τίναγμα και στεγνώνει ώστε να δημιουργήσει ένα διακοσμητικό ή προστατευτικό φίλμ.</skos:definition>
        <skos:prefLabel xml:lang="en">Paint</skos:prefLabel>
        <skos:prefLabel xml:lang="el">Χρώμα</skos:prefLabel>
    </owl:NamedIndividual>
    


    <!-- http://w3id.org/dcri-ont/vocabulary/concept_00068 -->


    <owl:NamedIndividual rdf:about="http://w3id.org/dcri-ont/vocabulary/concept_00068">
        <rdf:type rdf:resource="http://www.w3.org/2004/02/skos/core#Concept"/>
        <skos:broader rdf:resource="http://w3id.org/dcri-ont/vocabulary/concept_00222"/>
        <skos:inScheme rdf:resource="http://w3id.org/dcri-ont/vocabulary/conceptscheme"/>
        <skos:narrower rdf:resource="http://w3id.org/dcri-ont/vocabulary/concept_00031"/>
        <rdfs:comment xml:lang="en">Materials produced by weaving, felting, knotting, twining, or otherwise processing natural or synthetic fibers so that they cohere into a form or unit.</rdfs:comment>
        <rdfs:comment xml:lang="el">Υλικά τα οποία έχουν προέλθει από ύφανση ή κάποια διαδικασία επεξεργασίας φυσικών ή συνθετικών ινών έτσι ώστε να έχουν μια ενιαία μορφή ή να αποτελούν μια μονάδα.</rdfs:comment>
        <rdfs:label xml:lang="en">Textile</rdfs:label>
        <rdfs:label xml:lang="el">Ύφασμα</rdfs:label>
        <skos:definition xml:lang="en">Materials produced by weaving, felting, knotting, twining, or otherwise processing natural or synthetic fibers so that they cohere into a form or unit.</skos:definition>
        <skos:definition xml:lang="el">Υλικά τα οποία έχουν προέλθει από ύφανση ή κάποια διαδικασία επεξεργασίας φυσικών ή συνθετικών ινών έτσι ώστε να έχουν μια ενιαία μορφή ή να αποτελούν μια μονάδα.</skos:definition>
        <skos:prefLabel xml:lang="en">Textile</skos:prefLabel>
        <skos:prefLabel xml:lang="el">Ύφασμα</skos:prefLabel>
    </owl:NamedIndividual>
    


    <!-- http://w3id.org/dcri-ont/vocabulary/concept_00069 -->


    <owl:NamedIndividual rdf:about="http://w3id.org/dcri-ont/vocabulary/concept_00069">
        <rdf:type rdf:resource="http://www.w3.org/2004/02/skos/core#Concept"/>
        <skos:broader rdf:resource="http://w3id.org/dcri-ont/vocabulary/concept_00222"/>
        <skos:inScheme rdf:resource="http://w3id.org/dcri-ont/vocabulary/conceptscheme"/>
        <skos:narrower rdf:resource="http://w3id.org/dcri-ont/vocabulary/concept_00180"/>
        <skos:narrower rdf:resource="http://w3id.org/dcri-ont/vocabulary/concept_00205"/>
        <skos:narrower rdf:resource="http://w3id.org/dcri-ont/vocabulary/concept_00206"/>
        <skos:narrower rdf:resource="http://w3id.org/dcri-ont/vocabulary/concept_00207"/>
        <rdfs:comment xml:lang="en">Natural or synthetic organic materials that can be molded, extruded, or cast when soft or liquid, and then set into a rigid or slightly elastic form. Natural plastics include tree resins, beeswax, gutta-percha, horn, and clay. Synthetic plastics were first made in the 19th century.</rdfs:comment>
        <rdfs:comment xml:lang="el">Φυσικά ή συνθετικά οργανικά υλικά που μπορούν να μορφοποιηθούν, να εξωθούνται ή να χυθούν όταν είναι μαλακά ή υγρά και στη συνέχεια να στερεοποιηθούν σε άκαμπτη ή ελαφρώς ελαστική μορφή. Τα φυσικά πλαστικά περιλαμβάνουν ρητίνες δέντρων, κερί μέλισσας, γουταπέρκα, κέρατο και πηλό. Τα συνθετικά πλαστικά κατασκευάστηκαν για πρώτη φορά τον 19ο αιώνα.</rdfs:comment>
        <rdfs:label xml:lang="en">Plastic</rdfs:label>
        <rdfs:label xml:lang="el">Πλαστικό</rdfs:label>
        <skos:definition xml:lang="en">Natural or synthetic organic materials that can be molded, extruded, or cast when soft or liquid, and then set into a rigid or slightly elastic form. Natural plastics include tree resins, beeswax, gutta-percha, horn, and clay. Synthetic plastics were first made in the 19th century.</skos:definition>
        <skos:definition xml:lang="el">Φυσικά ή συνθετικά οργανικά υλικά που μπορούν να μορφοποιηθούν, να εξωθούνται ή να χυθούν όταν είναι μαλακά ή υγρά και στη συνέχεια να στερεοποιηθούν σε άκαμπτη ή ελαφρώς ελαστική μορφή. Τα φυσικά πλαστικά περιλαμβάνουν ρητίνες δέντρων, κερί μέλισσας, γουταπέρκα, κέρατο και πηλό. Τα συνθετικά πλαστικά κατασκευάστηκαν για πρώτη φορά τον 19ο αιώνα.</skos:definition>
        <skos:prefLabel xml:lang="en">Plastic</skos:prefLabel>
        <skos:prefLabel xml:lang="el">Πλαστικό</skos:prefLabel>
    </owl:NamedIndividual>
    


    <!-- http://w3id.org/dcri-ont/vocabulary/concept_00070 -->


    <owl:NamedIndividual rdf:about="http://w3id.org/dcri-ont/vocabulary/concept_00070">
        <rdf:type rdf:resource="http://www.w3.org/2004/02/skos/core#Concept"/>
        <skos:broader rdf:resource="http://w3id.org/dcri-ont/vocabulary/concept_00222"/>
        <skos:inScheme rdf:resource="http://w3id.org/dcri-ont/vocabulary/conceptscheme"/>
        <rdfs:comment xml:lang="en">The principal tissue of trees and other plants that provides both strength and a means of conducting nutrients.</rdfs:comment>
        <rdfs:comment xml:lang="el">Ο βασικός ιστός των δέντρων και άλλων φυτών που παρέχει τόσο δύναμη όσο και ένα μέσο αγωγής θρεπτικών συστατικών.</rdfs:comment>
        <rdfs:label xml:lang="en">Wood</rdfs:label>
        <rdfs:label xml:lang="el">Ξύλο</rdfs:label>
        <skos:definition xml:lang="en">The principal tissue of trees and other plants that provides both strength and a means of conducting nutrients.</skos:definition>
        <skos:definition xml:lang="el">Ο βασικός ιστός των δέντρων και άλλων φυτών που παρέχει τόσο δύναμη όσο και ένα μέσο αγωγής θρεπτικών συστατικών.</skos:definition>
        <skos:prefLabel xml:lang="en">Wood</skos:prefLabel>
        <skos:prefLabel xml:lang="el">Ξύλο</skos:prefLabel>
    </owl:NamedIndividual>
    


    <!-- http://w3id.org/dcri-ont/vocabulary/concept_00071 -->


    <owl:NamedIndividual rdf:about="http://w3id.org/dcri-ont/vocabulary/concept_00071">
        <rdf:type rdf:resource="http://www.w3.org/2004/02/skos/core#Concept"/>
        <skos:broader rdf:resource="http://w3id.org/dcri-ont/vocabulary/concept_00155"/>
        <skos:inScheme rdf:resource="http://w3id.org/dcri-ont/vocabulary/conceptscheme"/>
        <rdfs:comment xml:lang="en">Naturally occurring crystalline form of carbon dimorphous with diamond. Graphite is opaque, soft, greasy to the touch, and iron black to steel gray in color; it occurs as crystals, flakes, scales, veins, bedded masses, or disseminations in metamorphic rocks.</rdfs:comment>
        <rdfs:comment xml:lang="el">Άνθρακας σε φυσική κρυσταλλική μορφή διαμορφωμένη με διαμάντι. Ο γραφίτης είναι αδιαφανής, απαλός, λιπαρός στην αφή και έχει χρώμα από μαύρο (σιδήρου) έως γκρί (ατσαλιού). Μπορεί να έχει την μορφή κρυστάλλων, νιφάδων, λεπιών, φλεβών, στρωμένες μάζες ή διασπορών σε μεταμορφωσιγενή πετρώματα.</rdfs:comment>
        <rdfs:label xml:lang="en">Graphite</rdfs:label>
        <rdfs:label xml:lang="el">Γραφίτης</rdfs:label>
        <skos:definition xml:lang="en">Naturally occurring crystalline form of carbon dimorphous with diamond. Graphite is opaque, soft, greasy to the touch, and iron black to steel gray in color; it occurs as crystals, flakes, scales, veins, bedded masses, or disseminations in metamorphic rocks.</skos:definition>
        <skos:definition xml:lang="el">Άνθρακας σε φυσική κρυσταλλική μορφή διαμορφωμένη με διαμάντι. Ο γραφίτης είναι αδιαφανής, απαλός, λιπαρός στην αφή και έχει χρώμα από μαύρο (σιδήρου) έως γκρί (ατσαλιού). Μπορεί να έχει την μορφή κρυστάλλων, νιφάδων, λεπιών, φλεβών, στρωμένες μάζες ή διασπορών σε μεταμορφωσιγενή πετρώματα.</skos:definition>
        <skos:prefLabel xml:lang="en">Graphite</skos:prefLabel>
        <skos:prefLabel xml:lang="el">Γραφίτης</skos:prefLabel>
    </owl:NamedIndividual>
    


    <!-- http://w3id.org/dcri-ont/vocabulary/concept_00072 -->


    <owl:NamedIndividual rdf:about="http://w3id.org/dcri-ont/vocabulary/concept_00072">
        <rdf:type rdf:resource="http://www.w3.org/2004/02/skos/core#Concept"/>
        <skos:broader rdf:resource="http://w3id.org/dcri-ont/vocabulary/concept_00155"/>
        <skos:inScheme rdf:resource="http://w3id.org/dcri-ont/vocabulary/conceptscheme"/>
        <rdfs:comment xml:lang="en">A fine-grained limestone, or soft, earthy form of calcium carbonate.</rdfs:comment>
        <rdfs:comment xml:lang="el">Ένας λεπτόκοκκος ασβεστόλιθος, ή μαλακή, γήινη μορφή ανθρακικού ασβεστίου.</rdfs:comment>
        <rdfs:label xml:lang="en">Chalk</rdfs:label>
        <rdfs:label xml:lang="el">Κιμωλία</rdfs:label>
        <skos:definition xml:lang="en">A fine-grained limestone, or soft, earthy form of calcium carbonate.</skos:definition>
        <skos:definition xml:lang="el">Ένας λεπτόκοκκος ασβεστόλιθος, ή μαλακή, γήινη μορφή ανθρακικού ασβεστίου.</skos:definition>
        <skos:prefLabel xml:lang="en">Chalk</skos:prefLabel>
        <skos:prefLabel xml:lang="el">Κιμωλία</skos:prefLabel>
    </owl:NamedIndividual>
    


    <!-- http://w3id.org/dcri-ont/vocabulary/concept_00073 -->


    <owl:NamedIndividual rdf:about="http://w3id.org/dcri-ont/vocabulary/concept_00073">
        <rdf:type rdf:resource="http://www.w3.org/2004/02/skos/core#Concept"/>
        <skos:broader rdf:resource="http://w3id.org/dcri-ont/vocabulary/concept_00155"/>
        <skos:inScheme rdf:resource="http://w3id.org/dcri-ont/vocabulary/conceptscheme"/>
        <rdfs:comment xml:lang="en">A fluid medium used for drawings or tracings. An opaque, usually black, pigment is mixed with a vehicle such as water to produce a fluid which can be applied with a pen or brush.</rdfs:comment>
        <rdfs:comment xml:lang="el">Ένα ρευστό μέσο που χρησιμοποιείται για σχέδια ή ιχνογραφίες. Μια αδιαφανής, συνήθως μαύρη, χρωστική ουσία αναμιγνύεται με ένα μέσο όπως το νερό για να παραχθεί ένα υγρό που μπορεί να εφαρμοστεί με στυλό ή βούρτσα.</rdfs:comment>
        <rdfs:label xml:lang="en">Ink</rdfs:label>
        <rdfs:label xml:lang="el">Μελάνι</rdfs:label>
        <skos:definition xml:lang="en">A fluid medium used for drawings or tracings. An opaque, usually black, pigment is mixed with a vehicle such as water to produce a fluid which can be applied with a pen or brush.</skos:definition>
        <skos:definition xml:lang="el">Ένα ρευστό μέσο που χρησιμοποιείται για σχέδια ή ιχνογραφίες. Μια αδιαφανής, συνήθως μαύρη, χρωστική ουσία αναμιγνύεται με ένα μέσο όπως το νερό για να παραχθεί ένα υγρό που μπορεί να εφαρμοστεί με στυλό ή βούρτσα.</skos:definition>
        <skos:prefLabel xml:lang="en">Ink</skos:prefLabel>
        <skos:prefLabel xml:lang="el">Μελάνι</skos:prefLabel>
    </owl:NamedIndividual>
    


    <!-- http://w3id.org/dcri-ont/vocabulary/concept_00074 -->


    <owl:NamedIndividual rdf:about="http://w3id.org/dcri-ont/vocabulary/concept_00074">
        <rdf:type rdf:resource="http://www.w3.org/2004/02/skos/core#Concept"/>
        <skos:broader rdf:resource="http://w3id.org/dcri-ont/vocabulary/concept_00155"/>
        <skos:broader rdf:resource="http://w3id.org/dcri-ont/vocabulary/concept_00156"/>
        <skos:inScheme rdf:resource="http://w3id.org/dcri-ont/vocabulary/conceptscheme"/>
        <rdfs:comment xml:lang="en">Combination of ground, powdery pigment and aqueous binder that are used in drawing and dry painting, delivered via a crayon or stick. Pastel as a material is soft and blendable.</rdfs:comment>
        <rdfs:comment xml:lang="el">Συνδυασμός αλεσμένης, κονιορτοποιημένης χρωστικής και υδατικού συνδετικού που χρησιμοποιούνται στο σχέδιο και στη ζωγραφική με ξηρά μέσα, τα οποία εφαρμόζονται μέσω ενός κραγιόν ή ραβδιού. Το παστέλ ως υλικό είναι μαλακό και αναμειγνύεται.</rdfs:comment>
        <rdfs:label xml:lang="en">Pastel</rdfs:label>
        <rdfs:label xml:lang="el">Παστέλ</rdfs:label>
        <skos:definition xml:lang="en">Combination of ground, powdery pigment and aqueous binder that are used in drawing and dry painting, delivered via a crayon or stick. Pastel as a material is soft and blendable.</skos:definition>
        <skos:definition xml:lang="el">Συνδυασμός αλεσμένης, κονιορτοποιημένης χρωστικής και υδατικού συνδετικού που χρησιμοποιούνται στο σχέδιο και στη ζωγραφική με ξηρά μέσα, τα οποία εφαρμόζονται μέσω ενός κραγιόν ή ραβδιού. Το παστέλ ως υλικό είναι μαλακό και αναμειγνύεται.</skos:definition>
        <skos:prefLabel xml:lang="en">Pastel</skos:prefLabel>
        <skos:prefLabel xml:lang="el">Παστέλ</skos:prefLabel>
    </owl:NamedIndividual>
    


    <!-- http://w3id.org/dcri-ont/vocabulary/concept_00075 -->


    <owl:NamedIndividual rdf:about="http://w3id.org/dcri-ont/vocabulary/concept_00075">
        <rdf:type rdf:resource="http://www.w3.org/2004/02/skos/core#Concept"/>
        <skos:broader rdf:resource="http://w3id.org/dcri-ont/vocabulary/concept_00227"/>
        <skos:inScheme rdf:resource="http://w3id.org/dcri-ont/vocabulary/conceptscheme"/>
        <skos:narrower rdf:resource="http://w3id.org/dcri-ont/vocabulary/concept_00076"/>
        <skos:narrower rdf:resource="http://w3id.org/dcri-ont/vocabulary/concept_00077"/>
        <skos:narrower rdf:resource="http://w3id.org/dcri-ont/vocabulary/concept_00078"/>
        <skos:narrower rdf:resource="http://w3id.org/dcri-ont/vocabulary/concept_00079"/>
        <skos:narrower rdf:resource="http://w3id.org/dcri-ont/vocabulary/concept_00080"/>
        <skos:narrower rdf:resource="http://w3id.org/dcri-ont/vocabulary/concept_00081"/>
        <skos:narrower rdf:resource="http://w3id.org/dcri-ont/vocabulary/concept_00082"/>
        <skos:narrower rdf:resource="http://w3id.org/dcri-ont/vocabulary/concept_00086"/>
        <rdfs:comment xml:lang="en">A mass or layer of matter of varying thickness that has subsided or been precipitated from a fluid medium onto another mass of material, or has collected in one place by any natural process. The bond of the superficial deposit to the surface is loose.</rdfs:comment>
        <rdfs:comment xml:lang="el">Μάζα ή στρώμα ύλης ποικίλου πάχους που έχει καθιζάνει ή καταβυθιστεί από ένα ρευστό μέσο σε μια άλλη μάζα υλικού ή έχει συγκεντρωθεί σε ένα μέρος με οποιαδήποτε φυσική διαδικασία. Οι δυνάμεις που συγκρατούν την επιφανειακή επικάθιση στην επιφάνεια είναι χαλαρές.</rdfs:comment>
        <rdfs:label xml:lang="en">Superficial deposit</rdfs:label>
        <rdfs:label xml:lang="el">Επιφανειακή επικάθιση</rdfs:label>
        <skos:altLabel xml:lang="en">Loose deposit</skos:altLabel>
        <skos:altLabel xml:lang="en">Superficial accretion</skos:altLabel>
        <skos:definition xml:lang="en">A mass or layer of matter of varying thickness that has subsided or been precipitated from a fluid medium onto another mass of material, or has collected in one place by any natural process. The bond of the superficial deposit to the surface is loose.</skos:definition>
        <skos:definition xml:lang="el">Μάζα ή στρώμα ύλης ποικίλου πάχους που έχει καθιζάνει ή καταβυθιστεί από ένα ρευστό μέσο σε μια άλλη μάζα υλικού ή έχει συγκεντρωθεί σε ένα μέρος με οποιαδήποτε φυσική διαδικασία. Οι δυνάμεις που συγκρατούν την επιφανειακή επικάθιση στην επιφάνεια είναι χαλαρές.</skos:definition>
        <skos:prefLabel xml:lang="en">Superficial deposit</skos:prefLabel>
        <skos:prefLabel xml:lang="el">Επιφανειακή επικάθιση</skos:prefLabel>
    </owl:NamedIndividual>
    


    <!-- http://w3id.org/dcri-ont/vocabulary/concept_00076 -->


    <owl:NamedIndividual rdf:about="http://w3id.org/dcri-ont/vocabulary/concept_00076">
        <rdf:type rdf:resource="http://www.w3.org/2004/02/skos/core#Concept"/>
        <skos:broader rdf:resource="http://w3id.org/dcri-ont/vocabulary/concept_00075"/>
        <skos:inScheme rdf:resource="http://w3id.org/dcri-ont/vocabulary/conceptscheme"/>
        <rdfs:comment xml:lang="en">Superficial deposit of unconsolidated material on the earth&apos;s surface formed by the weathering of rock.</rdfs:comment>
        <rdfs:comment xml:lang="el">Επιφανειακή επικάθιση από μη σταθεροποιημένο υλικό στην επιφάνεια της γης που σχηματίζεται από τη διάβρωση του λίθου.</rdfs:comment>
        <rdfs:label xml:lang="en">Soil (superficial deposit)</rdfs:label>
        <rdfs:label xml:lang="el">Χώμα (επιφανειακή επικάθιση)</rdfs:label>
        <skos:definition xml:lang="en">Superficial deposit of unconsolidated material on the earth&apos;s surface formed by the weathering of rock.</skos:definition>
        <skos:definition xml:lang="el">Επιφανειακή επικάθιση από μη σταθεροποιημένο υλικό στην επιφάνεια της γης που σχηματίζεται από τη διάβρωση του λίθου.</skos:definition>
        <skos:prefLabel xml:lang="en">Soil (superficial deposit)</skos:prefLabel>
        <skos:prefLabel xml:lang="el">Χώμα (επιφανειακή επικάθιση)</skos:prefLabel>
    </owl:NamedIndividual>
    


    <!-- http://w3id.org/dcri-ont/vocabulary/concept_00077 -->


    <owl:NamedIndividual rdf:about="http://w3id.org/dcri-ont/vocabulary/concept_00077">
        <rdf:type rdf:resource="http://www.w3.org/2004/02/skos/core#Concept"/>
        <skos:broader rdf:resource="http://w3id.org/dcri-ont/vocabulary/concept_00075"/>
        <skos:inScheme rdf:resource="http://w3id.org/dcri-ont/vocabulary/conceptscheme"/>
        <rdfs:comment xml:lang="en">Waste matter discharged from the insects.</rdfs:comment>
        <rdfs:comment xml:lang="el">Απόβλητες ουσίες που αποβάλλονται από έντομα.</rdfs:comment>
        <rdfs:label xml:lang="en">Insect excrement</rdfs:label>
        <rdfs:label xml:lang="el">Απεκκρίματα εντόμων</rdfs:label>
        <skos:altLabel xml:lang="en">Insect dropping</skos:altLabel>
        <skos:definition xml:lang="en">Waste matter discharged from the insects.</skos:definition>
        <skos:definition xml:lang="el">Απόβλητες ουσίες που αποβάλλονται από έντομα.</skos:definition>
        <skos:prefLabel xml:lang="en">Insect excrement</skos:prefLabel>
        <skos:prefLabel xml:lang="el">Απεκκρίματα εντόμων</skos:prefLabel>
    </owl:NamedIndividual>
    


    <!-- http://w3id.org/dcri-ont/vocabulary/concept_00078 -->


    <owl:NamedIndividual rdf:about="http://w3id.org/dcri-ont/vocabulary/concept_00078">
        <rdf:type rdf:resource="http://www.w3.org/2004/02/skos/core#Concept"/>
        <skos:broader rdf:resource="http://w3id.org/dcri-ont/vocabulary/concept_00075"/>
        <skos:inScheme rdf:resource="http://w3id.org/dcri-ont/vocabulary/conceptscheme"/>
        <rdfs:comment xml:lang="en">Webs that are spun by spiders, made of spider silk as interlaced threads of viscous protein fluid that solidify on exposure to air.</rdfs:comment>
        <rdfs:comment xml:lang="el">Ιστοί που υφαίνονται από αράχνες, κατασκευασμένοι από μετάξι αράχνης ως συμπλεγμένα νήματα ιξώδους πρωτεϊνικού υγρού που στερεοποιούνται κατά την έκθεση στον αέρα.</rdfs:comment>
        <rdfs:label xml:lang="en">Spider web</rdfs:label>
        <rdfs:label xml:lang="el">Ιστός αράχνης</rdfs:label>
        <skos:definition xml:lang="en">Webs that are spun by spiders, made of spider silk as interlaced threads of viscous protein fluid that solidify on exposure to air.</skos:definition>
        <skos:definition xml:lang="el">Ιστοί που υφαίνονται από αράχνες, κατασκευασμένοι από μετάξι αράχνης ως συμπλεγμένα νήματα ιξώδους πρωτεϊνικού υγρού που στερεοποιούνται κατά την έκθεση στον αέρα.</skos:definition>
        <skos:prefLabel xml:lang="en">Spider web</skos:prefLabel>
        <skos:prefLabel xml:lang="el">Ιστός αράχνης</skos:prefLabel>
    </owl:NamedIndividual>
    


    <!-- http://w3id.org/dcri-ont/vocabulary/concept_00079 -->


    <owl:NamedIndividual rdf:about="http://w3id.org/dcri-ont/vocabulary/concept_00079">
        <rdf:type rdf:resource="http://www.w3.org/2004/02/skos/core#Concept"/>
        <skos:broader rdf:resource="http://w3id.org/dcri-ont/vocabulary/concept_00075"/>
        <skos:inScheme rdf:resource="http://w3id.org/dcri-ont/vocabulary/conceptscheme"/>
        <rdfs:comment xml:lang="en">Various fungi that produce a conspicuous, furry mass of mycelium (masses of vegetative filaments, or hyphae) and fruiting structures, particularly those of the genera Aspergillus, Penicillium, and Rhizopus, which are associated with food spoilage, plant diseases, and damage to artifacts.</rdfs:comment>
        <rdfs:comment xml:lang="el">Ποικίλοι μύκητες οι οποίοι παράγουν μια διακριτή, τριχωειδή μάζα μυκηλίου (μάζες φυτικών νημάτων ή υφών) και καρποφόρων δομών, ιδίως εκείνων των γενών Aspergillus, Penicillium και Rhizopus, που σχετίζονται με αλλοίωση τροφίμων, ασθένειες των φυτών και βλάβες σε τεχνουργήματα.</rdfs:comment>
        <rdfs:label xml:lang="en">Mold</rdfs:label>
        <rdfs:label xml:lang="el">Μούχλα</rdfs:label>
        <skos:definition xml:lang="en">Various fungi that produce a conspicuous, furry mass of mycelium (masses of vegetative filaments, or hyphae) and fruiting structures, particularly those of the genera Aspergillus, Penicillium, and Rhizopus, which are associated with food spoilage, plant diseases, and damage to artifacts.</skos:definition>
        <skos:definition xml:lang="el">Ποικίλοι μύκητες οι οποίοι παράγουν μια διακριτή, τριχωειδή μάζα μυκηλίου (μάζες φυτικών νημάτων ή υφών) και καρποφόρων δομών, ιδίως εκείνων των γενών Aspergillus, Penicillium και Rhizopus, που σχετίζονται με αλλοίωση τροφίμων, ασθένειες των φυτών και βλάβες σε τεχνουργήματα.</skos:definition>
        <skos:prefLabel xml:lang="en">Mold</skos:prefLabel>
        <skos:prefLabel xml:lang="el">Μούχλα</skos:prefLabel>
    </owl:NamedIndividual>
    


    <!-- http://w3id.org/dcri-ont/vocabulary/concept_00080 -->


    <owl:NamedIndividual rdf:about="http://w3id.org/dcri-ont/vocabulary/concept_00080">
        <rdf:type rdf:resource="http://www.w3.org/2004/02/skos/core#Concept"/>
        <skos:broader rdf:resource="http://w3id.org/dcri-ont/vocabulary/concept_00075"/>
        <skos:inScheme rdf:resource="http://w3id.org/dcri-ont/vocabulary/conceptscheme"/>
        <rdfs:comment xml:lang="en">Fine, dry particles of matter regarded as the result of disintegration. Dust may be accumulated on surfaces.</rdfs:comment>
        <rdfs:comment xml:lang="el">Λεπτά, ξηρά σωματίδια ύλης τα οποία θεωρούνται αποτέλεσμα αποσύνθεσης. Η σκόνη μπορεί να συσσωρεύεται σε επιφάνειες.</rdfs:comment>
        <rdfs:label xml:lang="en">Dust</rdfs:label>
        <rdfs:label xml:lang="el">Σκόνη</rdfs:label>
        <skos:definition xml:lang="en">Fine, dry particles of matter regarded as the result of disintegration. Dust may be accumulated on surfaces.</skos:definition>
        <skos:definition xml:lang="el">Λεπτά, ξηρά σωματίδια ύλης τα οποία θεωρούνται αποτέλεσμα αποσύνθεσης. Η σκόνη μπορεί να συσσωρεύεται σε επιφάνειες.</skos:definition>
        <skos:prefLabel xml:lang="en">Dust</skos:prefLabel>
        <skos:prefLabel xml:lang="el">Σκόνη</skos:prefLabel>
    </owl:NamedIndividual>
    


    <!-- http://w3id.org/dcri-ont/vocabulary/concept_00081 -->


    <owl:NamedIndividual rdf:about="http://w3id.org/dcri-ont/vocabulary/concept_00081">
        <rdf:type rdf:resource="http://www.w3.org/2004/02/skos/core#Concept"/>
        <skos:broader rdf:resource="http://w3id.org/dcri-ont/vocabulary/concept_00075"/>
        <skos:inScheme rdf:resource="http://w3id.org/dcri-ont/vocabulary/conceptscheme"/>
        <rdfs:comment xml:lang="en">Fine particles of erasers which have been left on a surface forming deposits.</rdfs:comment>
        <rdfs:comment xml:lang="el">Μικρά κομμάτια γόμας τα οποία έχουν παραμείνει σε μια επιφάνεια σχηματίζοντας επικαθίσεις.</rdfs:comment>
        <rdfs:label xml:lang="en">Eraser crumbs (residue)</rdfs:label>
        <rdfs:label xml:lang="el">Τρίμματα γόμας (υπολείμματα)</rdfs:label>
        <skos:definition xml:lang="en">Fine particles of erasers which have been left on a surface forming deposits.</skos:definition>
        <skos:definition xml:lang="el">Μικρά κομμάτια γόμας τα οποία έχουν παραμείνει σε μια επιφάνεια σχηματίζοντας επικαθίσεις.</skos:definition>
        <skos:prefLabel xml:lang="en">Eraser crumbs (residue)</skos:prefLabel>
        <skos:prefLabel xml:lang="el">Τρίμματα γόμας (υπολείμματα)</skos:prefLabel>
    </owl:NamedIndividual>
    


    <!-- http://w3id.org/dcri-ont/vocabulary/concept_00082 -->


    <owl:NamedIndividual rdf:about="http://w3id.org/dcri-ont/vocabulary/concept_00082">
        <rdf:type rdf:resource="http://www.w3.org/2004/02/skos/core#Concept"/>
        <skos:broader rdf:resource="http://w3id.org/dcri-ont/vocabulary/concept_00075"/>
        <skos:inScheme rdf:resource="http://w3id.org/dcri-ont/vocabulary/conceptscheme"/>
        <rdfs:label xml:lang="en">Glass fragments</rdfs:label>
        <rdfs:label xml:lang="el">Κομμάτια γυαλιού</rdfs:label>
        <skos:prefLabel xml:lang="en">Glass fragments</skos:prefLabel>
        <skos:prefLabel xml:lang="el">Κομμάτια γυαλιού</skos:prefLabel>
    </owl:NamedIndividual>
    


    <!-- http://w3id.org/dcri-ont/vocabulary/concept_00083 -->


    <owl:NamedIndividual rdf:about="http://w3id.org/dcri-ont/vocabulary/concept_00083">
        <rdf:type rdf:resource="http://www.w3.org/2004/02/skos/core#Concept"/>
        <skos:broader rdf:resource="http://w3id.org/dcri-ont/vocabulary/concept_00227"/>
        <skos:inScheme rdf:resource="http://w3id.org/dcri-ont/vocabulary/conceptscheme"/>
        <rdfs:comment xml:lang="en">The quality of being easily crumbled or reduced to a powder.</rdfs:comment>
        <rdfs:comment xml:lang="el">Η ιδιότητα του να θριμματίζεται κάτι εύκολα ή να γίνεται σκόνη.</rdfs:comment>
        <rdfs:label xml:lang="en">Friability</rdfs:label>
        <rdfs:label xml:lang="el">Ευθρυπτότητα</rdfs:label>
        <skos:altLabel xml:lang="en">Brittle</skos:altLabel>
        <skos:definition xml:lang="en">The quality of being easily crumbled or reduced to a powder.</skos:definition>
        <skos:definition xml:lang="el">Η ιδιότητα του να θριμματίζεται κάτι εύκολα ή να γίνεται σκόνη.</skos:definition>
        <skos:prefLabel xml:lang="en">Friability</skos:prefLabel>
        <skos:prefLabel xml:lang="el">Ευθρυπτότητα</skos:prefLabel>
    </owl:NamedIndividual>
    


    <!-- http://w3id.org/dcri-ont/vocabulary/concept_00084 -->


    <owl:NamedIndividual rdf:about="http://w3id.org/dcri-ont/vocabulary/concept_00084">
        <rdf:type rdf:resource="http://www.w3.org/2004/02/skos/core#Concept"/>
        <skos:broader rdf:resource="http://w3id.org/dcri-ont/vocabulary/concept_00227"/>
        <skos:inScheme rdf:resource="http://w3id.org/dcri-ont/vocabulary/conceptscheme"/>
        <rdfs:comment xml:lang="en">The quality of being easily broken, shattered, or damaged.</rdfs:comment>
        <rdfs:comment xml:lang="el">Η ιδιότητα του να σπάει, να κομματιάζεται ή να χαλάει κάτι εύκολα.</rdfs:comment>
        <rdfs:label xml:lang="en">Fragility</rdfs:label>
        <rdfs:label xml:lang="el">Ευθραυστότητα</rdfs:label>
        <skos:definition xml:lang="en">The quality of being easily broken, shattered, or damaged.</skos:definition>
        <skos:definition xml:lang="el">Η ιδιότητα του να σπάει, να κομματιάζεται ή να χαλάει κάτι εύκολα.</skos:definition>
        <skos:prefLabel xml:lang="en">Fragility</skos:prefLabel>
        <skos:prefLabel xml:lang="el">Ευθραυστότητα</skos:prefLabel>
    </owl:NamedIndividual>
    


    <!-- http://w3id.org/dcri-ont/vocabulary/concept_00085 -->


    <owl:NamedIndividual rdf:about="http://w3id.org/dcri-ont/vocabulary/concept_00085">
        <rdf:type rdf:resource="http://www.w3.org/2004/02/skos/core#Concept"/>
        <skos:broader rdf:resource="http://w3id.org/dcri-ont/vocabulary/concept_00227"/>
        <skos:inScheme rdf:resource="http://w3id.org/dcri-ont/vocabulary/conceptscheme"/>
        <rdfs:comment xml:lang="en">The quality or state of lacking stability, of tending toward changeability, or of readily decomposing or changing chemically.</rdfs:comment>
        <rdfs:comment xml:lang="el">Η ιδιότητα ή κατάσταση της έλλειψης σταθερότητας, της τάσης για αλλαγή ή της εύκολης αποσύνθεσης ή χημικής αλλαγής.</rdfs:comment>
        <rdfs:label xml:lang="en">Instability</rdfs:label>
        <rdfs:label xml:lang="el">Αστάθεια</rdfs:label>
        <skos:definition xml:lang="en">The quality or state of lacking stability, of tending toward changeability, or of readily decomposing or changing chemically.</skos:definition>
        <skos:definition xml:lang="el">Η ιδιότητα ή κατάσταση της έλλειψης σταθερότητας, της τάσης για αλλαγή ή της εύκολης αποσύνθεσης ή χημικής αλλαγής.</skos:definition>
        <skos:prefLabel xml:lang="en">Instability</skos:prefLabel>
        <skos:prefLabel xml:lang="el">Αστάθεια</skos:prefLabel>
    </owl:NamedIndividual>
    


    <!-- http://w3id.org/dcri-ont/vocabulary/concept_00086 -->


    <owl:NamedIndividual rdf:about="http://w3id.org/dcri-ont/vocabulary/concept_00086">
        <rdf:type rdf:resource="http://www.w3.org/2004/02/skos/core#Concept"/>
        <skos:broader rdf:resource="http://w3id.org/dcri-ont/vocabulary/concept_00075"/>
        <skos:inScheme rdf:resource="http://w3id.org/dcri-ont/vocabulary/conceptscheme"/>
        <rdfs:comment xml:lang="en">Solid particulate matter sitting on the surface of an object.</rdfs:comment>
        <rdfs:comment xml:lang="el">Στερεά σωματίδια που επικάθονται στην επιφάνεια ενός αντικειμένου.</rdfs:comment>
        <rdfs:label xml:lang="en">Soiling (loose bonding)</rdfs:label>
        <rdfs:label xml:lang="el">Βρωμιά (χαλαρός δεσμός)</rdfs:label>
        <skos:altLabel xml:lang="en">Dirt (loose bonding)</skos:altLabel>
        <skos:definition xml:lang="en">Solid particulate matter sitting on the surface of an object.</skos:definition>
        <skos:definition xml:lang="el">Στερεά σωματίδια που επικάθονται στην επιφάνεια ενός αντικειμένου.</skos:definition>
        <skos:prefLabel xml:lang="en">Soiling (loose bonding)</skos:prefLabel>
        <skos:prefLabel xml:lang="el">Βρωμιά (χαλαρός δεσμός)</skos:prefLabel>
    </owl:NamedIndividual>
    


    <!-- http://w3id.org/dcri-ont/vocabulary/concept_00087 -->


    <owl:NamedIndividual rdf:about="http://w3id.org/dcri-ont/vocabulary/concept_00087">
        <rdf:type rdf:resource="http://www.w3.org/2004/02/skos/core#Concept"/>
        <skos:broader rdf:resource="http://w3id.org/dcri-ont/vocabulary/concept_00227"/>
        <skos:inScheme rdf:resource="http://w3id.org/dcri-ont/vocabulary/conceptscheme"/>
        <rdfs:comment xml:lang="en">Separating into thin flattened pieces or layers.</rdfs:comment>
        <rdfs:comment xml:lang="el">Διαχωρισμός σε λεπτά ίσια κομμάτια ή στρώματα.</rdfs:comment>
        <rdfs:label xml:lang="en">Flaking</rdfs:label>
        <rdfs:label xml:lang="el">Απολέπιση</rdfs:label>
        <skos:definition xml:lang="en">Separating into thin flattened pieces or layers.</skos:definition>
        <skos:definition xml:lang="el">Διαχωρισμός σε λεπτά ίσια κομμάτια ή στρώματα.</skos:definition>
        <skos:prefLabel xml:lang="en">Flaking</skos:prefLabel>
        <skos:prefLabel xml:lang="el">Απολέπιση</skos:prefLabel>
    </owl:NamedIndividual>
    


    <!-- http://w3id.org/dcri-ont/vocabulary/concept_00088 -->


    <owl:NamedIndividual rdf:about="http://w3id.org/dcri-ont/vocabulary/concept_00088">
        <rdf:type rdf:resource="http://www.w3.org/2004/02/skos/core#Concept"/>
        <skos:broader rdf:resource="http://w3id.org/dcri-ont/vocabulary/concept_00227"/>
        <skos:inScheme rdf:resource="http://w3id.org/dcri-ont/vocabulary/conceptscheme"/>
        <rdfs:comment xml:lang="en">The act or process of reducing to powder, pulverization; in conservation science context refers to granular disintegration of stone and pigments.</rdfs:comment>
        <rdfs:comment xml:lang="el">Η πράξη ή η διαδικασία αναγωγής σε σκόνη, κονιορτοποίηση. Στο πλαίσιο της επιστήμης της διατήρησης αναφέρεται στην αποδόμηση σε κόκκους της πέτρας και των χρωστικών.</rdfs:comment>
        <rdfs:label xml:lang="en">Powdering</rdfs:label>
        <rdfs:label xml:lang="el">Κονιορτοποίηση</rdfs:label>
        <skos:altLabel xml:lang="en">Pulverization</skos:altLabel>
        <skos:definition xml:lang="en">The act or process of reducing to powder, pulverization; in conservation science context refers to granular disintegration of stone and pigments.</skos:definition>
        <skos:definition xml:lang="el">Η πράξη ή η διαδικασία αναγωγής σε σκόνη, κονιορτοποίηση. Στο πλαίσιο της επιστήμης της διατήρησης αναφέρεται στην αποδόμηση σε κόκκους της πέτρας και των χρωστικών.</skos:definition>
        <skos:prefLabel xml:lang="en">Powdering</skos:prefLabel>
        <skos:prefLabel xml:lang="el">Κονιορτοποίηση</skos:prefLabel>
    </owl:NamedIndividual>
    


    <!-- http://w3id.org/dcri-ont/vocabulary/concept_00089 -->


    <owl:NamedIndividual rdf:about="http://w3id.org/dcri-ont/vocabulary/concept_00089">
        <rdfs:label xml:lang="en">Chalking</rdfs:label>
        <skos:prefLabel xml:lang="en">Chalking</skos:prefLabel>
    </owl:NamedIndividual>
    


    <!-- http://w3id.org/dcri-ont/vocabulary/concept_00090 -->


    <owl:NamedIndividual rdf:about="http://w3id.org/dcri-ont/vocabulary/concept_00090">
        <rdf:type rdf:resource="http://www.w3.org/2004/02/skos/core#Concept"/>
        <skos:broader rdf:resource="http://w3id.org/dcri-ont/vocabulary/concept_00227"/>
        <skos:inScheme rdf:resource="http://w3id.org/dcri-ont/vocabulary/conceptscheme"/>
        <rdfs:comment xml:lang="en">A mass or layer of matter of varying thickness that has subsided or been precipitated from a fluid medium onto another mass of material, or has collected in one place by any natural process. The bond of the ingrained deposit to the surface is firm.</rdfs:comment>
        <rdfs:comment xml:lang="el">Μάζα ή στρώμα ύλης ποικίλου πάχους που έχει καθιζάνει ή καταβυθιστεί από ένα ρευστό μέσο σε μια άλλη μάζα υλικού ή έχει συγκεντρωθεί σε ένα μέρος με οποιαδήποτε φυσική διαδικασία. Οι δυνάμεις που συγκρατούν την εμποτισμένη επικάθιση στην επιφάνεια είναι ισχυρές.</rdfs:comment>
        <rdfs:label xml:lang="en">Ingrained deposit</rdfs:label>
        <rdfs:label xml:lang="el">Εμποτισμένη επικάθιση</rdfs:label>
        <skos:definition xml:lang="en">A mass or layer of matter of varying thickness that has subsided or been precipitated from a fluid medium onto another mass of material, or has collected in one place by any natural process. The bond of the ingrained deposit to the surface is firm.</skos:definition>
        <skos:definition xml:lang="el">Μάζα ή στρώμα ύλης ποικίλου πάχους που έχει καθιζάνει ή καταβυθιστεί από ένα ρευστό μέσο σε μια άλλη μάζα υλικού ή έχει συγκεντρωθεί σε ένα μέρος με οποιαδήποτε φυσική διαδικασία. Οι δυνάμεις που συγκρατούν την εμποτισμένη επικάθιση στην επιφάνεια είναι ισχυρές.</skos:definition>
        <skos:prefLabel xml:lang="en">Ingrained deposit</skos:prefLabel>
        <skos:prefLabel xml:lang="el">Εμποτισμένη επικάθιση</skos:prefLabel>
    </owl:NamedIndividual>
    


    <!-- http://w3id.org/dcri-ont/vocabulary/concept_00091 -->


    <owl:NamedIndividual rdf:about="http://w3id.org/dcri-ont/vocabulary/concept_00091">
        <rdf:type rdf:resource="http://www.w3.org/2004/02/skos/core#Concept"/>
        <skos:broader rdf:resource="http://w3id.org/dcri-ont/vocabulary/concept_00227"/>
        <skos:inScheme rdf:resource="http://w3id.org/dcri-ont/vocabulary/conceptscheme"/>
        <rdfs:comment xml:lang="en">The quality of having a surface diversified with small projections, points, and irregularities so as to be harsh or uneven to the sight or touch.</rdfs:comment>
        <rdfs:comment xml:lang="el">Η ιδιότητα μιας επιφάνειας να έχει διαφοροποιήσεις με μικρές προεξοχές, σημεία και ανωμαλίες έτσι ώστε να είναι σκηρή ή ανώμαλη στην όψη και την υφή.</rdfs:comment>
        <rdfs:label xml:lang="en">Roughness</rdfs:label>
        <rdfs:label xml:lang="el">Τραχύτητα</rdfs:label>
        <skos:definition xml:lang="en">The quality of having a surface diversified with small projections, points, and irregularities so as to be harsh or uneven to the sight or touch.</skos:definition>
        <skos:definition xml:lang="el">Η ιδιότητα μιας επιφάνειας να έχει διαφοροποιήσεις με μικρές προεξοχές, σημεία και ανωμαλίες έτσι ώστε να είναι σκηρή ή ανώμαλη στην όψη και την υφή.</skos:definition>
        <skos:prefLabel xml:lang="en">Roughness</skos:prefLabel>
        <skos:prefLabel xml:lang="el">Τραχύτητα</skos:prefLabel>
    </owl:NamedIndividual>
    


    <!-- http://w3id.org/dcri-ont/vocabulary/concept_00092 -->


    <owl:NamedIndividual rdf:about="http://w3id.org/dcri-ont/vocabulary/concept_00092">
        <rdf:type rdf:resource="http://www.w3.org/2004/02/skos/core#Concept"/>
        <skos:broader rdf:resource="http://w3id.org/dcri-ont/vocabulary/concept_00227"/>
        <skos:inScheme rdf:resource="http://w3id.org/dcri-ont/vocabulary/conceptscheme"/>
        <rdfs:comment xml:lang="en">The quality of a surface to stick.</rdfs:comment>
        <rdfs:comment xml:lang="el">Η ιδιότητα μιας επιφάνειας να κολλάει.</rdfs:comment>
        <rdfs:label xml:lang="en">Stickiness</rdfs:label>
        <rdfs:label xml:lang="el">Κολλώδες</rdfs:label>
        <skos:definition xml:lang="en">The quality of a surface to stick.</skos:definition>
        <skos:definition xml:lang="el">Η ιδιότητα μιας επιφάνειας να κολλάει.</skos:definition>
        <skos:prefLabel xml:lang="en">Stickiness</skos:prefLabel>
        <skos:prefLabel xml:lang="el">Κολλώδες</skos:prefLabel>
    </owl:NamedIndividual>
    


    <!-- http://w3id.org/dcri-ont/vocabulary/concept_00149 -->


    <owl:NamedIndividual rdf:about="http://w3id.org/dcri-ont/vocabulary/concept_00149">
        <rdf:type rdf:resource="http://www.w3.org/2004/02/skos/core#Concept"/>
        <skos:broader rdf:resource="http://w3id.org/dcri-ont/vocabulary/concept_00226"/>
        <skos:inScheme rdf:resource="http://w3id.org/dcri-ont/vocabulary/conceptscheme"/>
        <rdfs:label xml:lang="en">Celsius scale</rdfs:label>
        <rdfs:label xml:lang="el">Κλίμακα Κελσίου</rdfs:label>
        <skos:prefLabel xml:lang="en">Celsius scale</skos:prefLabel>
        <skos:prefLabel xml:lang="el">Κλίμακα Κελσίου</skos:prefLabel>
    </owl:NamedIndividual>
    


    <!-- http://w3id.org/dcri-ont/vocabulary/concept_00150 -->


    <owl:NamedIndividual rdf:about="http://w3id.org/dcri-ont/vocabulary/concept_00150">
        <rdf:type rdf:resource="http://www.w3.org/2004/02/skos/core#Concept"/>
        <skos:broader rdf:resource="http://w3id.org/dcri-ont/vocabulary/concept_00226"/>
        <skos:inScheme rdf:resource="http://w3id.org/dcri-ont/vocabulary/conceptscheme"/>
        <rdfs:label xml:lang="en">pH scale</rdfs:label>
        <rdfs:label xml:lang="el">Κλίμακα pH</rdfs:label>
        <skos:prefLabel xml:lang="en">pH scale</skos:prefLabel>
        <skos:prefLabel xml:lang="el">Κλίμακα pH</skos:prefLabel>
    </owl:NamedIndividual>
    


    <!-- http://w3id.org/dcri-ont/vocabulary/concept_00154 -->


    <owl:NamedIndividual rdf:about="http://w3id.org/dcri-ont/vocabulary/concept_00154">
        <rdf:type rdf:resource="http://www.w3.org/2004/02/skos/core#Concept"/>
        <skos:broader rdf:resource="http://w3id.org/dcri-ont/vocabulary/concept_00222"/>
        <skos:inScheme rdf:resource="http://w3id.org/dcri-ont/vocabulary/conceptscheme"/>
        <rdfs:comment xml:lang="en">Substances that typically show a characteristic luster, are good conductors of electricity and heat, are opaque, can be fused, and are usually malleable or ductile.</rdfs:comment>
        <rdfs:comment xml:lang="el">Ουσίες που παρουσιάζουν μια χαρακτηριστική γυαλάδα, είναι καλοί αγωγοί ηλεκτρισμού και θερμότητας, είναι αδιαφανείς, μπορούν να λιωθούν, και είναι συνήθως εύπλαστες ή όλκιμες.</rdfs:comment>
        <rdfs:label xml:lang="en">Metal</rdfs:label>
        <rdfs:label xml:lang="el">Μέταλλο</rdfs:label>
        <skos:definition xml:lang="en">Substances that typically show a characteristic luster, are good conductors of electricity and heat, are opaque, can be fused, and are usually malleable or ductile.</skos:definition>
        <skos:definition xml:lang="el">Ουσίες που παρουσιάζουν μια χαρακτηριστική γυαλάδα, είναι καλοί αγωγοί ηλεκτρισμού και θερμότητας, είναι αδιαφανείς, μπορούν να λιωθούν, και είναι συνήθως εύπλαστες ή όλκιμες.</skos:definition>
        <skos:prefLabel xml:lang="en">Metal</skos:prefLabel>
        <skos:prefLabel xml:lang="el">Μέταλλο</skos:prefLabel>
    </owl:NamedIndividual>
    


    <!-- http://w3id.org/dcri-ont/vocabulary/concept_00155 -->


    <owl:NamedIndividual rdf:about="http://w3id.org/dcri-ont/vocabulary/concept_00155">
        <rdf:type rdf:resource="http://www.w3.org/2004/02/skos/core#Concept"/>
        <skos:broader rdf:resource="http://w3id.org/dcri-ont/vocabulary/concept_00222"/>
        <skos:inScheme rdf:resource="http://w3id.org/dcri-ont/vocabulary/conceptscheme"/>
        <skos:narrower rdf:resource="http://w3id.org/dcri-ont/vocabulary/concept_00066"/>
        <skos:narrower rdf:resource="http://w3id.org/dcri-ont/vocabulary/concept_00071"/>
        <skos:narrower rdf:resource="http://w3id.org/dcri-ont/vocabulary/concept_00072"/>
        <skos:narrower rdf:resource="http://w3id.org/dcri-ont/vocabulary/concept_00073"/>
        <skos:narrower rdf:resource="http://w3id.org/dcri-ont/vocabulary/concept_00074"/>
        <skos:narrower rdf:resource="http://w3id.org/dcri-ont/vocabulary/concept_00187"/>
        <skos:narrower rdf:resource="http://w3id.org/dcri-ont/vocabulary/concept_00188"/>
        <skos:narrower rdf:resource="http://w3id.org/dcri-ont/vocabulary/concept_00201"/>
        <rdfs:comment xml:lang="en">Materials used for the production of a design on a support.</rdfs:comment>
        <rdfs:comment xml:lang="el">Τα υλικά μέσα τα οποία χρησιμοποιούνται για την δημιουργία ενός σχεδίου σε ένα υποστήριγμα.</rdfs:comment>
        <rdfs:label xml:lang="en">Design media</rdfs:label>
        <rdfs:label xml:lang="el">Μέσα σχεδίου</rdfs:label>
        <skos:altLabel xml:lang="en">Drawing media</skos:altLabel>
        <skos:definition xml:lang="en">Materials used for the production of a design on a support.</skos:definition>
        <skos:definition xml:lang="el">Τα υλικά μέσα τα οποία χρησιμοποιούνται για την δημιουργία ενός σχεδίου σε ένα υποστήριγμα.</skos:definition>
        <skos:prefLabel xml:lang="en">Design media</skos:prefLabel>
        <skos:prefLabel xml:lang="el">Μέσα σχεδίου</skos:prefLabel>
    </owl:NamedIndividual>
    


    <!-- http://w3id.org/dcri-ont/vocabulary/concept_00156 -->


    <owl:NamedIndividual rdf:about="http://w3id.org/dcri-ont/vocabulary/concept_00156">
        <rdf:type rdf:resource="http://www.w3.org/2004/02/skos/core#Concept"/>
        <skos:broader rdf:resource="http://w3id.org/dcri-ont/vocabulary/concept_00222"/>
        <skos:inScheme rdf:resource="http://w3id.org/dcri-ont/vocabulary/conceptscheme"/>
        <skos:narrower rdf:resource="http://w3id.org/dcri-ont/vocabulary/concept_00067"/>
        <skos:narrower rdf:resource="http://w3id.org/dcri-ont/vocabulary/concept_00074"/>
        <rdfs:comment xml:lang="en">Materials used for the production of a painting on a support.</rdfs:comment>
        <rdfs:comment xml:lang="el">Τα υλικά μέσα τα οποία χρησιμοποιούνται για την ζωγραφική σε ένα υποστήριγμα.</rdfs:comment>
        <rdfs:label xml:lang="en">Painting media</rdfs:label>
        <rdfs:label xml:lang="el">Μέσα ζωγραφικής</rdfs:label>
        <skos:definition xml:lang="en">Materials used for the production of a painting on a support.</skos:definition>
        <skos:definition xml:lang="el">Τα υλικά μέσα τα οποία χρησιμοποιούνται για την ζωγραφική σε ένα υποστήριγμα.</skos:definition>
        <skos:prefLabel xml:lang="en">Painting media</skos:prefLabel>
        <skos:prefLabel xml:lang="el">Μέσα ζωγραφικής</skos:prefLabel>
    </owl:NamedIndividual>
    


    <!-- http://w3id.org/dcri-ont/vocabulary/concept_00157 -->


    <owl:NamedIndividual rdf:about="http://w3id.org/dcri-ont/vocabulary/concept_00157">
        <rdf:type rdf:resource="http://www.w3.org/2004/02/skos/core#Concept"/>
        <skos:broader rdf:resource="http://w3id.org/dcri-ont/vocabulary/concept_00226"/>
        <skos:inScheme rdf:resource="http://w3id.org/dcri-ont/vocabulary/conceptscheme"/>
        <rdfs:label xml:lang="en">Centimetre</rdfs:label>
        <rdfs:label xml:lang="el">Εκατοστά</rdfs:label>
        <skos:prefLabel xml:lang="en">Centimetre</skos:prefLabel>
        <skos:prefLabel xml:lang="el">Εκατοστά</skos:prefLabel>
    </owl:NamedIndividual>
    


    <!-- http://w3id.org/dcri-ont/vocabulary/concept_00158 -->


    <owl:NamedIndividual rdf:about="http://w3id.org/dcri-ont/vocabulary/concept_00158">
        <rdf:type rdf:resource="http://www.w3.org/2004/02/skos/core#Concept"/>
        <skos:broader rdf:resource="http://w3id.org/dcri-ont/vocabulary/concept_00222"/>
        <skos:inScheme rdf:resource="http://w3id.org/dcri-ont/vocabulary/conceptscheme"/>
        <skos:narrower rdf:resource="http://w3id.org/dcri-ont/vocabulary/concept_00062"/>
        <skos:narrower rdf:resource="http://w3id.org/dcri-ont/vocabulary/concept_00063"/>
        <skos:narrower rdf:resource="http://w3id.org/dcri-ont/vocabulary/concept_00168"/>
        <rdfs:comment xml:lang="en">Any material, usually liquid, having the power of dissolving another material.</rdfs:comment>
        <rdfs:comment xml:lang="el">Οποιοδήποτε υλικό, συνήθως ρευστό, το οποίο έχει την ικανότητα να διαλύσει ένα άλλο υλικό.</rdfs:comment>
        <rdfs:label xml:lang="en">Solvent</rdfs:label>
        <rdfs:label xml:lang="el">Διαλύτης</rdfs:label>
        <skos:definition xml:lang="en">Any material, usually liquid, having the power of dissolving another material.</skos:definition>
        <skos:definition xml:lang="el">Οποιοδήποτε υλικό, συνήθως ρευστό, το οποίο έχει την ικανότητα να διαλύσει ένα άλλο υλικό.</skos:definition>
        <skos:prefLabel xml:lang="en">Solvent</skos:prefLabel>
        <skos:prefLabel xml:lang="el">Διαλύτης</skos:prefLabel>
    </owl:NamedIndividual>
    


    <!-- http://w3id.org/dcri-ont/vocabulary/concept_00159 -->


    <owl:NamedIndividual rdf:about="http://w3id.org/dcri-ont/vocabulary/concept_00159">
        <rdf:type rdf:resource="http://www.w3.org/2004/02/skos/core#Concept"/>
        <skos:broader rdf:resource="http://w3id.org/dcri-ont/vocabulary/concept_00222"/>
        <skos:inScheme rdf:resource="http://w3id.org/dcri-ont/vocabulary/conceptscheme"/>
        <rdfs:comment xml:lang="en">Combination of two or more substances in no definite proportions, within which the constituent substances retain their individual properties and are separable by ordinary physical means. </rdfs:comment>
        <rdfs:comment xml:lang="el">Συνδυασμός δύο ή περισσότερων ουσιών σε μη καθορισμένες ποσότηττες, μέσα στον οποίο οι ουσίες διατηρούν τις ιδιότητές τους και μπορούν να διαχωριστούν με φυσικού τρόπους.</rdfs:comment>
        <rdfs:label xml:lang="en">Mixture</rdfs:label>
        <rdfs:label xml:lang="el">Μίγμα</rdfs:label>
        <skos:definition xml:lang="en">Combination of two or more substances in no definite proportions, within which the constituent substances retain their individual properties and are separable by ordinary physical means. </skos:definition>
        <skos:definition xml:lang="el">Συνδυασμός δύο ή περισσότερων ουσιών σε μη καθορισμένες ποσότηττες, μέσα στον οποίο οι ουσίες διατηρούν τις ιδιότητές τους και μπορούν να διαχωριστούν με φυσικού τρόπους.</skos:definition>
        <skos:prefLabel xml:lang="en">Mixture</skos:prefLabel>
        <skos:prefLabel xml:lang="el">Μίγμα</skos:prefLabel>
    </owl:NamedIndividual>
    


    <!-- http://w3id.org/dcri-ont/vocabulary/concept_00160 -->


    <owl:NamedIndividual rdf:about="http://w3id.org/dcri-ont/vocabulary/concept_00160">
        <rdf:type rdf:resource="http://www.w3.org/2004/02/skos/core#Concept"/>
        <skos:broader rdf:resource="http://w3id.org/dcri-ont/vocabulary/concept_00222"/>
        <skos:inScheme rdf:resource="http://w3id.org/dcri-ont/vocabulary/conceptscheme"/>
        <skos:narrower rdf:resource="http://w3id.org/dcri-ont/vocabulary/concept_00169"/>
        <skos:narrower rdf:resource="http://w3id.org/dcri-ont/vocabulary/concept_00254"/>
        <rdfs:comment xml:lang="en">Any substance introduced into a deteriorated surface where it strengthens and stabilizes the surface, making it solid, or compact.</rdfs:comment>
        <rdfs:comment xml:lang="el">Οποιαδήποτε ουσία που εισάγεται σε μια διαβρωμένη επιφάνεια η οποία ενδυναμώνει και σταθεροποιεί την επιφάνεια, καθιστώντας την σταθερή ή συμπαγής.</rdfs:comment>
        <rdfs:label xml:lang="en">Consolidant</rdfs:label>
        <rdfs:label xml:lang="el">Συγκολλητικό</rdfs:label>
        <skos:definition xml:lang="en">Any substance introduced into a deteriorated surface where it strengthens and stabilizes the surface, making it solid, or compact.</skos:definition>
        <skos:definition xml:lang="el">Οποιαδήποτε ουσία που εισάγεται σε μια διαβρωμένη επιφάνεια η οποία ενδυναμώνει και σταθεροποιεί την επιφάνεια, καθιστώντας την σταθερή ή συμπαγής.</skos:definition>
        <skos:prefLabel xml:lang="en">Consolidant</skos:prefLabel>
        <skos:prefLabel xml:lang="el">Συγκολλητικό</skos:prefLabel>
    </owl:NamedIndividual>
    


    <!-- http://w3id.org/dcri-ont/vocabulary/concept_00161 -->


    <owl:NamedIndividual rdf:about="http://w3id.org/dcri-ont/vocabulary/concept_00161">
        <rdf:type rdf:resource="http://www.w3.org/2004/02/skos/core#Concept"/>
        <skos:broader rdf:resource="http://w3id.org/dcri-ont/vocabulary/concept_00228"/>
        <skos:inScheme rdf:resource="http://w3id.org/dcri-ont/vocabulary/conceptscheme"/>
        <rdfs:label xml:lang="en">Width</rdfs:label>
        <rdfs:label xml:lang="el">Πλάτος</rdfs:label>
        <skos:prefLabel xml:lang="en">Width</skos:prefLabel>
        <skos:prefLabel xml:lang="el">Πλάτος</skos:prefLabel>
    </owl:NamedIndividual>
    


    <!-- http://w3id.org/dcri-ont/vocabulary/concept_00162 -->


    <owl:NamedIndividual rdf:about="http://w3id.org/dcri-ont/vocabulary/concept_00162">
        <rdf:type rdf:resource="http://www.w3.org/2004/02/skos/core#Concept"/>
        <skos:broader rdf:resource="http://w3id.org/dcri-ont/vocabulary/concept_00228"/>
        <skos:inScheme rdf:resource="http://w3id.org/dcri-ont/vocabulary/conceptscheme"/>
        <rdfs:label xml:lang="en">Depth</rdfs:label>
        <rdfs:label xml:lang="el">Βάθος</rdfs:label>
        <skos:prefLabel xml:lang="en">Depth</skos:prefLabel>
        <skos:prefLabel xml:lang="el">Βάθος</skos:prefLabel>
    </owl:NamedIndividual>
    


    <!-- http://w3id.org/dcri-ont/vocabulary/concept_00163 -->


    <owl:NamedIndividual rdf:about="http://w3id.org/dcri-ont/vocabulary/concept_00163">
        <rdf:type rdf:resource="http://www.w3.org/2004/02/skos/core#Concept"/>
        <skos:broader rdf:resource="http://w3id.org/dcri-ont/vocabulary/concept_00228"/>
        <skos:inScheme rdf:resource="http://w3id.org/dcri-ont/vocabulary/conceptscheme"/>
        <rdfs:label xml:lang="en">Height</rdfs:label>
        <rdfs:label xml:lang="el">Ύψος</rdfs:label>
        <skos:prefLabel xml:lang="en">Height</skos:prefLabel>
        <skos:prefLabel xml:lang="el">Ύψος</skos:prefLabel>
    </owl:NamedIndividual>
    


    <!-- http://w3id.org/dcri-ont/vocabulary/concept_00164 -->


    <owl:NamedIndividual rdf:about="http://w3id.org/dcri-ont/vocabulary/concept_00164">
        <rdf:type rdf:resource="http://www.w3.org/2004/02/skos/core#Concept"/>
        <skos:broader rdf:resource="http://w3id.org/dcri-ont/vocabulary/concept_00223"/>
        <skos:inScheme rdf:resource="http://w3id.org/dcri-ont/vocabulary/conceptscheme"/>
        <rdfs:comment xml:lang="en">A device used for misting of consolidants. It is created from a modified ultrasonic humidifier. It was first developed by Canadian Conservation Institute.</rdfs:comment>
        <rdfs:comment xml:lang="el">Συσκευή που χρησιμοποιείται για τον ψεκασμό συγκολλητικών υλικών. Έχει δημιουργηθεί με την τροποποίηση ενός υγραντήρα υπερήχων. Δημιουργήθηκε πρώτη φορά από το Canadian Conservation Institute.</rdfs:comment>
        <rdfs:label xml:lang="en">Ultrasonic mister</rdfs:label>
        <rdfs:label xml:lang="el">Ψεκαστήρας με υπερήχους</rdfs:label>
        <skos:definition xml:lang="en">A device used for misting of consolidants. It is created from a modified ultrasonic humidifier. It was first developed by Canadian Conservation Institute.</skos:definition>
        <skos:definition xml:lang="el">Συσκευή που χρησιμοποιείται για τον ψεκασμό συγκολλητικών υλικών. Έχει δημιουργηθεί με την τροποποίηση ενός υγραντήρα υπερήχων. Δημιουργήθηκε πρώτη φορά από το Canadian Conservation Institute.</skos:definition>
        <skos:prefLabel xml:lang="en">Ultrasonic mister</skos:prefLabel>
        <skos:prefLabel xml:lang="el">Ψεκαστήρας με υπερήχους</skos:prefLabel>
    </owl:NamedIndividual>
    


    <!-- http://w3id.org/dcri-ont/vocabulary/concept_00165 -->


    <owl:NamedIndividual rdf:about="http://w3id.org/dcri-ont/vocabulary/concept_00165">
        <rdf:type rdf:resource="http://www.w3.org/2004/02/skos/core#Concept"/>
        <skos:broader rdf:resource="http://w3id.org/dcri-ont/vocabulary/concept_00223"/>
        <skos:inScheme rdf:resource="http://w3id.org/dcri-ont/vocabulary/conceptscheme"/>
        <rdfs:comment xml:lang="en">A tool consisting of a handle onto which bristles are wound. The bristles form a round-tapered shape. It is usually used in the context of conservation interventions related to consolidation of structular layers of movable or immovable Cultural Heritage (painting layers, substartes etc).</rdfs:comment>
        <rdfs:comment xml:lang="el">Εργαλείο το οποίο αποτελείται από μια λαβή πάνω στην οποία είναι στερεωμένες τρίχες. Οι τρίχες σχηματίζουν ένα στρογγυλό-κωνικό σχήμα. Χρησιμοποιείται συνήθως στο πλαίσιο επεμβάσεων συντήρησης σχετικές με την στερέωση δομικών στρωμάτων κινητών ή μη κινητών αντικειμένων Πολιτιστικής Κληρονομιάς (ζωγραφικά στρώματα, υπόστρωμα έργων τέχνης κ.ά.).</rdfs:comment>
        <rdfs:label xml:lang="en">Round brush</rdfs:label>
        <rdfs:label xml:lang="el">Στρογγυλό πινέλο</rdfs:label>
        <skos:definition xml:lang="en">A tool consisting of a handle onto which bristles are wound. The bristles form a round-tapered shape. It is usually used in the context of conservation interventions related to consolidation of structular layers of movable or immovable Cultural Heritage (painting layers, substartes etc).</skos:definition>
        <skos:definition xml:lang="el">Εργαλείο το οποίο αποτελείται από μια λαβή πάνω στην οποία είναι στερεωμένες τρίχες. Οι τρίχες σχηματίζουν ένα στρογγυλό-κωνικό σχήμα. Χρησιμοποιείται συνήθως στο πλαίσιο επεμβάσεων συντήρησης σχετικές με την στερέωση δομικών στρωμάτων κινητών ή μη κινητών αντικειμένων Πολιτιστικής Κληρονομιάς (ζωγραφικά στρώματα, υπόστρωμα έργων τέχνης κ.ά.).</skos:definition>
        <skos:prefLabel xml:lang="en">Round brush</skos:prefLabel>
        <skos:prefLabel xml:lang="el">Στρογγυλό πινέλο</skos:prefLabel>
    </owl:NamedIndividual>
    


    <!-- http://w3id.org/dcri-ont/vocabulary/concept_00166 -->


    <owl:NamedIndividual rdf:about="http://w3id.org/dcri-ont/vocabulary/concept_00166">
        <rdf:type rdf:resource="http://www.w3.org/2004/02/skos/core#Concept"/>
        <skos:broader rdf:resource="http://w3id.org/dcri-ont/vocabulary/concept_00223"/>
        <skos:inScheme rdf:resource="http://w3id.org/dcri-ont/vocabulary/conceptscheme"/>
        <rdfs:comment xml:lang="en">Atomizer used for applying a fine spray of paint or another coating or consolidant by compressed air.</rdfs:comment>
        <rdfs:comment xml:lang="el">Ψεκαστήρας που χρησιμοποιείται για την εφαρμογή ενός λεπτού ψεκάσματος χρώματος ή κάποιου άλλου επικαλυπτικού ή συγκολλητικού υλικού με πεπιεσμένο αέρα.</rdfs:comment>
        <rdfs:label xml:lang="en">Airbrush</rdfs:label>
        <rdfs:label xml:lang="el">Αερογράφος</rdfs:label>
        <skos:definition xml:lang="en">Atomizer used for applying a fine spray of paint or another coating or consolidant by compressed air.</skos:definition>
        <skos:definition xml:lang="el">Ψεκαστήρας που χρησιμοποιείται για την εφαρμογή ενός λεπτού ψεκάσματος χρώματος ή κάποιου άλλου επικαλυπτικού ή συγκολλητικού υλικού με πεπιεσμένο αέρα.</skos:definition>
        <skos:prefLabel xml:lang="en">Airbrush</skos:prefLabel>
        <skos:prefLabel xml:lang="el">Αερογράφος</skos:prefLabel>
    </owl:NamedIndividual>
    


    <!-- http://w3id.org/dcri-ont/vocabulary/concept_00167 -->


    <owl:NamedIndividual rdf:about="http://w3id.org/dcri-ont/vocabulary/concept_00167">
        <rdf:type rdf:resource="http://www.w3.org/2004/02/skos/core#Concept"/>
        <skos:broader rdf:resource="http://w3id.org/dcri-ont/vocabulary/concept_00222"/>
        <skos:inScheme rdf:resource="http://w3id.org/dcri-ont/vocabulary/conceptscheme"/>
        <rdfs:comment xml:lang="en">Methylated derivative of cellulose. It is usually used in the context of textile and paper conservation interventions related to consolidation, as well as to cleaning-removal of stains.</rdfs:comment>
        <rdfs:comment xml:lang="el">Μεθυλιωμένο παράγωγο κυτταρίνης. Χρησιμοποιείται συνήθως στο πλαίσιο επεμβάσεων συντήρησης χαρτιού και υφάσματος σχετικές με συγκόλληση, καθώς και για τον καθαρισμό-αφαίρεση λεκκέδων.</rdfs:comment>
        <rdfs:label xml:lang="en">Methyl cellulose</rdfs:label>
        <rdfs:label xml:lang="el">Μεθυλοκυτταρίνη</rdfs:label>
        <skos:definition xml:lang="en">Methylated derivative of cellulose. It is usually used in the context of textile and paper conservation interventions related to consolidation, as well as to cleaning-removal of stains.</skos:definition>
        <skos:definition xml:lang="el">Μεθυλιωμένο παράγωγο κυτταρίνης. Χρησιμοποιείται συνήθως στο πλαίσιο επεμβάσεων συντήρησης χαρτιού και υφάσματος σχετικές με συγκόλληση, καθώς και για τον καθαρισμό-αφαίρεση λεκκέδων.</skos:definition>
        <skos:prefLabel xml:lang="en">Methyl cellulose</skos:prefLabel>
        <skos:prefLabel xml:lang="el">Μεθυλοκυτταρίνη</skos:prefLabel>
    </owl:NamedIndividual>
    


    <!-- http://w3id.org/dcri-ont/vocabulary/concept_00168 -->


    <owl:NamedIndividual rdf:about="http://w3id.org/dcri-ont/vocabulary/concept_00168">
        <rdf:type rdf:resource="http://www.w3.org/2004/02/skos/core#Concept"/>
        <skos:broader rdf:resource="http://w3id.org/dcri-ont/vocabulary/concept_00158"/>
        <skos:inScheme rdf:resource="http://w3id.org/dcri-ont/vocabulary/conceptscheme"/>
        <rdfs:comment xml:lang="en">A mixture of three isomeric hydrocarbons form commercial xylene. It is a colorless, flammable, toxic liquid insoluble in water.</rdfs:comment>
        <rdfs:comment xml:lang="el">Ένα μείγμα τριών ισομερών υδρογονανθράκων το οποίο σχηματίζει το εμπορικό ξυλόλιο. Είναι ένα άχρωμο, εύφλεκτο, τοξικό υγρό αδιάλυτο στο νερό.</rdfs:comment>
        <rdfs:label xml:lang="en">Xylene</rdfs:label>
        <rdfs:label xml:lang="el">Ξυλένιο</rdfs:label>
        <skos:definition xml:lang="en">A mixture of three isomeric hydrocarbons form commercial xylene. It is a colorless, flammable, toxic liquid insoluble in water.</skos:definition>
        <skos:definition xml:lang="el">Ένα μείγμα τριών ισομερών υδρογονανθράκων το οποίο σχηματίζει το εμπορικό ξυλόλιο. Είναι ένα άχρωμο, εύφλεκτο, τοξικό υγρό αδιάλυτο στο νερό.</skos:definition>
        <skos:prefLabel xml:lang="en">Xylene</skos:prefLabel>
        <skos:prefLabel xml:lang="el">Ξυλένιο</skos:prefLabel>
    </owl:NamedIndividual>
    


    <!-- http://w3id.org/dcri-ont/vocabulary/concept_00169 -->


    <owl:NamedIndividual rdf:about="http://w3id.org/dcri-ont/vocabulary/concept_00169">
        <rdf:type rdf:resource="http://www.w3.org/2004/02/skos/core#Concept"/>
        <skos:broader rdf:resource="http://w3id.org/dcri-ont/vocabulary/concept_00160"/>
        <skos:inScheme rdf:resource="http://w3id.org/dcri-ont/vocabulary/conceptscheme"/>
        <rdfs:comment xml:lang="en">Trademarked commercial name for a synthetic thermal plastic resin that does not embrittle or discolor over time, having a liquid density of 8.3 pounds per gallon, a flash point of 60 degrees Fahrenheit, and a viscosity of 3700-6200 cps. It is widely used in conservation treatments.</rdfs:comment>
        <rdfs:comment xml:lang="el">Εμπορική ονομασία για μια συνθετική θερμοπλαστική ρητίνη που δεν γίνεται εύθραυστη ή αποχρωματίζεται με την πάροδο του χρόνου, με πυκνότητα υγρού 8,3 λίβρες ανά γαλόνι, σημείο ανάφλεξης 60 βαθμούς Φαρενάιτ και ιξώδες 3700-6200 cps. Χρησιμοποιείται ευρέως σε επεμβάσεις συντήρησης σχετικές με συγκόλληση.</rdfs:comment>
        <rdfs:label xml:lang="el">Paraloid B72</rdfs:label>
        <rdfs:label xml:lang="en">Paraloid B72</rdfs:label>
        <skos:definition xml:lang="en">Trademarked commercial name for a synthetic thermal plastic resin that does not embrittle or discolor over time, having a liquid density of 8.3 pounds per gallon, a flash point of 60 degrees Fahrenheit, and a viscosity of 3700-6200 cps. It is widely used in conservation treatments.</skos:definition>
        <skos:definition xml:lang="el">Εμπορική ονομασία για μια συνθετική θερμοπλαστική ρητίνη που δεν γίνεται εύθραυστη ή αποχρωματίζεται με την πάροδο του χρόνου, με πυκνότητα υγρού 8,3 λίβρες ανά γαλόνι, σημείο ανάφλεξης 60 βαθμούς Φαρενάιτ και ιξώδες 3700-6200 cps. Χρησιμοποιείται ευρέως σε επεμβάσεις συντήρησης σχετικές με συγκόλληση.</skos:definition>
        <skos:prefLabel xml:lang="el">Paraloid B72</skos:prefLabel>
        <skos:prefLabel xml:lang="en">Paraloid B72</skos:prefLabel>
    </owl:NamedIndividual>
    


    <!-- http://w3id.org/dcri-ont/vocabulary/concept_00170 -->


    <owl:NamedIndividual rdf:about="http://w3id.org/dcri-ont/vocabulary/concept_00170">
        <rdf:type rdf:resource="http://www.w3.org/2004/02/skos/core#Concept"/>
        <skos:broader rdf:resource="http://w3id.org/dcri-ont/vocabulary/concept_00222"/>
        <skos:inScheme rdf:resource="http://w3id.org/dcri-ont/vocabulary/conceptscheme"/>
        <rdfs:comment xml:lang="en">A water-soluble, tasteless colloidal form of processed collagen obtained from bones, hooves or skins. Is high in molecular weight after processing. It is usually used in the context of conservation interventions related to consolidation and fixing of paintings and photographs.</rdfs:comment>
        <rdfs:comment xml:lang="el">Μια υδατοδιαλυτή, άνευ γεύσης, κολλοειδούς μορφής επεξεργασμένου κολλαγόνου που λαμβάνεται από οστά, οπλές ή δέρματα. Έχει υψηλό μοριακό βάρος μετά την επεξεργασία. Χρησιμοποιείται συνήθως στο πλαίσιο επεμβάσεων συντήρησης σχετικές με συγκόλληση και στερέωση ζωγραφικών έργων και φωτογραφιών.</rdfs:comment>
        <rdfs:label xml:lang="en">Gelatin</rdfs:label>
        <rdfs:label xml:lang="el">Ζελατίνη</rdfs:label>
        <skos:definition xml:lang="en">A water-soluble, tasteless colloidal form of processed collagen obtained from bones, hooves or skins. Is high in molecular weight after processing. It is usually used in the context of conservation interventions related to consolidation and fixing of paintings and photographs.</skos:definition>
        <skos:definition xml:lang="el">Μια υδατοδιαλυτή, άνευ γεύσης, κολλοειδούς μορφής επεξεργασμένου κολλαγόνου που λαμβάνεται από οστά, οπλές ή δέρματα. Έχει υψηλό μοριακό βάρος μετά την επεξεργασία. Χρησιμοποιείται συνήθως στο πλαίσιο επεμβάσεων συντήρησης σχετικές με συγκόλληση και στερέωση ζωγραφικών έργων και φωτογραφιών.</skos:definition>
        <skos:prefLabel xml:lang="en">Gelatin</skos:prefLabel>
        <skos:prefLabel xml:lang="el">Ζελατίνη</skos:prefLabel>
    </owl:NamedIndividual>
    


    <!-- http://w3id.org/dcri-ont/vocabulary/concept_00171 -->


    <owl:NamedIndividual rdf:about="http://w3id.org/dcri-ont/vocabulary/concept_00171">
        <rdf:type rdf:resource="http://www.w3.org/2004/02/skos/core#Concept"/>
        <skos:broader rdf:resource="http://w3id.org/dcri-ont/vocabulary/concept_00227"/>
        <skos:inScheme rdf:resource="http://w3id.org/dcri-ont/vocabulary/conceptscheme"/>
        <rdfs:comment xml:lang="en">The property of surface of being dull or lusterless.</rdfs:comment>
        <rdfs:comment xml:lang="el">Η ιδιότητα μιας επιφάνειας να είναι θαμπή ή χωρίς γυαλάδα.</rdfs:comment>
        <rdfs:label xml:lang="en">Matte</rdfs:label>
        <rdfs:label xml:lang="el">Μάτ</rdfs:label>
        <skos:definition xml:lang="en">The property of surface of being dull or lusterless.</skos:definition>
        <skos:definition xml:lang="el">Η ιδιότητα μιας επιφάνειας να είναι θαμπή ή χωρίς γυαλάδα.</skos:definition>
        <skos:prefLabel xml:lang="en">Matte</skos:prefLabel>
        <skos:prefLabel xml:lang="el">Μάτ</skos:prefLabel>
    </owl:NamedIndividual>
    


    <!-- http://w3id.org/dcri-ont/vocabulary/concept_00172 -->


    <owl:NamedIndividual rdf:about="http://w3id.org/dcri-ont/vocabulary/concept_00172">
        <rdf:type rdf:resource="http://www.w3.org/2004/02/skos/core#Concept"/>
        <skos:broader rdf:resource="http://w3id.org/dcri-ont/vocabulary/concept_00067"/>
        <skos:inScheme rdf:resource="http://w3id.org/dcri-ont/vocabulary/conceptscheme"/>
        <rdfs:comment xml:lang="en">A matte, opaque watercolor paint typically having gum arabic, gum senegal, or dextrin as a binder. Gouache paints differ from watercolor paints, which use transparent pigments. Chalk and other white fillers may be added to some colors.</rdfs:comment>
        <rdfs:comment xml:lang="el">Ένα ματ, αδιαφανές χρώμα ακουαρέλας που έχει τυπικά αραβικό κόμμι, κόμμι Σενεγάλης ή δεξτρίνη ως συνδετικό. Τα χρώματα γκουάς διαφέρουν από τα χρώματα ακουαρέλας, τα οποία χρησιμοποιούν διαφανείς χρωστικές. Σε ορισμένα χρώματα μπορεί να προστεθούν κιμωλία και άλλα λευκά υλικά πλήρωσης.</rdfs:comment>
        <rdfs:label xml:lang="en">Gouache</rdfs:label>
        <rdfs:label xml:lang="el">Γκουάς</rdfs:label>
        <skos:definition xml:lang="en">A matte, opaque watercolor paint typically having gum arabic, gum senegal, or dextrin as a binder. Gouache paints differ from watercolor paints, which use transparent pigments. Chalk and other white fillers may be added to some colors.</skos:definition>
        <skos:definition xml:lang="el">Ένα ματ, αδιαφανές χρώμα ακουαρέλας που έχει τυπικά αραβικό κόμμι, κόμμι Σενεγάλης ή δεξτρίνη ως συνδετικό. Τα χρώματα γκουάς διαφέρουν από τα χρώματα ακουαρέλας, τα οποία χρησιμοποιούν διαφανείς χρωστικές. Σε ορισμένα χρώματα μπορεί να προστεθούν κιμωλία και άλλα λευκά υλικά πλήρωσης.</skos:definition>
        <skos:prefLabel xml:lang="en">Gouache</skos:prefLabel>
        <skos:prefLabel xml:lang="el">Γκουάς</skos:prefLabel>
    </owl:NamedIndividual>
    


    <!-- http://w3id.org/dcri-ont/vocabulary/concept_00173 -->


    <owl:NamedIndividual rdf:about="http://w3id.org/dcri-ont/vocabulary/concept_00173">
        <rdf:type rdf:resource="http://www.w3.org/2004/02/skos/core#Concept"/>
        <skos:broader rdf:resource="http://w3id.org/dcri-ont/vocabulary/concept_00228"/>
        <skos:inScheme rdf:resource="http://w3id.org/dcri-ont/vocabulary/conceptscheme"/>
        <rdfs:comment xml:lang="en">The strength that a consolidant shows after use.</rdfs:comment>
        <rdfs:comment xml:lang="el">Η ισχύς-δύναμη που παρουσιάζει μια συγκολλητική ουσία μετά την χρήση.</rdfs:comment>
        <rdfs:label xml:lang="en">Adhesion strength</rdfs:label>
        <rdfs:label xml:lang="el">Ισχύς συγκόλλησης</rdfs:label>
        <skos:definition xml:lang="en">The strength that a consolidant shows after use.</skos:definition>
        <skos:definition xml:lang="el">Η ισχύς-δύναμη που παρουσιάζει μια συγκολλητική ουσία μετά την χρήση.</skos:definition>
        <skos:prefLabel xml:lang="en">Adhesion strength</skos:prefLabel>
        <skos:prefLabel xml:lang="el">Ισχύς συγκόλλησης</skos:prefLabel>
    </owl:NamedIndividual>
    


    <!-- http://w3id.org/dcri-ont/vocabulary/concept_00174 -->


    <owl:NamedIndividual rdf:about="http://w3id.org/dcri-ont/vocabulary/concept_00174">
        <rdf:type rdf:resource="http://www.w3.org/2004/02/skos/core#Concept"/>
        <skos:broader rdf:resource="http://w3id.org/dcri-ont/vocabulary/concept_00065"/>
        <skos:inScheme rdf:resource="http://w3id.org/dcri-ont/vocabulary/conceptscheme"/>
        <rdfs:comment xml:lang="en">A thick paper formed from multiple sheets adhered with an adhesive and pressed to produce a hard, stiff board.</rdfs:comment>
        <rdfs:comment xml:lang="el">Είδος χαρτιού μεγάλου πάχους το οποίο αποτελείται από πολλαπλά φύλλα χαρτιού κολημμένα με συγκολλητική ουσία, τα οποία έχουν πιεστεί δημιουργώντας μια σκληρή άκαμπτη επιφάνεια.</rdfs:comment>
        <rdfs:label xml:lang="en">Pasteboard</rdfs:label>
        <rdfs:label xml:lang="el">Χαρτόνι</rdfs:label>
        <skos:definition xml:lang="en">A thick paper formed from multiple sheets adhered with an adhesive and pressed to produce a hard, stiff board.</skos:definition>
        <skos:definition xml:lang="el">Είδος χαρτιού μεγάλου πάχους το οποίο αποτελείται από πολλαπλά φύλλα χαρτιού κολημμένα με συγκολλητική ουσία, τα οποία έχουν πιεστεί δημιουργώντας μια σκληρή άκαμπτη επιφάνεια.</skos:definition>
        <skos:prefLabel xml:lang="en">Pasteboard</skos:prefLabel>
        <skos:prefLabel xml:lang="el">Χαρτόνι</skos:prefLabel>
    </owl:NamedIndividual>
    


    <!-- http://w3id.org/dcri-ont/vocabulary/concept_00175 -->


    <owl:NamedIndividual rdf:about="http://w3id.org/dcri-ont/vocabulary/concept_00175">
        <rdf:type rdf:resource="http://www.w3.org/2004/02/skos/core#Concept"/>
        <skos:broader rdf:resource="http://w3id.org/dcri-ont/vocabulary/concept_00065"/>
        <skos:inScheme rdf:resource="http://w3id.org/dcri-ont/vocabulary/conceptscheme"/>
        <rdfs:comment xml:lang="en">Paper made from thin layers of pith cut from two species of rice paper trees cultivated in China, Japan, and Thailand.</rdfs:comment>
        <rdfs:comment xml:lang="el">Χαρτί φτιαγμένο από λεπτές στρώσεις φλοιού κομμένου από δύο είδη δέντρων ριζόχαρτου τα οποία καλλιεργούνται στην Κίνα, την Ιαπωνία και την Ταιλάνδη.</rdfs:comment>
        <rdfs:label xml:lang="en">Rice paper</rdfs:label>
        <rdfs:label xml:lang="el">Ριζόχαρτο</rdfs:label>
        <skos:definition xml:lang="en">Paper made from thin layers of pith cut from two species of rice paper trees cultivated in China, Japan, and Thailand.</skos:definition>
        <skos:definition xml:lang="el">Χαρτί φτιαγμένο από λεπτές στρώσεις φλοιού κομμένου από δύο είδη δέντρων ριζόχαρτου τα οποία καλλιεργούνται στην Κίνα, την Ιαπωνία και την Ταιλάνδη.</skos:definition>
        <skos:prefLabel xml:lang="en">Rice paper</skos:prefLabel>
        <skos:prefLabel xml:lang="el">Ριζόχαρτο</skos:prefLabel>
    </owl:NamedIndividual>
    


    <!-- http://w3id.org/dcri-ont/vocabulary/concept_00176 -->


    <owl:NamedIndividual rdf:about="http://w3id.org/dcri-ont/vocabulary/concept_00176">
        <rdf:type rdf:resource="http://www.w3.org/2004/02/skos/core#Concept"/>
        <skos:broader rdf:resource="http://w3id.org/dcri-ont/vocabulary/concept_00067"/>
        <skos:inScheme rdf:resource="http://w3id.org/dcri-ont/vocabulary/conceptscheme"/>
        <rdfs:comment xml:lang="en">A paint made bypigments and a drying oil such as linseed oil.</rdfs:comment>
        <rdfs:comment xml:lang="el">Μπογιά φτιαγμένη από ανάμειξη χρωστικών και ξηραινόμενων ελαίων όπως λινέλαιο.</rdfs:comment>
        <rdfs:label xml:lang="en">Oil paint</rdfs:label>
        <rdfs:label xml:lang="el">Λάδι (χρώμα)</rdfs:label>
        <skos:definition xml:lang="en">A paint made bypigments and a drying oil such as linseed oil.</skos:definition>
        <skos:definition xml:lang="el">Μπογιά φτιαγμένη από ανάμειξη χρωστικών και ξηραινόμενων ελαίων όπως λινέλαιο.</skos:definition>
        <skos:prefLabel xml:lang="en">Oil paint</skos:prefLabel>
        <skos:prefLabel xml:lang="el">Λάδι (χρώμα)</skos:prefLabel>
    </owl:NamedIndividual>
    


    <!-- http://w3id.org/dcri-ont/vocabulary/concept_00177 -->


    <owl:NamedIndividual rdf:about="http://w3id.org/dcri-ont/vocabulary/concept_00177">
        <rdf:type rdf:resource="http://www.w3.org/2004/02/skos/core#Concept"/>
        <skos:broader rdf:resource="http://w3id.org/dcri-ont/vocabulary/concept_00067"/>
        <skos:inScheme rdf:resource="http://w3id.org/dcri-ont/vocabulary/conceptscheme"/>
        <rdfs:comment xml:lang="en">A paint made by pigments or dyes in acrylic, which is a colorless, transparent, thermoplastic synthetic resin made by the polymerization of acrylic acid derivatives.</rdfs:comment>
        <rdfs:comment xml:lang="el">Χρώμα από χρωστικές ή βαφές σε ακρυλικό, το οποίο είναι μια άχρωμη, διάφανη, θερμοπλαστική συνθετική ρητίνη φτιαγμένη από τον πολυμερισμό παραγώγων ακρυλικού οξέος.</rdfs:comment>
        <rdfs:label xml:lang="en">Acrylic paint</rdfs:label>
        <rdfs:label xml:lang="el">Ακρυλικό (χρώμα)</rdfs:label>
        <skos:definition xml:lang="en">A paint made by pigments or dyes in acrylic, which is a colorless, transparent, thermoplastic synthetic resin made by the polymerization of acrylic acid derivatives.</skos:definition>
        <skos:definition xml:lang="el">Χρώμα από χρωστικές ή βαφές σε ακρυλικό, το οποίο είναι μια άχρωμη, διάφανη, θερμοπλαστική συνθετική ρητίνη φτιαγμένη από τον πολυμερισμό παραγώγων ακρυλικού οξέος.</skos:definition>
        <skos:prefLabel xml:lang="en">Acrylic paint</skos:prefLabel>
        <skos:prefLabel xml:lang="el">Ακρυλικό (χρώμα)</skos:prefLabel>
    </owl:NamedIndividual>
    


    <!-- http://w3id.org/dcri-ont/vocabulary/concept_00178 -->


    <owl:NamedIndividual rdf:about="http://w3id.org/dcri-ont/vocabulary/concept_00178">
        <rdf:type rdf:resource="http://www.w3.org/2004/02/skos/core#Concept"/>
        <skos:broader rdf:resource="http://w3id.org/dcri-ont/vocabulary/concept_00067"/>
        <skos:inScheme rdf:resource="http://w3id.org/dcri-ont/vocabulary/conceptscheme"/>
        <rdfs:comment xml:lang="en">A paint made by pigments and egg (usually the yolk).</rdfs:comment>
        <rdfs:comment xml:lang="el">Χρώμα φτιαγμένο από ανάμειξη χρωστικών και αυγό (συνήθως τον κρόκο).</rdfs:comment>
        <rdfs:label xml:lang="en">Egg tempera</rdfs:label>
        <rdfs:label xml:lang="el">Αυγοτέμπερα</rdfs:label>
        <skos:definition xml:lang="en">A paint made by pigments and egg (usually the yolk).</skos:definition>
        <skos:definition xml:lang="el">Χρώμα φτιαγμένο από ανάμειξη χρωστικών και αυγό (συνήθως τον κρόκο).</skos:definition>
        <skos:prefLabel xml:lang="en">Egg tempera</skos:prefLabel>
        <skos:prefLabel xml:lang="el">Αυγοτέμπερα</skos:prefLabel>
    </owl:NamedIndividual>
    


    <!-- http://w3id.org/dcri-ont/vocabulary/concept_00179 -->


    <owl:NamedIndividual rdf:about="http://w3id.org/dcri-ont/vocabulary/concept_00179">
        <rdf:type rdf:resource="http://www.w3.org/2004/02/skos/core#Concept"/>
        <skos:broader rdf:resource="http://w3id.org/dcri-ont/vocabulary/concept_00222"/>
        <skos:inScheme rdf:resource="http://w3id.org/dcri-ont/vocabulary/conceptscheme"/>
        <rdfs:comment xml:lang="en">An amorphous, inorganic substance made by fusing silica (silicon dioxide) with a basic oxide; generally transparent but often translucent or opaque.</rdfs:comment>
        <rdfs:comment xml:lang="el">Μια άμορφη, ανόργανη ουσία φτιαγμένη από σύντηξη διοξειδίου του πυρητίου με βασικό οξείδιο. Γενικά είναι διάφανο, αλλά μπορεί να είναι και ημιδιάφανο ή αδιάφανο.</rdfs:comment>
        <rdfs:label xml:lang="en">Glass</rdfs:label>
        <rdfs:label xml:lang="el">Γυαλί</rdfs:label>
        <skos:definition xml:lang="en">An amorphous, inorganic substance made by fusing silica (silicon dioxide) with a basic oxide; generally transparent but often translucent or opaque.</skos:definition>
        <skos:definition xml:lang="el">Μια άμορφη, ανόργανη ουσία φτιαγμένη από σύντηξη διοξειδίου του πυρητίου με βασικό οξείδιο. Γενικά είναι διάφανο, αλλά μπορεί να είναι και ημιδιάφανο ή αδιάφανο.</skos:definition>
        <skos:prefLabel xml:lang="en">Glass</skos:prefLabel>
        <skos:prefLabel xml:lang="el">Γυαλί</skos:prefLabel>
    </owl:NamedIndividual>
    


    <!-- http://w3id.org/dcri-ont/vocabulary/concept_00180 -->


    <owl:NamedIndividual rdf:about="http://w3id.org/dcri-ont/vocabulary/concept_00180">
        <rdf:type rdf:resource="http://www.w3.org/2004/02/skos/core#Concept"/>
        <skos:broader rdf:resource="http://w3id.org/dcri-ont/vocabulary/concept_00069"/>
        <skos:inScheme rdf:resource="http://w3id.org/dcri-ont/vocabulary/conceptscheme"/>
        <rdfs:comment xml:lang="en">Proprietary name for polymerized methyl methacrylate, used as a substitute for glass in products such as windows, frames etc.</rdfs:comment>
        <rdfs:comment xml:lang="el">Εμπορικό όνομα του πολυμερισμένου μεθακρυλικό μεθυλεστέρα, που χρησιμοποιείται ως υποκατάστατο του γυαλιού σε προιόντα όπως τα παράθυρα, οι κορνίζες κ.ά.</rdfs:comment>
        <rdfs:label xml:lang="en">Plexiglass</rdfs:label>
        <rdfs:label xml:lang="el">Πλέξιγκλας</rdfs:label>
        <skos:definition xml:lang="en">Proprietary name for polymerized methyl methacrylate, used as a substitute for glass in products such as windows, frames etc.</skos:definition>
        <skos:definition xml:lang="el">Εμπορικό όνομα του πολυμερισμένου μεθακρυλικό μεθυλεστέρα, που χρησιμοποιείται ως υποκατάστατο του γυαλιού σε προιόντα όπως τα παράθυρα, οι κορνίζες κ.ά.</skos:definition>
        <skos:prefLabel xml:lang="en">Plexiglass</skos:prefLabel>
        <skos:prefLabel xml:lang="el">Πλέξιγκλας</skos:prefLabel>
    </owl:NamedIndividual>
    


    <!-- http://w3id.org/dcri-ont/vocabulary/concept_00181 -->


    <owl:NamedIndividual rdf:about="http://w3id.org/dcri-ont/vocabulary/concept_00181">
        <rdf:type rdf:resource="http://www.w3.org/2004/02/skos/core#Concept"/>
        <skos:broader rdf:resource="http://w3id.org/dcri-ont/vocabulary/concept_00226"/>
        <skos:inScheme rdf:resource="http://w3id.org/dcri-ont/vocabulary/conceptscheme"/>
        <rdfs:comment xml:lang="en">The edges of the area where cracking of a surface occurs are uplifted.</rdfs:comment>
        <rdfs:comment xml:lang="el">Οι ακμές περιμετρικά της περιοχής που παρουσιάζουν ρωγμή έχουν ανυψωθεί.</rdfs:comment>
        <rdfs:label xml:lang="en">Uplifted crack edge</rdfs:label>
        <rdfs:label xml:lang="el">Ανυψωμένα άκρα ρωγμών</rdfs:label>
        <skos:definition xml:lang="en">The edges of the area where cracking of a surface occurs are uplifted.</skos:definition>
        <skos:definition xml:lang="el">Οι ακμές περιμετρικά της περιοχής που παρουσιάζουν ρωγμή έχουν ανυψωθεί.</skos:definition>
        <skos:prefLabel xml:lang="en">Uplifted crack edge</skos:prefLabel>
        <skos:prefLabel xml:lang="el">Ανυψωμένα άκρα ρωγμών</skos:prefLabel>
    </owl:NamedIndividual>
    


    <!-- http://w3id.org/dcri-ont/vocabulary/concept_00182 -->


    <owl:NamedIndividual rdf:about="http://w3id.org/dcri-ont/vocabulary/concept_00182">
        <rdf:type rdf:resource="http://www.w3.org/2004/02/skos/core#Concept"/>
        <skos:broader rdf:resource="http://w3id.org/dcri-ont/vocabulary/concept_00183"/>
        <skos:inScheme rdf:resource="http://w3id.org/dcri-ont/vocabulary/conceptscheme"/>
        <rdfs:comment xml:lang="en">The removal of an object or object component from physical contact with another.</rdfs:comment>
        <rdfs:comment xml:lang="el">Η αφαίρεση ενός αντικειμένου ή ενός τμήματος αντικειμένου από την φυσική επαφή που είχε με ένα άλλο.</rdfs:comment>
        <rdfs:label xml:lang="en">Detaching</rdfs:label>
        <rdfs:label xml:lang="el">Αποκολλήσεις</rdfs:label>
        <skos:definition xml:lang="en">The removal of an object or object component from physical contact with another.</skos:definition>
        <skos:definition xml:lang="el">Η αφαίρεση ενός αντικειμένου ή ενός τμήματος αντικειμένου από την φυσική επαφή που είχε με ένα άλλο.</skos:definition>
        <skos:prefLabel xml:lang="en">Detaching</skos:prefLabel>
        <skos:prefLabel xml:lang="el">Αποκολλήσεις</skos:prefLabel>
    </owl:NamedIndividual>
    


    <!-- http://w3id.org/dcri-ont/vocabulary/concept_00183 -->


    <owl:NamedIndividual rdf:about="http://w3id.org/dcri-ont/vocabulary/concept_00183">
        <rdf:type rdf:resource="http://www.w3.org/2004/02/skos/core#Concept"/>
        <skos:broader rdf:resource="http://w3id.org/dcri-ont/vocabulary/concept_00227"/>
        <skos:inScheme rdf:resource="http://w3id.org/dcri-ont/vocabulary/conceptscheme"/>
        <rdfs:comment xml:lang="en">Fracturing in a material or object, usually along a single or branched path.</rdfs:comment>
        <rdfs:comment xml:lang="el">Διάνοιξη σε ένα υλικό ή αντικείμενο, συνήθως κατά μήκος ενός μονού ή διακλαδισμένου μονοπατιού.</rdfs:comment>
        <rdfs:label xml:lang="en">Crack</rdfs:label>
        <rdfs:label xml:lang="el">Ρωγμές</rdfs:label>
        <skos:definition xml:lang="en">Fracturing in a material or object, usually along a single or branched path.</skos:definition>
        <skos:definition xml:lang="el">Διάνοιξη σε ένα υλικό ή αντικείμενο, συνήθως κατά μήκος ενός μονού ή διακλαδισμένου μονοπατιού.</skos:definition>
        <skos:prefLabel xml:lang="en">Crack</skos:prefLabel>
        <skos:prefLabel xml:lang="el">Ρωγμές</skos:prefLabel>
    </owl:NamedIndividual>
    


    <!-- http://w3id.org/dcri-ont/vocabulary/concept_00184 -->


    <owl:NamedIndividual rdf:about="http://w3id.org/dcri-ont/vocabulary/concept_00184">
        <rdf:type rdf:resource="http://www.w3.org/2004/02/skos/core#Concept"/>
        <skos:broader rdf:resource="http://w3id.org/dcri-ont/vocabulary/concept_00227"/>
        <skos:inScheme rdf:resource="http://w3id.org/dcri-ont/vocabulary/conceptscheme"/>
        <rdfs:label xml:lang="en">Adhesion problem</rdfs:label>
        <rdfs:label xml:lang="el">Προβλήματα πρόσφυσης</rdfs:label>
        <skos:prefLabel xml:lang="en">Adhesion problem</skos:prefLabel>
        <skos:prefLabel xml:lang="el">Προβλήματα πρόσφυσης</skos:prefLabel>
    </owl:NamedIndividual>
    


    <!-- http://w3id.org/dcri-ont/vocabulary/concept_00186 -->


    <owl:NamedIndividual rdf:about="http://w3id.org/dcri-ont/vocabulary/concept_00186">
        <rdf:type rdf:resource="http://www.w3.org/2004/02/skos/core#Concept"/>
        <skos:broader rdf:resource="http://w3id.org/dcri-ont/vocabulary/concept_00227"/>
        <skos:inScheme rdf:resource="http://w3id.org/dcri-ont/vocabulary/conceptscheme"/>
        <rdfs:label xml:lang="en">Flimsiness</rdfs:label>
        <rdfs:label xml:lang="el">Σαθρότητα</rdfs:label>
        <skos:prefLabel xml:lang="en">Flimsiness</skos:prefLabel>
        <skos:prefLabel xml:lang="el">Σαθρότητα</skos:prefLabel>
    </owl:NamedIndividual>
    


    <!-- http://w3id.org/dcri-ont/vocabulary/concept_00187 -->


    <owl:NamedIndividual rdf:about="http://w3id.org/dcri-ont/vocabulary/concept_00187">
        <rdf:type rdf:resource="http://www.w3.org/2004/02/skos/core#Concept"/>
        <skos:broader rdf:resource="http://w3id.org/dcri-ont/vocabulary/concept_00155"/>
        <skos:inScheme rdf:resource="http://w3id.org/dcri-ont/vocabulary/conceptscheme"/>
        <rdfs:label xml:lang="en">Soft pencil</rdfs:label>
        <rdfs:label xml:lang="el">Μαλακό μολύβι</rdfs:label>
        <skos:prefLabel xml:lang="en">Soft pencil</skos:prefLabel>
        <skos:prefLabel xml:lang="el">Μαλακό μολύβι</skos:prefLabel>
    </owl:NamedIndividual>
    


    <!-- http://w3id.org/dcri-ont/vocabulary/concept_00188 -->


    <owl:NamedIndividual rdf:about="http://w3id.org/dcri-ont/vocabulary/concept_00188">
        <rdf:type rdf:resource="http://www.w3.org/2004/02/skos/core#Concept"/>
        <skos:broader rdf:resource="http://w3id.org/dcri-ont/vocabulary/concept_00155"/>
        <skos:inScheme rdf:resource="http://w3id.org/dcri-ont/vocabulary/conceptscheme"/>
        <rdfs:label xml:lang="en">Hard pencil</rdfs:label>
        <rdfs:label xml:lang="el">Σκληρό μολύβι</rdfs:label>
        <skos:prefLabel xml:lang="en">Hard pencil</skos:prefLabel>
        <skos:prefLabel xml:lang="el">Σκληρό μολύβι</skos:prefLabel>
    </owl:NamedIndividual>
    


    <!-- http://w3id.org/dcri-ont/vocabulary/concept_00189 -->


    <owl:NamedIndividual rdf:about="http://w3id.org/dcri-ont/vocabulary/concept_00189">
        <rdf:type rdf:resource="http://www.w3.org/2004/02/skos/core#Concept"/>
        <skos:broader rdf:resource="http://w3id.org/dcri-ont/vocabulary/concept_00222"/>
        <skos:inScheme rdf:resource="http://w3id.org/dcri-ont/vocabulary/conceptscheme"/>
        <rdfs:comment xml:lang="en">The suspension of droplets of one liquid in another liquid in which the first liquid is not soluble. Also, an intimate mixture of a solid or semi-solid substance with a liquid, sometimes with the aid of an emulsifier. In photography, the mixture of binder and final image material.</rdfs:comment>
        <rdfs:comment xml:lang="el">Το εναιώρημα σταγονιδίων ενός υγρού σε άλλο υγρό στο οποίο το πρώτο υγρό δεν είναι διαλυτό. Επίσης, ένα μείγμα στερεάς ή ημιστερεής ουσίας με υγρό, μερικές φορές με τη βοήθεια γαλακτωματοποιητή. Στη φωτογραφία, η μίξη του συνδετικού υλικού και του τελικού υλικού εικόνας.</rdfs:comment>
        <rdfs:label xml:lang="en">Emulsion</rdfs:label>
        <rdfs:label xml:lang="el">Γαλάκτωμα</rdfs:label>
        <skos:definition xml:lang="en">The suspension of droplets of one liquid in another liquid in which the first liquid is not soluble. Also, an intimate mixture of a solid or semi-solid substance with a liquid, sometimes with the aid of an emulsifier. In photography, the mixture of binder and final image material.</skos:definition>
        <skos:definition xml:lang="el">Το εναιώρημα σταγονιδίων ενός υγρού σε άλλο υγρό στο οποίο το πρώτο υγρό δεν είναι διαλυτό. Επίσης, ένα μείγμα στερεάς ή ημιστερεής ουσίας με υγρό, μερικές φορές με τη βοήθεια γαλακτωματοποιητή. Στη φωτογραφία, η μίξη του συνδετικού υλικού και του τελικού υλικού εικόνας.</skos:definition>
        <skos:prefLabel xml:lang="en">Emulsion</skos:prefLabel>
        <skos:prefLabel xml:lang="el">Γαλάκτωμα</skos:prefLabel>
    </owl:NamedIndividual>
    


    <!-- http://w3id.org/dcri-ont/vocabulary/concept_00190 -->


    <owl:NamedIndividual rdf:about="http://w3id.org/dcri-ont/vocabulary/concept_00190">
        <rdf:type rdf:resource="http://www.w3.org/2004/02/skos/core#Concept"/>
        <skos:broader rdf:resource="http://w3id.org/dcri-ont/vocabulary/concept_00222"/>
        <skos:inScheme rdf:resource="http://w3id.org/dcri-ont/vocabulary/conceptscheme"/>
        <skos:narrower rdf:resource="http://w3id.org/dcri-ont/vocabulary/concept_00219"/>
        <skos:narrower rdf:resource="http://w3id.org/dcri-ont/vocabulary/concept_00220"/>
        <skos:narrower rdf:resource="http://w3id.org/dcri-ont/vocabulary/concept_00221"/>
        <rdfs:comment xml:lang="en">Use generally for any substance spread over a surface, usually for protection or decoration.</rdfs:comment>
        <rdfs:comment xml:lang="el">Αναφέρεται γενικά σε οποιαδήποτε ουσία απλώνεται σε μια επιφάνεια, συνήθως για προστασία ή διακόσμηση.</rdfs:comment>
        <rdfs:label xml:lang="en">Coating</rdfs:label>
        <rdfs:label xml:lang="el">Επικαλυπτικό υλικό</rdfs:label>
        <skos:definition xml:lang="en">Use generally for any substance spread over a surface, usually for protection or decoration.</skos:definition>
        <skos:definition xml:lang="el">Αναφέρεται γενικά σε οποιαδήποτε ουσία απλώνεται σε μια επιφάνεια, συνήθως για προστασία ή διακόσμηση.</skos:definition>
        <skos:prefLabel xml:lang="en">Coating</skos:prefLabel>
        <skos:prefLabel xml:lang="el">Επικαλυπτικό υλικό</skos:prefLabel>
    </owl:NamedIndividual>
    


    <!-- http://w3id.org/dcri-ont/vocabulary/concept_00191 -->


    <owl:NamedIndividual rdf:about="http://w3id.org/dcri-ont/vocabulary/concept_00191">
        <rdf:type rdf:resource="http://www.w3.org/2004/02/skos/core#Concept"/>
        <skos:broader rdf:resource="http://w3id.org/dcri-ont/vocabulary/concept_00222"/>
        <skos:inScheme rdf:resource="http://w3id.org/dcri-ont/vocabulary/conceptscheme"/>
        <rdfs:comment xml:lang="en">The skin of an animal that has been processed for further use e.g., for furniture, clothing, bookbinding. It is relatively soft and flexible when dry.</rdfs:comment>
        <rdfs:comment xml:lang="el">Το δέρμα ζώου που έχει υποστεί επεξεργασία για περαιτέρω χρήση όπως π.χ., η κατασκευή επίπλων, ρουχισμού, βιβλιοδεσίας. Είναι σχετικά μαλακό και εύκαμπτο όταν είναι στεγνό.</rdfs:comment>
        <rdfs:label xml:lang="en">Leather</rdfs:label>
        <rdfs:label xml:lang="el">Δέρμα</rdfs:label>
        <skos:definition xml:lang="en">The skin of an animal that has been processed for further use e.g., for furniture, clothing, bookbinding. It is relatively soft and flexible when dry.</skos:definition>
        <skos:definition xml:lang="el">Το δέρμα ζώου που έχει υποστεί επεξεργασία για περαιτέρω χρήση όπως π.χ., η κατασκευή επίπλων, ρουχισμού, βιβλιοδεσίας. Είναι σχετικά μαλακό και εύκαμπτο όταν είναι στεγνό.</skos:definition>
        <skos:prefLabel xml:lang="en">Leather</skos:prefLabel>
        <skos:prefLabel xml:lang="el">Δέρμα</skos:prefLabel>
    </owl:NamedIndividual>
    


    <!-- http://w3id.org/dcri-ont/vocabulary/concept_00192 -->


    <owl:NamedIndividual rdf:about="http://w3id.org/dcri-ont/vocabulary/concept_00192">
        <rdf:type rdf:resource="http://www.w3.org/2004/02/skos/core#Concept"/>
        <skos:broader rdf:resource="http://w3id.org/dcri-ont/vocabulary/concept_00222"/>
        <skos:inScheme rdf:resource="http://w3id.org/dcri-ont/vocabulary/conceptscheme"/>
        <rdfs:label xml:lang="en">Leatherette</rdfs:label>
        <rdfs:label xml:lang="el">Δερματίνη</rdfs:label>
        <skos:prefLabel xml:lang="en">Leatherette</skos:prefLabel>
        <skos:prefLabel xml:lang="el">Δερματίνη</skos:prefLabel>
    </owl:NamedIndividual>
    


    <!-- http://w3id.org/dcri-ont/vocabulary/concept_00193 -->


    <owl:NamedIndividual rdf:about="http://w3id.org/dcri-ont/vocabulary/concept_00193">
        <rdf:type rdf:resource="http://www.w3.org/2004/02/skos/core#Concept"/>
        <skos:broader rdf:resource="http://w3id.org/dcri-ont/vocabulary/concept_00227"/>
        <skos:inScheme rdf:resource="http://w3id.org/dcri-ont/vocabulary/conceptscheme"/>
        <rdfs:comment xml:lang="en">A symptom of oxidative-reductive deterioration in photographs.</rdfs:comment>
        <rdfs:comment xml:lang="el">Ένα σύμπτωμα οξειδωτικής-αναγωγικής φθοράς στις φωτογραφίες.</rdfs:comment>
        <rdfs:label xml:lang="en">Silver mirroring</rdfs:label>
        <rdfs:label xml:lang="el">Καθρέφτισμα</rdfs:label>
        <skos:definition xml:lang="en">A symptom of oxidative-reductive deterioration in photographs.</skos:definition>
        <skos:definition xml:lang="el">Ένα σύμπτωμα οξειδωτικής-αναγωγικής φθοράς στις φωτογραφίες.</skos:definition>
        <skos:prefLabel xml:lang="en">Silver mirroring</skos:prefLabel>
        <skos:prefLabel xml:lang="el">Καθρέφτισμα</skos:prefLabel>
    </owl:NamedIndividual>
    


    <!-- http://w3id.org/dcri-ont/vocabulary/concept_00194 -->


    <owl:NamedIndividual rdf:about="http://w3id.org/dcri-ont/vocabulary/concept_00194">
        <rdf:type rdf:resource="http://www.w3.org/2004/02/skos/core#Concept"/>
        <skos:broader rdf:resource="http://w3id.org/dcri-ont/vocabulary/concept_00223"/>
        <skos:inScheme rdf:resource="http://w3id.org/dcri-ont/vocabulary/conceptscheme"/>
        <rdfs:comment xml:lang="en">Sponge composed of rubber, which is used for the removal of dirt and mainly soot from surgaces.</rdfs:comment>
        <rdfs:comment xml:lang="el">Σφουγγάρι φτιαγμένο από καουτσούκ, το οποίο χρησιμοποιείται για την απομάκρυνση βρωμιάς και κατά κύριο λόγο αιθάλης από επιφάνειες.</rdfs:comment>
        <rdfs:label xml:lang="en">Smoke sponge</rdfs:label>
        <rdfs:label xml:lang="el">Σφουγγάρι αιθάλης</rdfs:label>
        <skos:definition xml:lang="en">Sponge composed of rubber, which is used for the removal of dirt and mainly soot from surgaces.</skos:definition>
        <skos:definition xml:lang="el">Σφουγγάρι φτιαγμένο από καουτσούκ, το οποίο χρησιμοποιείται για την απομάκρυνση βρωμιάς και κατά κύριο λόγο αιθάλης από επιφάνειες.</skos:definition>
        <skos:prefLabel xml:lang="en">Smoke sponge</skos:prefLabel>
        <skos:prefLabel xml:lang="el">Σφουγγάρι αιθάλης</skos:prefLabel>
    </owl:NamedIndividual>
    


    <!-- http://w3id.org/dcri-ont/vocabulary/concept_00195 -->


    <owl:NamedIndividual rdf:about="http://w3id.org/dcri-ont/vocabulary/concept_00195">
        <rdf:type rdf:resource="http://www.w3.org/2004/02/skos/core#Concept"/>
        <skos:broader rdf:resource="http://w3id.org/dcri-ont/vocabulary/concept_00223"/>
        <skos:inScheme rdf:resource="http://w3id.org/dcri-ont/vocabulary/conceptscheme"/>
        <rdfs:comment xml:lang="en">Fine particles of erasers used for the removal of dirt from (mainly) paper composed surfaces.</rdfs:comment>
        <rdfs:comment xml:lang="el">Μικρά κομμάτια γόμας που χρησιμοποιούνται για την απομάκρυνση βρωμιάς από (κυρίως) επιφάνειες από χαρτί.</rdfs:comment>
        <rdfs:label xml:lang="en">Eraser crumbs</rdfs:label>
        <rdfs:label xml:lang="el">Τρίμματα γόμας</rdfs:label>
        <skos:definition xml:lang="en">Fine particles of erasers used for the removal of dirt from (mainly) paper composed surfaces.</skos:definition>
        <skos:definition xml:lang="el">Μικρά κομμάτια γόμας που χρησιμοποιούνται για την απομάκρυνση βρωμιάς από (κυρίως) επιφάνειες από χαρτί.</skos:definition>
        <skos:prefLabel xml:lang="en">Eraser crumbs</skos:prefLabel>
        <skos:prefLabel xml:lang="el">Τρίμματα γόμας</skos:prefLabel>
    </owl:NamedIndividual>
    


    <!-- http://w3id.org/dcri-ont/vocabulary/concept_00196 -->


    <owl:NamedIndividual rdf:about="http://w3id.org/dcri-ont/vocabulary/concept_00196">
        <rdf:type rdf:resource="http://www.w3.org/2004/02/skos/core#Concept"/>
        <skos:broader rdf:resource="http://w3id.org/dcri-ont/vocabulary/concept_00227"/>
        <skos:inScheme rdf:resource="http://w3id.org/dcri-ont/vocabulary/conceptscheme"/>
        <rdfs:comment xml:lang="en">It refers to the looseness that textile support presents when it is not fully stretched on the support.</rdfs:comment>
        <rdfs:comment xml:lang="el">Αναφέρεται στην χαλαρότητα που παρουσιάζεται όταν το ύφασμα δεν είναι πλήρως τεντωμένο στο υποστήριγμα.</rdfs:comment>
        <rdfs:label xml:lang="en">Looseness</rdfs:label>
        <rdfs:label xml:lang="el">Χαλαρότητα</rdfs:label>
        <skos:definition xml:lang="en">It refers to the looseness that textile support presents when it is not fully stretched on the support.</skos:definition>
        <skos:definition xml:lang="el">Αναφέρεται στην χαλαρότητα που παρουσιάζεται όταν το ύφασμα δεν είναι πλήρως τεντωμένο στο υποστήριγμα.</skos:definition>
        <skos:prefLabel xml:lang="en">Looseness</skos:prefLabel>
        <skos:prefLabel xml:lang="el">Χαλαρότητα</skos:prefLabel>
    </owl:NamedIndividual>
    


    <!-- http://w3id.org/dcri-ont/vocabulary/concept_00197 -->


    <owl:NamedIndividual rdf:about="http://w3id.org/dcri-ont/vocabulary/concept_00197">
        <rdf:type rdf:resource="http://www.w3.org/2004/02/skos/core#Concept"/>
        <skos:broader rdf:resource="http://w3id.org/dcri-ont/vocabulary/concept_00228"/>
        <skos:inScheme rdf:resource="http://w3id.org/dcri-ont/vocabulary/conceptscheme"/>
        <rdfs:label xml:lang="en">Size</rdfs:label>
        <rdfs:label xml:lang="el">Μέγεθος</rdfs:label>
        <skos:prefLabel xml:lang="en">Size</skos:prefLabel>
        <skos:prefLabel xml:lang="el">Μέγεθος</skos:prefLabel>
    </owl:NamedIndividual>
    


    <!-- http://w3id.org/dcri-ont/vocabulary/concept_00198 -->


    <owl:NamedIndividual rdf:about="http://w3id.org/dcri-ont/vocabulary/concept_00198">
        <rdf:type rdf:resource="http://www.w3.org/2004/02/skos/core#Concept"/>
        <skos:broader rdf:resource="http://w3id.org/dcri-ont/vocabulary/concept_00222"/>
        <skos:inScheme rdf:resource="http://w3id.org/dcri-ont/vocabulary/conceptscheme"/>
        <rdfs:label xml:lang="en">Stone</rdfs:label>
        <rdfs:label xml:lang="el">Λίθος</rdfs:label>
        <skos:prefLabel xml:lang="en">Stone</skos:prefLabel>
        <skos:prefLabel xml:lang="el">Λίθος</skos:prefLabel>
    </owl:NamedIndividual>
    


    <!-- http://w3id.org/dcri-ont/vocabulary/concept_00199 -->


    <owl:NamedIndividual rdf:about="http://w3id.org/dcri-ont/vocabulary/concept_00199">
        <rdf:type rdf:resource="http://www.w3.org/2004/02/skos/core#Concept"/>
        <skos:broader rdf:resource="http://w3id.org/dcri-ont/vocabulary/concept_00222"/>
        <skos:inScheme rdf:resource="http://w3id.org/dcri-ont/vocabulary/conceptscheme"/>
        <rdfs:label xml:lang="en">Ceramic</rdfs:label>
        <rdfs:label xml:lang="el">Κεραμικό</rdfs:label>
        <skos:prefLabel xml:lang="en">Ceramic</skos:prefLabel>
        <skos:prefLabel xml:lang="el">Κεραμικό</skos:prefLabel>
    </owl:NamedIndividual>
    


    <!-- http://w3id.org/dcri-ont/vocabulary/concept_00200 -->


    <owl:NamedIndividual rdf:about="http://w3id.org/dcri-ont/vocabulary/concept_00200">
        <rdf:type rdf:resource="http://www.w3.org/2004/02/skos/core#Concept"/>
        <skos:broader rdf:resource="http://w3id.org/dcri-ont/vocabulary/concept_00228"/>
        <skos:inScheme rdf:resource="http://w3id.org/dcri-ont/vocabulary/conceptscheme"/>
        <rdfs:label xml:lang="en">Physical feature extent</rdfs:label>
        <rdfs:label xml:lang="el">Έκταση φυσικού χαρακτηριστικού</rdfs:label>
        <skos:prefLabel xml:lang="en">Physical feature extent</skos:prefLabel>
        <skos:prefLabel xml:lang="el">Έκταση φυσικού χαρακτηριστικού</skos:prefLabel>
    </owl:NamedIndividual>
    


    <!-- http://w3id.org/dcri-ont/vocabulary/concept_00201 -->


    <owl:NamedIndividual rdf:about="http://w3id.org/dcri-ont/vocabulary/concept_00201">
        <rdf:type rdf:resource="http://www.w3.org/2004/02/skos/core#Concept"/>
        <skos:broader rdf:resource="http://w3id.org/dcri-ont/vocabulary/concept_00155"/>
        <skos:inScheme rdf:resource="http://w3id.org/dcri-ont/vocabulary/conceptscheme"/>
        <rdfs:label xml:lang="en">Marker</rdfs:label>
        <rdfs:label xml:lang="el">Μαρκαδόρος</rdfs:label>
        <skos:prefLabel xml:lang="en">Marker</skos:prefLabel>
        <skos:prefLabel xml:lang="el">Μαρκαδόρος</skos:prefLabel>
    </owl:NamedIndividual>
    


    <!-- http://w3id.org/dcri-ont/vocabulary/concept_00202 -->


    <owl:NamedIndividual rdf:about="http://w3id.org/dcri-ont/vocabulary/concept_00202">
        <rdf:type rdf:resource="http://www.w3.org/2004/02/skos/core#Concept"/>
        <skos:broader rdf:resource="http://w3id.org/dcri-ont/vocabulary/concept_00227"/>
        <skos:inScheme rdf:resource="http://w3id.org/dcri-ont/vocabulary/conceptscheme"/>
        <rdfs:label xml:lang="en">Loss</rdfs:label>
        <rdfs:label xml:lang="el">Απώλεια</rdfs:label>
        <skos:prefLabel xml:lang="en">Loss</skos:prefLabel>
        <skos:prefLabel xml:lang="el">Απώλεια</skos:prefLabel>
    </owl:NamedIndividual>
    


    <!-- http://w3id.org/dcri-ont/vocabulary/concept_00203 -->


    <owl:NamedIndividual rdf:about="http://w3id.org/dcri-ont/vocabulary/concept_00203">
        <rdf:type rdf:resource="http://www.w3.org/2004/02/skos/core#Concept"/>
        <skos:broader rdf:resource="http://w3id.org/dcri-ont/vocabulary/concept_00227"/>
        <skos:inScheme rdf:resource="http://w3id.org/dcri-ont/vocabulary/conceptscheme"/>
        <rdfs:label xml:lang="en">Polymerism</rdfs:label>
        <rdfs:label xml:lang="el">Πολυμερισμός</rdfs:label>
        <skos:prefLabel xml:lang="en">Polymerism</skos:prefLabel>
        <skos:prefLabel xml:lang="el">Πολυμερισμός</skos:prefLabel>
    </owl:NamedIndividual>
    


    <!-- http://w3id.org/dcri-ont/vocabulary/concept_00204 -->


    <owl:NamedIndividual rdf:about="http://w3id.org/dcri-ont/vocabulary/concept_00204">
        <rdf:type rdf:resource="http://www.w3.org/2004/02/skos/core#Concept"/>
        <skos:broader rdf:resource="http://w3id.org/dcri-ont/vocabulary/concept_00228"/>
        <skos:inScheme rdf:resource="http://w3id.org/dcri-ont/vocabulary/conceptscheme"/>
        <rdfs:label xml:lang="en">Polymerism degree</rdfs:label>
        <rdfs:label xml:lang="el">Βαθμός πολυμερισμού</rdfs:label>
        <skos:prefLabel xml:lang="en">Polymerism degree</skos:prefLabel>
        <skos:prefLabel xml:lang="el">Βαθμός πολυμερισμού</skos:prefLabel>
    </owl:NamedIndividual>
    


    <!-- http://w3id.org/dcri-ont/vocabulary/concept_00205 -->


    <owl:NamedIndividual rdf:about="http://w3id.org/dcri-ont/vocabulary/concept_00205">
        <rdf:type rdf:resource="http://www.w3.org/2004/02/skos/core#Concept"/>
        <skos:broader rdf:resource="http://w3id.org/dcri-ont/vocabulary/concept_00069"/>
        <skos:inScheme rdf:resource="http://w3id.org/dcri-ont/vocabulary/conceptscheme"/>
        <rdfs:label xml:lang="en">Polyvinyl chloride</rdfs:label>
        <rdfs:label xml:lang="el">Πολυβινυλοχλωρίδιο</rdfs:label>
        <skos:prefLabel xml:lang="en">Polyvinyl chloride</skos:prefLabel>
        <skos:prefLabel xml:lang="el">Πολυβινυλοχλωρίδιο</skos:prefLabel>
    </owl:NamedIndividual>
    


    <!-- http://w3id.org/dcri-ont/vocabulary/concept_00206 -->


    <owl:NamedIndividual rdf:about="http://w3id.org/dcri-ont/vocabulary/concept_00206">
        <rdf:type rdf:resource="http://www.w3.org/2004/02/skos/core#Concept"/>
        <skos:broader rdf:resource="http://w3id.org/dcri-ont/vocabulary/concept_00069"/>
        <skos:inScheme rdf:resource="http://w3id.org/dcri-ont/vocabulary/conceptscheme"/>
        <rdfs:label xml:lang="en">Polyethelene</rdfs:label>
        <rdfs:label xml:lang="el">Πολυαιθυλένιο</rdfs:label>
        <skos:prefLabel xml:lang="en">Polyethelene</skos:prefLabel>
        <skos:prefLabel xml:lang="el">Πολυαιθυλένιο</skos:prefLabel>
    </owl:NamedIndividual>
    


    <!-- http://w3id.org/dcri-ont/vocabulary/concept_00207 -->


    <owl:NamedIndividual rdf:about="http://w3id.org/dcri-ont/vocabulary/concept_00207">
        <rdf:type rdf:resource="http://www.w3.org/2004/02/skos/core#Concept"/>
        <skos:broader rdf:resource="http://w3id.org/dcri-ont/vocabulary/concept_00069"/>
        <skos:inScheme rdf:resource="http://w3id.org/dcri-ont/vocabulary/conceptscheme"/>
        <rdfs:label xml:lang="en">Poly methyl methacrylate</rdfs:label>
        <rdfs:label xml:lang="el">Πολυμεθυλομεθακρυλικό</rdfs:label>
        <skos:prefLabel xml:lang="en">Poly methyl methacrylate</skos:prefLabel>
        <skos:prefLabel xml:lang="el">Πολυμεθυλομεθακρυλικό</skos:prefLabel>
    </owl:NamedIndividual>
    


    <!-- http://w3id.org/dcri-ont/vocabulary/concept_00208 -->


    <owl:NamedIndividual rdf:about="http://w3id.org/dcri-ont/vocabulary/concept_00208">
        <rdf:type rdf:resource="http://www.w3.org/2004/02/skos/core#Concept"/>
        <skos:inScheme rdf:resource="http://w3id.org/dcri-ont/vocabulary/conceptscheme"/>
        <skos:narrower rdf:resource="http://w3id.org/dcri-ont/vocabulary/concept_00210"/>
        <skos:narrower rdf:resource="http://w3id.org/dcri-ont/vocabulary/concept_00245"/>
        <skos:narrower rdf:resource="http://w3id.org/dcri-ont/vocabulary/concept_00246"/>
        <skos:topConceptOf rdf:resource="http://w3id.org/dcri-ont/vocabulary/conceptscheme"/>
        <rdfs:label xml:lang="en">Conservation object (vocabulary top concept)</rdfs:label>
        <rdfs:label xml:lang="el">Αντικείμενο συντήρησης</rdfs:label>
        <skos:prefLabel xml:lang="en">Conservation object (vocabulary top concept)</skos:prefLabel>
        <skos:prefLabel xml:lang="el">Αντικείμενο συντήρησης</skos:prefLabel>
    </owl:NamedIndividual>
    


    <!-- http://w3id.org/dcri-ont/vocabulary/concept_00210 -->


    <owl:NamedIndividual rdf:about="http://w3id.org/dcri-ont/vocabulary/concept_00210">
        <rdf:type rdf:resource="http://www.w3.org/2004/02/skos/core#Concept"/>
        <skos:broader rdf:resource="http://w3id.org/dcri-ont/vocabulary/concept_00208"/>
        <skos:inScheme rdf:resource="http://w3id.org/dcri-ont/vocabulary/conceptscheme"/>
        <skos:narrower rdf:resource="http://w3id.org/dcri-ont/vocabulary/concept_00212"/>
        <skos:narrower rdf:resource="http://w3id.org/dcri-ont/vocabulary/concept_00213"/>
        <skos:narrower rdf:resource="http://w3id.org/dcri-ont/vocabulary/concept_00214"/>
        <skos:narrower rdf:resource="http://w3id.org/dcri-ont/vocabulary/concept_00215"/>
        <skos:narrower rdf:resource="http://w3id.org/dcri-ont/vocabulary/concept_00218"/>
        <skos:narrower rdf:resource="http://w3id.org/dcri-ont/vocabulary/concept_00232"/>
        <rdfs:label xml:lang="en">Structural layer</rdfs:label>
        <rdfs:label xml:lang="el">Δομικό στρώμα</rdfs:label>
        <skos:prefLabel xml:lang="en">Structural layer</skos:prefLabel>
        <skos:prefLabel xml:lang="el">Δομικό στρώμα</skos:prefLabel>
    </owl:NamedIndividual>
    


    <!-- http://w3id.org/dcri-ont/vocabulary/concept_00211 -->


    <owl:NamedIndividual rdf:about="http://w3id.org/dcri-ont/vocabulary/concept_00211">
        <rdf:type rdf:resource="http://www.w3.org/2004/02/skos/core#Concept"/>
        <skos:broader rdf:resource="http://w3id.org/dcri-ont/vocabulary/concept_00210"/>
        <skos:inScheme rdf:resource="http://w3id.org/dcri-ont/vocabulary/conceptscheme"/>
        <rdfs:label xml:lang="en">Painting layer</rdfs:label>
        <rdfs:label xml:lang="el">Ζωγραφικό στρώμα</rdfs:label>
        <skos:prefLabel xml:lang="en">Painting layer</skos:prefLabel>
        <skos:prefLabel xml:lang="el">Ζωγραφικό στρώμα</skos:prefLabel>
    </owl:NamedIndividual>
    


    <!-- http://w3id.org/dcri-ont/vocabulary/concept_00212 -->


    <owl:NamedIndividual rdf:about="http://w3id.org/dcri-ont/vocabulary/concept_00212">
        <rdf:type rdf:resource="http://www.w3.org/2004/02/skos/core#Concept"/>
        <skos:broader rdf:resource="http://w3id.org/dcri-ont/vocabulary/concept_00210"/>
        <skos:inScheme rdf:resource="http://w3id.org/dcri-ont/vocabulary/conceptscheme"/>
        <rdfs:label xml:lang="en">Coating layer</rdfs:label>
        <rdfs:label xml:lang="el">Επικαλυπτικό στρώμα</rdfs:label>
        <skos:prefLabel xml:lang="en">Coating layer</skos:prefLabel>
        <skos:prefLabel xml:lang="el">Επικαλυπτικό στρώμα</skos:prefLabel>
    </owl:NamedIndividual>
    


    <!-- http://w3id.org/dcri-ont/vocabulary/concept_00213 -->


    <owl:NamedIndividual rdf:about="http://w3id.org/dcri-ont/vocabulary/concept_00213">
        <rdf:type rdf:resource="http://www.w3.org/2004/02/skos/core#Concept"/>
        <skos:broader rdf:resource="http://w3id.org/dcri-ont/vocabulary/concept_00210"/>
        <skos:inScheme rdf:resource="http://w3id.org/dcri-ont/vocabulary/conceptscheme"/>
        <rdfs:label xml:lang="en">Support layer</rdfs:label>
        <rdfs:label xml:lang="el">Στρώμα υποστήριξης</rdfs:label>
        <skos:prefLabel xml:lang="en">Support layer</skos:prefLabel>
        <skos:prefLabel xml:lang="el">Στρώμα υποστήριξης</skos:prefLabel>
    </owl:NamedIndividual>
    


    <!-- http://w3id.org/dcri-ont/vocabulary/concept_00214 -->


    <owl:NamedIndividual rdf:about="http://w3id.org/dcri-ont/vocabulary/concept_00214">
        <rdf:type rdf:resource="http://www.w3.org/2004/02/skos/core#Concept"/>
        <skos:broader rdf:resource="http://w3id.org/dcri-ont/vocabulary/concept_00210"/>
        <skos:inScheme rdf:resource="http://w3id.org/dcri-ont/vocabulary/conceptscheme"/>
        <rdfs:label xml:lang="en">Substrate layer</rdfs:label>
        <rdfs:label xml:lang="el">Υπόστρωμα</rdfs:label>
        <skos:prefLabel xml:lang="en">Substrate layer</skos:prefLabel>
        <skos:prefLabel xml:lang="el">Υπόστρωμα</skos:prefLabel>
    </owl:NamedIndividual>
    


    <!-- http://w3id.org/dcri-ont/vocabulary/concept_00215 -->


    <owl:NamedIndividual rdf:about="http://w3id.org/dcri-ont/vocabulary/concept_00215">
        <rdf:type rdf:resource="http://www.w3.org/2004/02/skos/core#Concept"/>
        <skos:broader rdf:resource="http://w3id.org/dcri-ont/vocabulary/concept_00210"/>
        <skos:inScheme rdf:resource="http://w3id.org/dcri-ont/vocabulary/conceptscheme"/>
        <rdfs:label xml:lang="en">Ground layer</rdfs:label>
        <rdfs:label xml:lang="el">Στρώμα προετοιμασίας</rdfs:label>
        <skos:prefLabel xml:lang="en">Ground layer</skos:prefLabel>
        <skos:prefLabel xml:lang="el">Στρώμα προετοιμασίας</skos:prefLabel>
    </owl:NamedIndividual>
    


    <!-- http://w3id.org/dcri-ont/vocabulary/concept_00216 -->


    <owl:NamedIndividual rdf:about="http://w3id.org/dcri-ont/vocabulary/concept_00216">
        <rdf:type rdf:resource="http://www.w3.org/2004/02/skos/core#Concept"/>
        <skos:broader rdf:resource="http://w3id.org/dcri-ont/vocabulary/concept_00218"/>
        <skos:inScheme rdf:resource="http://w3id.org/dcri-ont/vocabulary/conceptscheme"/>
        <rdfs:label xml:lang="en">Design layer</rdfs:label>
        <rdfs:label xml:lang="el">Στρώμα σχεδίου</rdfs:label>
        <skos:prefLabel xml:lang="en">Design layer</skos:prefLabel>
        <skos:prefLabel xml:lang="el">Στρώμα σχεδίου</skos:prefLabel>
    </owl:NamedIndividual>
    


    <!-- http://w3id.org/dcri-ont/vocabulary/concept_00217 -->


    <owl:NamedIndividual rdf:about="http://w3id.org/dcri-ont/vocabulary/concept_00217">
        <rdf:type rdf:resource="http://www.w3.org/2004/02/skos/core#Concept"/>
        <skos:broader rdf:resource="http://w3id.org/dcri-ont/vocabulary/concept_00218"/>
        <skos:inScheme rdf:resource="http://w3id.org/dcri-ont/vocabulary/conceptscheme"/>
        <rdfs:label xml:lang="en">Emulsion layer</rdfs:label>
        <rdfs:label xml:lang="el">Στρώμα εμουλσιόν</rdfs:label>
        <skos:prefLabel xml:lang="en">Emulsion layer</skos:prefLabel>
        <skos:prefLabel xml:lang="el">Στρώμα εμουλσιόν</skos:prefLabel>
    </owl:NamedIndividual>
    


    <!-- http://w3id.org/dcri-ont/vocabulary/concept_00218 -->


    <owl:NamedIndividual rdf:about="http://w3id.org/dcri-ont/vocabulary/concept_00218">
        <rdf:type rdf:resource="http://www.w3.org/2004/02/skos/core#Concept"/>
        <skos:broader rdf:resource="http://w3id.org/dcri-ont/vocabulary/concept_00210"/>
        <skos:inScheme rdf:resource="http://w3id.org/dcri-ont/vocabulary/conceptscheme"/>
        <skos:narrower rdf:resource="http://w3id.org/dcri-ont/vocabulary/concept_00211"/>
        <skos:narrower rdf:resource="http://w3id.org/dcri-ont/vocabulary/concept_00216"/>
        <skos:narrower rdf:resource="http://w3id.org/dcri-ont/vocabulary/concept_00217"/>
        <rdfs:label xml:lang="en">Media layer</rdfs:label>
        <rdfs:label xml:lang="el">Στρώμα μέσων</rdfs:label>
        <skos:prefLabel xml:lang="en">Media layer</skos:prefLabel>
        <skos:prefLabel xml:lang="el">Στρώμα μέσων</skos:prefLabel>
    </owl:NamedIndividual>
    


    <!-- http://w3id.org/dcri-ont/vocabulary/concept_00219 -->


    <owl:NamedIndividual rdf:about="http://w3id.org/dcri-ont/vocabulary/concept_00219">
        <rdf:type rdf:resource="http://www.w3.org/2004/02/skos/core#Concept"/>
        <skos:broader rdf:resource="http://w3id.org/dcri-ont/vocabulary/concept_00190"/>
        <skos:inScheme rdf:resource="http://w3id.org/dcri-ont/vocabulary/conceptscheme"/>
        <rdfs:label xml:lang="en">Wax coating</rdfs:label>
        <rdfs:label xml:lang="el">Επικαλυπτικό υλικό κεριού</rdfs:label>
        <skos:prefLabel xml:lang="en">Wax coating</skos:prefLabel>
        <skos:prefLabel xml:lang="el">Επικαλυπτικό υλικό κεριού</skos:prefLabel>
    </owl:NamedIndividual>
    


    <!-- http://w3id.org/dcri-ont/vocabulary/concept_00220 -->


    <owl:NamedIndividual rdf:about="http://w3id.org/dcri-ont/vocabulary/concept_00220">
        <rdf:type rdf:resource="http://www.w3.org/2004/02/skos/core#Concept"/>
        <skos:broader rdf:resource="http://w3id.org/dcri-ont/vocabulary/concept_00190"/>
        <skos:inScheme rdf:resource="http://w3id.org/dcri-ont/vocabulary/conceptscheme"/>
        <rdfs:label xml:lang="en">Resin coating</rdfs:label>
        <rdfs:label xml:lang="el">Επικαλυπτικό υλικό ρητίνης</rdfs:label>
        <skos:prefLabel xml:lang="en">Resin coating</skos:prefLabel>
        <skos:prefLabel xml:lang="el">Επικαλυπτικό υλικό ρητίνης</skos:prefLabel>
    </owl:NamedIndividual>
    


    <!-- http://w3id.org/dcri-ont/vocabulary/concept_00221 -->


    <owl:NamedIndividual rdf:about="http://w3id.org/dcri-ont/vocabulary/concept_00221">
        <rdf:type rdf:resource="http://www.w3.org/2004/02/skos/core#Concept"/>
        <skos:broader rdf:resource="http://w3id.org/dcri-ont/vocabulary/concept_00190"/>
        <skos:inScheme rdf:resource="http://w3id.org/dcri-ont/vocabulary/conceptscheme"/>
        <skos:narrower rdf:resource="http://w3id.org/dcri-ont/vocabulary/concept_00230"/>
        <skos:narrower rdf:resource="http://w3id.org/dcri-ont/vocabulary/concept_00231"/>
        <skos:narrower rdf:resource="http://w3id.org/dcri-ont/vocabulary/concept_00243"/>
        <rdfs:label xml:lang="en">Paint coating</rdfs:label>
        <rdfs:label xml:lang="el">Επικαλυπτικό υλικό χρώματος</rdfs:label>
        <skos:prefLabel xml:lang="en">Paint coating</skos:prefLabel>
        <skos:prefLabel xml:lang="el">Επικαλυπτικό υλικό χρώματος</skos:prefLabel>
    </owl:NamedIndividual>
    


    <!-- http://w3id.org/dcri-ont/vocabulary/concept_00222 -->


    <owl:NamedIndividual rdf:about="http://w3id.org/dcri-ont/vocabulary/concept_00222">
        <rdf:type rdf:resource="http://www.w3.org/2004/02/skos/core#Concept"/>
        <skos:inScheme rdf:resource="http://w3id.org/dcri-ont/vocabulary/conceptscheme"/>
        <skos:narrower rdf:resource="http://w3id.org/dcri-ont/vocabulary/concept_00065"/>
        <skos:narrower rdf:resource="http://w3id.org/dcri-ont/vocabulary/concept_00068"/>
        <skos:narrower rdf:resource="http://w3id.org/dcri-ont/vocabulary/concept_00069"/>
        <skos:narrower rdf:resource="http://w3id.org/dcri-ont/vocabulary/concept_00070"/>
        <skos:narrower rdf:resource="http://w3id.org/dcri-ont/vocabulary/concept_00154"/>
        <skos:narrower rdf:resource="http://w3id.org/dcri-ont/vocabulary/concept_00155"/>
        <skos:narrower rdf:resource="http://w3id.org/dcri-ont/vocabulary/concept_00156"/>
        <skos:narrower rdf:resource="http://w3id.org/dcri-ont/vocabulary/concept_00158"/>
        <skos:narrower rdf:resource="http://w3id.org/dcri-ont/vocabulary/concept_00159"/>
        <skos:narrower rdf:resource="http://w3id.org/dcri-ont/vocabulary/concept_00160"/>
        <skos:narrower rdf:resource="http://w3id.org/dcri-ont/vocabulary/concept_00167"/>
        <skos:narrower rdf:resource="http://w3id.org/dcri-ont/vocabulary/concept_00170"/>
        <skos:narrower rdf:resource="http://w3id.org/dcri-ont/vocabulary/concept_00179"/>
        <skos:narrower rdf:resource="http://w3id.org/dcri-ont/vocabulary/concept_00189"/>
        <skos:narrower rdf:resource="http://w3id.org/dcri-ont/vocabulary/concept_00190"/>
        <skos:narrower rdf:resource="http://w3id.org/dcri-ont/vocabulary/concept_00191"/>
        <skos:narrower rdf:resource="http://w3id.org/dcri-ont/vocabulary/concept_00192"/>
        <skos:narrower rdf:resource="http://w3id.org/dcri-ont/vocabulary/concept_00198"/>
        <skos:narrower rdf:resource="http://w3id.org/dcri-ont/vocabulary/concept_00199"/>
        <skos:narrower rdf:resource="http://w3id.org/dcri-ont/vocabulary/concept_00241"/>
        <skos:narrower rdf:resource="http://w3id.org/dcri-ont/vocabulary/concept_00242"/>
        <skos:narrower rdf:resource="http://w3id.org/dcri-ont/vocabulary/concept_00257"/>
        <skos:topConceptOf rdf:resource="http://w3id.org/dcri-ont/vocabulary/conceptscheme"/>
        <rdfs:label xml:lang="en">Material (vocabulary top concept)</rdfs:label>
        <rdfs:label xml:lang="el">Υλικό</rdfs:label>
        <skos:prefLabel xml:lang="en">Material (vocabulary top concept)</skos:prefLabel>
        <skos:prefLabel xml:lang="el">Υλικό</skos:prefLabel>
    </owl:NamedIndividual>
    


    <!-- http://w3id.org/dcri-ont/vocabulary/concept_00223 -->


    <owl:NamedIndividual rdf:about="http://w3id.org/dcri-ont/vocabulary/concept_00223">
        <rdf:type rdf:resource="http://www.w3.org/2004/02/skos/core#Concept"/>
        <skos:inScheme rdf:resource="http://w3id.org/dcri-ont/vocabulary/conceptscheme"/>
        <skos:narrower rdf:resource="http://w3id.org/dcri-ont/vocabulary/concept_00047"/>
        <skos:narrower rdf:resource="http://w3id.org/dcri-ont/vocabulary/concept_00048"/>
        <skos:narrower rdf:resource="http://w3id.org/dcri-ont/vocabulary/concept_00049"/>
        <skos:narrower rdf:resource="http://w3id.org/dcri-ont/vocabulary/concept_00050"/>
        <skos:narrower rdf:resource="http://w3id.org/dcri-ont/vocabulary/concept_00051"/>
        <skos:narrower rdf:resource="http://w3id.org/dcri-ont/vocabulary/concept_00052"/>
        <skos:narrower rdf:resource="http://w3id.org/dcri-ont/vocabulary/concept_00054"/>
        <skos:narrower rdf:resource="http://w3id.org/dcri-ont/vocabulary/concept_00058"/>
        <skos:narrower rdf:resource="http://w3id.org/dcri-ont/vocabulary/concept_00164"/>
        <skos:narrower rdf:resource="http://w3id.org/dcri-ont/vocabulary/concept_00165"/>
        <skos:narrower rdf:resource="http://w3id.org/dcri-ont/vocabulary/concept_00166"/>
        <skos:narrower rdf:resource="http://w3id.org/dcri-ont/vocabulary/concept_00194"/>
        <skos:narrower rdf:resource="http://w3id.org/dcri-ont/vocabulary/concept_00195"/>
        <skos:topConceptOf rdf:resource="http://w3id.org/dcri-ont/vocabulary/conceptscheme"/>
        <rdfs:label xml:lang="en">Equipment (vocabulary top concept)</rdfs:label>
        <rdfs:label xml:lang="el">Εξοπλισμός</rdfs:label>
        <skos:prefLabel xml:lang="en">Equipment (vocabulary top concept)</skos:prefLabel>
        <skos:prefLabel xml:lang="el">Εξοπλισμός</skos:prefLabel>
    </owl:NamedIndividual>
    


    <!-- http://w3id.org/dcri-ont/vocabulary/concept_00224 -->


    <owl:NamedIndividual rdf:about="http://w3id.org/dcri-ont/vocabulary/concept_00224">
        <rdf:type rdf:resource="http://www.w3.org/2004/02/skos/core#Concept"/>
        <skos:inScheme rdf:resource="http://w3id.org/dcri-ont/vocabulary/conceptscheme"/>
        <skos:topConceptOf rdf:resource="http://w3id.org/dcri-ont/vocabulary/conceptscheme"/>
        <rdfs:label xml:lang="en">Activity (vocabulary top concept)</rdfs:label>
        <rdfs:label xml:lang="el">Δραστηριότητα</rdfs:label>
        <skos:prefLabel xml:lang="en">Activity (vocabulary top concept)</skos:prefLabel>
        <skos:prefLabel xml:lang="el">Δραστηριότητα</skos:prefLabel>
    </owl:NamedIndividual>
    


    <!-- http://w3id.org/dcri-ont/vocabulary/concept_00225 -->


    <owl:NamedIndividual rdf:about="http://w3id.org/dcri-ont/vocabulary/concept_00225">
        <rdf:type rdf:resource="http://www.w3.org/2004/02/skos/core#Concept"/>
        <skos:inScheme rdf:resource="http://w3id.org/dcri-ont/vocabulary/conceptscheme"/>
        <skos:narrower rdf:resource="http://w3id.org/dcri-ont/vocabulary/concept_00018"/>
        <skos:narrower rdf:resource="http://w3id.org/dcri-ont/vocabulary/concept_00019"/>
        <skos:narrower rdf:resource="http://w3id.org/dcri-ont/vocabulary/concept_00020"/>
        <skos:topConceptOf rdf:resource="http://w3id.org/dcri-ont/vocabulary/conceptscheme"/>
        <rdfs:label xml:lang="en">Design or procedure (vocabulary top concept)</rdfs:label>
        <rdfs:label xml:lang="el">Σχέδιο ή διαδικασία</rdfs:label>
        <skos:prefLabel xml:lang="en">Design or procedure (vocabulary top concept)</skos:prefLabel>
        <skos:prefLabel xml:lang="el">Σχέδιο ή διαδικασία</skos:prefLabel>
    </owl:NamedIndividual>
    


    <!-- http://w3id.org/dcri-ont/vocabulary/concept_00226 -->


    <owl:NamedIndividual rdf:about="http://w3id.org/dcri-ont/vocabulary/concept_00226">
        <rdf:type rdf:resource="http://www.w3.org/2004/02/skos/core#Concept"/>
        <skos:inScheme rdf:resource="http://w3id.org/dcri-ont/vocabulary/conceptscheme"/>
        <skos:narrower rdf:resource="http://w3id.org/dcri-ont/vocabulary/concept_00149"/>
        <skos:narrower rdf:resource="http://w3id.org/dcri-ont/vocabulary/concept_00150"/>
        <skos:narrower rdf:resource="http://w3id.org/dcri-ont/vocabulary/concept_00157"/>
        <skos:narrower rdf:resource="http://w3id.org/dcri-ont/vocabulary/concept_00259"/>
        <skos:topConceptOf rdf:resource="http://w3id.org/dcri-ont/vocabulary/conceptscheme"/>
        <rdfs:label xml:lang="en">Measurement unit (vocabulary top concept)</rdfs:label>
        <rdfs:label xml:lang="el">Μονάδα μέτρησης</rdfs:label>
        <skos:prefLabel xml:lang="en">Measurement unit (vocabulary top concept)</skos:prefLabel>
        <skos:prefLabel xml:lang="el">Μονάδα μέτρησης</skos:prefLabel>
    </owl:NamedIndividual>
    


    <!-- http://w3id.org/dcri-ont/vocabulary/concept_00227 -->


    <owl:NamedIndividual rdf:about="http://w3id.org/dcri-ont/vocabulary/concept_00227">
        <rdf:type rdf:resource="http://www.w3.org/2004/02/skos/core#Concept"/>
        <skos:inScheme rdf:resource="http://w3id.org/dcri-ont/vocabulary/conceptscheme"/>
        <skos:narrower rdf:resource="http://w3id.org/dcri-ont/vocabulary/concept_00075"/>
        <skos:narrower rdf:resource="http://w3id.org/dcri-ont/vocabulary/concept_00083"/>
        <skos:narrower rdf:resource="http://w3id.org/dcri-ont/vocabulary/concept_00084"/>
        <skos:narrower rdf:resource="http://w3id.org/dcri-ont/vocabulary/concept_00085"/>
        <skos:narrower rdf:resource="http://w3id.org/dcri-ont/vocabulary/concept_00087"/>
        <skos:narrower rdf:resource="http://w3id.org/dcri-ont/vocabulary/concept_00088"/>
        <skos:narrower rdf:resource="http://w3id.org/dcri-ont/vocabulary/concept_00090"/>
        <skos:narrower rdf:resource="http://w3id.org/dcri-ont/vocabulary/concept_00091"/>
        <skos:narrower rdf:resource="http://w3id.org/dcri-ont/vocabulary/concept_00092"/>
        <skos:narrower rdf:resource="http://w3id.org/dcri-ont/vocabulary/concept_00171"/>
        <skos:narrower rdf:resource="http://w3id.org/dcri-ont/vocabulary/concept_00181"/>
        <skos:narrower rdf:resource="http://w3id.org/dcri-ont/vocabulary/concept_00182"/>
        <skos:narrower rdf:resource="http://w3id.org/dcri-ont/vocabulary/concept_00183"/>
        <skos:narrower rdf:resource="http://w3id.org/dcri-ont/vocabulary/concept_00184"/>
        <skos:narrower rdf:resource="http://w3id.org/dcri-ont/vocabulary/concept_00186"/>
        <skos:narrower rdf:resource="http://w3id.org/dcri-ont/vocabulary/concept_00193"/>
        <skos:narrower rdf:resource="http://w3id.org/dcri-ont/vocabulary/concept_00196"/>
        <skos:narrower rdf:resource="http://w3id.org/dcri-ont/vocabulary/concept_00202"/>
        <skos:narrower rdf:resource="http://w3id.org/dcri-ont/vocabulary/concept_00203"/>
        <skos:narrower rdf:resource="http://w3id.org/dcri-ont/vocabulary/concept_00233"/>
        <skos:narrower rdf:resource="http://w3id.org/dcri-ont/vocabulary/concept_00234"/>
        <skos:narrower rdf:resource="http://w3id.org/dcri-ont/vocabulary/concept_00235"/>
        <skos:narrower rdf:resource="http://w3id.org/dcri-ont/vocabulary/concept_00236"/>
        <skos:narrower rdf:resource="http://w3id.org/dcri-ont/vocabulary/concept_00237"/>
        <skos:narrower rdf:resource="http://w3id.org/dcri-ont/vocabulary/concept_00238"/>
        <skos:narrower rdf:resource="http://w3id.org/dcri-ont/vocabulary/concept_00239"/>
        <skos:narrower rdf:resource="http://w3id.org/dcri-ont/vocabulary/concept_00240"/>
        <skos:narrower rdf:resource="http://w3id.org/dcri-ont/vocabulary/concept_00244"/>
        <skos:narrower rdf:resource="http://w3id.org/dcri-ont/vocabulary/concept_00247"/>
        <skos:narrower rdf:resource="http://w3id.org/dcri-ont/vocabulary/concept_00248"/>
        <skos:narrower rdf:resource="http://w3id.org/dcri-ont/vocabulary/concept_00249"/>
        <skos:narrower rdf:resource="http://w3id.org/dcri-ont/vocabulary/concept_00250"/>
        <skos:topConceptOf rdf:resource="http://w3id.org/dcri-ont/vocabulary/conceptscheme"/>
        <rdfs:label xml:lang="en">Physical feature (vocabulary top concept)</rdfs:label>
        <rdfs:label xml:lang="el">Φυσικό χαρακτηριστικό</rdfs:label>
        <skos:prefLabel xml:lang="en">Physical feature (vocabulary top concept)</skos:prefLabel>
        <skos:prefLabel xml:lang="el">Φυσικό χαρακτηριστικό</skos:prefLabel>
    </owl:NamedIndividual>
    


    <!-- http://w3id.org/dcri-ont/vocabulary/concept_00228 -->


    <owl:NamedIndividual rdf:about="http://w3id.org/dcri-ont/vocabulary/concept_00228">
        <rdf:type rdf:resource="http://www.w3.org/2004/02/skos/core#Concept"/>
        <skos:inScheme rdf:resource="http://w3id.org/dcri-ont/vocabulary/conceptscheme"/>
        <skos:narrower rdf:resource="http://w3id.org/dcri-ont/vocabulary/concept_00002"/>
        <skos:narrower rdf:resource="http://w3id.org/dcri-ont/vocabulary/concept_00014"/>
        <skos:narrower rdf:resource="http://w3id.org/dcri-ont/vocabulary/concept_00028"/>
        <skos:narrower rdf:resource="http://w3id.org/dcri-ont/vocabulary/concept_00029"/>
        <skos:narrower rdf:resource="http://w3id.org/dcri-ont/vocabulary/concept_00030"/>
        <skos:narrower rdf:resource="http://w3id.org/dcri-ont/vocabulary/concept_00033"/>
        <skos:narrower rdf:resource="http://w3id.org/dcri-ont/vocabulary/concept_00039"/>
        <skos:narrower rdf:resource="http://w3id.org/dcri-ont/vocabulary/concept_00040"/>
        <skos:narrower rdf:resource="http://w3id.org/dcri-ont/vocabulary/concept_00041"/>
        <skos:narrower rdf:resource="http://w3id.org/dcri-ont/vocabulary/concept_00042"/>
        <skos:narrower rdf:resource="http://w3id.org/dcri-ont/vocabulary/concept_00046"/>
        <skos:narrower rdf:resource="http://w3id.org/dcri-ont/vocabulary/concept_00161"/>
        <skos:narrower rdf:resource="http://w3id.org/dcri-ont/vocabulary/concept_00162"/>
        <skos:narrower rdf:resource="http://w3id.org/dcri-ont/vocabulary/concept_00163"/>
        <skos:narrower rdf:resource="http://w3id.org/dcri-ont/vocabulary/concept_00173"/>
        <skos:narrower rdf:resource="http://w3id.org/dcri-ont/vocabulary/concept_00197"/>
        <skos:narrower rdf:resource="http://w3id.org/dcri-ont/vocabulary/concept_00200"/>
        <skos:narrower rdf:resource="http://w3id.org/dcri-ont/vocabulary/concept_00204"/>
        <skos:topConceptOf rdf:resource="http://w3id.org/dcri-ont/vocabulary/conceptscheme"/>
        <rdfs:label xml:lang="en">Property (vocabulary top concept)</rdfs:label>
        <rdfs:label xml:lang="el">Ιδιότητα</rdfs:label>
        <skos:prefLabel xml:lang="en">Property (vocabulary top concept)</skos:prefLabel>
        <skos:prefLabel xml:lang="el">Ιδιότητα</skos:prefLabel>
    </owl:NamedIndividual>
    


    <!-- http://w3id.org/dcri-ont/vocabulary/concept_00229 -->


    <owl:NamedIndividual rdf:about="http://w3id.org/dcri-ont/vocabulary/concept_00229">
        <rdf:type rdf:resource="http://www.w3.org/2004/02/skos/core#Concept"/>
        <skos:broader rdf:resource="http://w3id.org/dcri-ont/vocabulary/concept_00067"/>
        <skos:inScheme rdf:resource="http://w3id.org/dcri-ont/vocabulary/conceptscheme"/>
        <rdfs:label xml:lang="en">Watercolor paint</rdfs:label>
        <rdfs:label xml:lang="el">Υδατοχρώματα</rdfs:label>
        <skos:prefLabel xml:lang="en">Watercolor paint</skos:prefLabel>
        <skos:prefLabel xml:lang="el">Υδατοχρώματα</skos:prefLabel>
    </owl:NamedIndividual>
    


    <!-- http://w3id.org/dcri-ont/vocabulary/concept_00230 -->


    <owl:NamedIndividual rdf:about="http://w3id.org/dcri-ont/vocabulary/concept_00230">
        <rdf:type rdf:resource="http://www.w3.org/2004/02/skos/core#Concept"/>
        <skos:broader rdf:resource="http://w3id.org/dcri-ont/vocabulary/concept_00221"/>
        <skos:inScheme rdf:resource="http://w3id.org/dcri-ont/vocabulary/conceptscheme"/>
        <rdfs:label xml:lang="en">Acrylic coating</rdfs:label>
        <rdfs:label xml:lang="el">Ακρυλικό επικαλυπτικό υλικό</rdfs:label>
        <skos:prefLabel xml:lang="en">Acrylic coating</skos:prefLabel>
        <skos:prefLabel xml:lang="el">Ακρυλικό επικαλυπτικό υλικό</skos:prefLabel>
    </owl:NamedIndividual>
    


    <!-- http://w3id.org/dcri-ont/vocabulary/concept_00231 -->


    <owl:NamedIndividual rdf:about="http://w3id.org/dcri-ont/vocabulary/concept_00231">
        <rdf:type rdf:resource="http://www.w3.org/2004/02/skos/core#Concept"/>
        <skos:broader rdf:resource="http://w3id.org/dcri-ont/vocabulary/concept_00221"/>
        <skos:inScheme rdf:resource="http://w3id.org/dcri-ont/vocabulary/conceptscheme"/>
        <rdfs:label xml:lang="en">Oil paint coating</rdfs:label>
        <rdfs:label xml:lang="el">Επικαλυπτικό υλικό λαδιού</rdfs:label>
        <skos:prefLabel xml:lang="en">Oil paint coating</skos:prefLabel>
        <skos:prefLabel xml:lang="el">Επικαλυπτικό υλικό λαδιού</skos:prefLabel>
    </owl:NamedIndividual>
    


    <!-- http://w3id.org/dcri-ont/vocabulary/concept_00232 -->


    <owl:NamedIndividual rdf:about="http://w3id.org/dcri-ont/vocabulary/concept_00232">
        <rdf:type rdf:resource="http://www.w3.org/2004/02/skos/core#Concept"/>
        <skos:broader rdf:resource="http://w3id.org/dcri-ont/vocabulary/concept_00210"/>
        <skos:inScheme rdf:resource="http://w3id.org/dcri-ont/vocabulary/conceptscheme"/>
        <rdfs:label xml:lang="en">Marking layer</rdfs:label>
        <rdfs:label xml:lang="el">Στρώμα σήμανσης</rdfs:label>
        <skos:prefLabel xml:lang="en">Marking layer</skos:prefLabel>
        <skos:prefLabel xml:lang="el">Στρώμα σήμανσης</skos:prefLabel>
    </owl:NamedIndividual>
    


    <!-- http://w3id.org/dcri-ont/vocabulary/concept_00233 -->


    <owl:NamedIndividual rdf:about="http://w3id.org/dcri-ont/vocabulary/concept_00233">
        <rdf:type rdf:resource="http://www.w3.org/2004/02/skos/core#Concept"/>
        <skos:broader rdf:resource="http://w3id.org/dcri-ont/vocabulary/concept_00227"/>
        <skos:inScheme rdf:resource="http://w3id.org/dcri-ont/vocabulary/conceptscheme"/>
        <rdfs:label xml:lang="en">Keys missing</rdfs:label>
        <rdfs:label xml:lang="el">Απώλεια σφηνών</rdfs:label>
        <skos:prefLabel xml:lang="en">Keys missing</skos:prefLabel>
        <skos:prefLabel xml:lang="el">Απώλεια σφηνών</skos:prefLabel>
    </owl:NamedIndividual>
    


    <!-- http://w3id.org/dcri-ont/vocabulary/concept_00234 -->


    <owl:NamedIndividual rdf:about="http://w3id.org/dcri-ont/vocabulary/concept_00234">
        <rdf:type rdf:resource="http://www.w3.org/2004/02/skos/core#Concept"/>
        <skos:broader rdf:resource="http://w3id.org/dcri-ont/vocabulary/concept_00227"/>
        <skos:inScheme rdf:resource="http://w3id.org/dcri-ont/vocabulary/conceptscheme"/>
        <rdfs:label xml:lang="en">Batten traces</rdfs:label>
        <rdfs:label xml:lang="el">Ίχνη τρέσου</rdfs:label>
        <skos:prefLabel xml:lang="en">Batten traces</skos:prefLabel>
        <skos:prefLabel xml:lang="el">Ίχνη τρέσου</skos:prefLabel>
    </owl:NamedIndividual>
    


    <!-- http://w3id.org/dcri-ont/vocabulary/concept_00235 -->


    <owl:NamedIndividual rdf:about="http://w3id.org/dcri-ont/vocabulary/concept_00235">
        <rdf:type rdf:resource="http://www.w3.org/2004/02/skos/core#Concept"/>
        <skos:broader rdf:resource="http://w3id.org/dcri-ont/vocabulary/concept_00227"/>
        <skos:inScheme rdf:resource="http://w3id.org/dcri-ont/vocabulary/conceptscheme"/>
        <rdfs:label xml:lang="en">Stretcher traces</rdfs:label>
        <rdfs:label xml:lang="el">Ίχνη τελάρου</rdfs:label>
        <skos:prefLabel xml:lang="en">Stretcher traces</skos:prefLabel>
        <skos:prefLabel xml:lang="el">Ίχνη τελάρου</skos:prefLabel>
    </owl:NamedIndividual>
    


    <!-- http://w3id.org/dcri-ont/vocabulary/concept_00236 -->


    <owl:NamedIndividual rdf:about="http://w3id.org/dcri-ont/vocabulary/concept_00236">
        <rdf:type rdf:resource="http://www.w3.org/2004/02/skos/core#Concept"/>
        <skos:broader rdf:resource="http://w3id.org/dcri-ont/vocabulary/concept_00227"/>
        <skos:inScheme rdf:resource="http://w3id.org/dcri-ont/vocabulary/conceptscheme"/>
        <rdfs:label xml:lang="en">Mechanical damage</rdfs:label>
        <rdfs:label xml:lang="el">Απώλεια μηχανικών ιδιοτήτων</rdfs:label>
        <skos:prefLabel xml:lang="en">Mechanical damage</skos:prefLabel>
        <skos:prefLabel xml:lang="el">Απώλεια μηχανικών ιδιοτήτων</skos:prefLabel>
    </owl:NamedIndividual>
    


    <!-- http://w3id.org/dcri-ont/vocabulary/concept_00237 -->


    <owl:NamedIndividual rdf:about="http://w3id.org/dcri-ont/vocabulary/concept_00237">
        <rdf:type rdf:resource="http://www.w3.org/2004/02/skos/core#Concept"/>
        <skos:broader rdf:resource="http://w3id.org/dcri-ont/vocabulary/concept_00227"/>
        <skos:inScheme rdf:resource="http://w3id.org/dcri-ont/vocabulary/conceptscheme"/>
        <rdfs:label xml:lang="en">Craquelure</rdfs:label>
        <rdfs:label xml:lang="el">Κρακλέ</rdfs:label>
        <skos:prefLabel xml:lang="en">Craquelure</skos:prefLabel>
        <skos:prefLabel xml:lang="el">Κρακλέ</skos:prefLabel>
    </owl:NamedIndividual>
    


    <!-- http://w3id.org/dcri-ont/vocabulary/concept_00238 -->


    <owl:NamedIndividual rdf:about="http://w3id.org/dcri-ont/vocabulary/concept_00238">
        <rdf:type rdf:resource="http://www.w3.org/2004/02/skos/core#Concept"/>
        <skos:broader rdf:resource="http://w3id.org/dcri-ont/vocabulary/concept_00227"/>
        <skos:inScheme rdf:resource="http://w3id.org/dcri-ont/vocabulary/conceptscheme"/>
        <rdfs:label xml:lang="en">Hole</rdfs:label>
        <rdfs:label xml:lang="el">Οπή</rdfs:label>
        <skos:prefLabel xml:lang="en">Hole</skos:prefLabel>
        <skos:prefLabel xml:lang="el">Οπή</skos:prefLabel>
    </owl:NamedIndividual>
    


    <!-- http://w3id.org/dcri-ont/vocabulary/concept_00239 -->


    <owl:NamedIndividual rdf:about="http://w3id.org/dcri-ont/vocabulary/concept_00239">
        <rdf:type rdf:resource="http://www.w3.org/2004/02/skos/core#Concept"/>
        <skos:broader rdf:resource="http://w3id.org/dcri-ont/vocabulary/concept_00227"/>
        <skos:inScheme rdf:resource="http://w3id.org/dcri-ont/vocabulary/conceptscheme"/>
        <rdfs:label xml:lang="en">Stain</rdfs:label>
        <rdfs:label xml:lang="el">Λεκές</rdfs:label>
        <skos:prefLabel xml:lang="en">Stain</skos:prefLabel>
        <skos:prefLabel xml:lang="el">Λεκές</skos:prefLabel>
    </owl:NamedIndividual>
    


    <!-- http://w3id.org/dcri-ont/vocabulary/concept_00240 -->


    <owl:NamedIndividual rdf:about="http://w3id.org/dcri-ont/vocabulary/concept_00240">
        <rdf:type rdf:resource="http://www.w3.org/2004/02/skos/core#Concept"/>
        <skos:broader rdf:resource="http://w3id.org/dcri-ont/vocabulary/concept_00227"/>
        <skos:inScheme rdf:resource="http://w3id.org/dcri-ont/vocabulary/conceptscheme"/>
        <rdfs:label xml:lang="en">Discoloration</rdfs:label>
        <rdfs:label xml:lang="el">Δυσχρωματισμός</rdfs:label>
        <skos:prefLabel xml:lang="en">Discoloration</skos:prefLabel>
        <skos:prefLabel xml:lang="el">Δυσχρωματισμός</skos:prefLabel>
    </owl:NamedIndividual>
    


    <!-- http://w3id.org/dcri-ont/vocabulary/concept_00241 -->


    <owl:NamedIndividual rdf:about="http://w3id.org/dcri-ont/vocabulary/concept_00241">
        <rdf:type rdf:resource="http://www.w3.org/2004/02/skos/core#Concept"/>
        <skos:broader rdf:resource="http://w3id.org/dcri-ont/vocabulary/concept_00222"/>
        <skos:inScheme rdf:resource="http://w3id.org/dcri-ont/vocabulary/conceptscheme"/>
        <rdfs:label xml:lang="en">Ground</rdfs:label>
        <rdfs:label xml:lang="el">Προετοιμασία</rdfs:label>
        <skos:prefLabel xml:lang="en">Ground</skos:prefLabel>
        <skos:prefLabel xml:lang="el">Προετοιμασία</skos:prefLabel>
    </owl:NamedIndividual>
    


    <!-- http://w3id.org/dcri-ont/vocabulary/concept_00242 -->


    <owl:NamedIndividual rdf:about="http://w3id.org/dcri-ont/vocabulary/concept_00242">
        <rdf:type rdf:resource="http://www.w3.org/2004/02/skos/core#Concept"/>
        <skos:broader rdf:resource="http://w3id.org/dcri-ont/vocabulary/concept_00222"/>
        <skos:inScheme rdf:resource="http://w3id.org/dcri-ont/vocabulary/conceptscheme"/>
        <rdfs:label xml:lang="en">Gypsum</rdfs:label>
        <rdfs:label xml:lang="el">Γύψος</rdfs:label>
        <skos:prefLabel xml:lang="en">Gypsum</skos:prefLabel>
        <skos:prefLabel xml:lang="el">Γύψος</skos:prefLabel>
    </owl:NamedIndividual>
    


    <!-- http://w3id.org/dcri-ont/vocabulary/concept_00243 -->


    <owl:NamedIndividual rdf:about="http://w3id.org/dcri-ont/vocabulary/concept_00243">
        <rdf:type rdf:resource="http://www.w3.org/2004/02/skos/core#Concept"/>
        <skos:broader rdf:resource="http://w3id.org/dcri-ont/vocabulary/concept_00221"/>
        <skos:inScheme rdf:resource="http://w3id.org/dcri-ont/vocabulary/conceptscheme"/>
        <rdfs:label xml:lang="en">Gold paint coating</rdfs:label>
        <rdfs:label xml:lang="el">Επικαλυπτικό υλικό χρυσού</rdfs:label>
        <skos:prefLabel xml:lang="en">Gold paint coating</skos:prefLabel>
        <skos:prefLabel xml:lang="el">Επικαλυπτικό υλικό χρυσού</skos:prefLabel>
    </owl:NamedIndividual>
    


    <!-- http://w3id.org/dcri-ont/vocabulary/concept_00244 -->


    <owl:NamedIndividual rdf:about="http://w3id.org/dcri-ont/vocabulary/concept_00244">
        <rdf:type rdf:resource="http://www.w3.org/2004/02/skos/core#Concept"/>
        <skos:broader rdf:resource="http://w3id.org/dcri-ont/vocabulary/concept_00227"/>
        <skos:inScheme rdf:resource="http://w3id.org/dcri-ont/vocabulary/conceptscheme"/>
        <rdfs:label xml:lang="en">Relief</rdfs:label>
        <rdfs:label xml:lang="el">Ανάγλυφο</rdfs:label>
        <skos:prefLabel xml:lang="en">Relief</skos:prefLabel>
        <skos:prefLabel xml:lang="el">Ανάγλυφο</skos:prefLabel>
    </owl:NamedIndividual>
    


    <!-- http://w3id.org/dcri-ont/vocabulary/concept_00245 -->


    <owl:NamedIndividual rdf:about="http://w3id.org/dcri-ont/vocabulary/concept_00245">
        <rdf:type rdf:resource="http://www.w3.org/2004/02/skos/core#Concept"/>
        <skos:broader rdf:resource="http://w3id.org/dcri-ont/vocabulary/concept_00208"/>
        <skos:inScheme rdf:resource="http://w3id.org/dcri-ont/vocabulary/conceptscheme"/>
        <rdfs:label xml:lang="en">Complex conservation object</rdfs:label>
        <rdfs:label xml:lang="el">Σύνθετο αντικείμενο συντήρησης</rdfs:label>
        <skos:prefLabel xml:lang="en">Complex conservation object</skos:prefLabel>
        <skos:prefLabel xml:lang="el">Σύνθετο αντικείμενο συντήρησης</skos:prefLabel>
    </owl:NamedIndividual>
    


    <!-- http://w3id.org/dcri-ont/vocabulary/concept_00246 -->


    <owl:NamedIndividual rdf:about="http://w3id.org/dcri-ont/vocabulary/concept_00246">
        <rdf:type rdf:resource="http://www.w3.org/2004/02/skos/core#Concept"/>
        <skos:broader rdf:resource="http://w3id.org/dcri-ont/vocabulary/concept_00208"/>
        <skos:inScheme rdf:resource="http://w3id.org/dcri-ont/vocabulary/conceptscheme"/>
        <rdfs:label xml:lang="en">Solid conservation object</rdfs:label>
        <rdfs:label xml:lang="el">Απλό αντικείμενο συντήρησης</rdfs:label>
        <skos:prefLabel xml:lang="en">Solid conservation object</skos:prefLabel>
        <skos:prefLabel xml:lang="el">Απλό αντικείμενο συντήρησης</skos:prefLabel>
    </owl:NamedIndividual>
    


    <!-- http://w3id.org/dcri-ont/vocabulary/concept_00247 -->


    <owl:NamedIndividual rdf:about="http://w3id.org/dcri-ont/vocabulary/concept_00247">
        <rdf:type rdf:resource="http://www.w3.org/2004/02/skos/core#Concept"/>
        <skos:broader rdf:resource="http://w3id.org/dcri-ont/vocabulary/concept_00227"/>
        <skos:inScheme rdf:resource="http://w3id.org/dcri-ont/vocabulary/conceptscheme"/>
        <rdfs:label xml:lang="en">Waves</rdfs:label>
        <rdfs:label xml:lang="el">Κυματισμός</rdfs:label>
        <skos:prefLabel xml:lang="en">Waves</skos:prefLabel>
        <skos:prefLabel xml:lang="el">Κυματισμός</skos:prefLabel>
    </owl:NamedIndividual>
    


    <!-- http://w3id.org/dcri-ont/vocabulary/concept_00248 -->


    <owl:NamedIndividual rdf:about="http://w3id.org/dcri-ont/vocabulary/concept_00248">
        <rdf:type rdf:resource="http://www.w3.org/2004/02/skos/core#Concept"/>
        <skos:broader rdf:resource="http://w3id.org/dcri-ont/vocabulary/concept_00227"/>
        <skos:inScheme rdf:resource="http://w3id.org/dcri-ont/vocabulary/conceptscheme"/>
        <rdfs:label xml:lang="en">Glue remains</rdfs:label>
        <rdfs:label xml:lang="el">Υπολείμματα κόλλας</rdfs:label>
        <skos:prefLabel xml:lang="en">Glue remains</skos:prefLabel>
        <skos:prefLabel xml:lang="el">Υπολείμματα κόλλας</skos:prefLabel>
    </owl:NamedIndividual>
    


    <!-- http://w3id.org/dcri-ont/vocabulary/concept_00249 -->


    <owl:NamedIndividual rdf:about="http://w3id.org/dcri-ont/vocabulary/concept_00249">
        <rdf:type rdf:resource="http://www.w3.org/2004/02/skos/core#Concept"/>
        <skos:broader rdf:resource="http://w3id.org/dcri-ont/vocabulary/concept_00227"/>
        <skos:inScheme rdf:resource="http://w3id.org/dcri-ont/vocabulary/conceptscheme"/>
        <rdfs:label xml:lang="en">Biological attack</rdfs:label>
        <rdfs:label xml:lang="el">Βιολογική προσβολή</rdfs:label>
        <skos:prefLabel xml:lang="en">Biological attack</skos:prefLabel>
        <skos:prefLabel xml:lang="el">Βιολογική προσβολή</skos:prefLabel>
    </owl:NamedIndividual>
    


    <!-- http://w3id.org/dcri-ont/vocabulary/concept_00250 -->


    <owl:NamedIndividual rdf:about="http://w3id.org/dcri-ont/vocabulary/concept_00250">
        <rdf:type rdf:resource="http://www.w3.org/2004/02/skos/core#Concept"/>
        <skos:broader rdf:resource="http://w3id.org/dcri-ont/vocabulary/concept_00227"/>
        <skos:inScheme rdf:resource="http://w3id.org/dcri-ont/vocabulary/conceptscheme"/>
        <rdfs:label xml:lang="en">Abrasion damage</rdfs:label>
        <rdfs:label xml:lang="el">Φθορές τριβής</rdfs:label>
        <skos:prefLabel xml:lang="en">Abrasion damage</skos:prefLabel>
        <skos:prefLabel xml:lang="el">Φθορές τριβής</skos:prefLabel>
    </owl:NamedIndividual>
    


    <!-- http://w3id.org/dcri-ont/vocabulary/concept_00251 -->


    <owl:NamedIndividual rdf:about="http://w3id.org/dcri-ont/vocabulary/concept_00251">
        <rdf:type rdf:resource="http://www.w3.org/2004/02/skos/core#Concept"/>
        <skos:inScheme rdf:resource="http://w3id.org/dcri-ont/vocabulary/conceptscheme"/>
        <skos:narrower rdf:resource="http://w3id.org/dcri-ont/vocabulary/concept_00252"/>
        <skos:narrower rdf:resource="http://w3id.org/dcri-ont/vocabulary/concept_00253"/>
        <skos:topConceptOf rdf:resource="http://w3id.org/dcri-ont/vocabulary/conceptscheme"/>
        <rdfs:label xml:lang="en">Conservation object&apos;s location (vocabulary top concept)</rdfs:label>
        <rdfs:label xml:lang="el">Θέση αντικειμένου συντήρησης</rdfs:label>
        <skos:prefLabel xml:lang="en">Conservation object&apos;s location (vocabulary top concept)</skos:prefLabel>
        <skos:prefLabel xml:lang="el">Θέση αντικειμένου συντήρησης</skos:prefLabel>
    </owl:NamedIndividual>
    


    <!-- http://w3id.org/dcri-ont/vocabulary/concept_00252 -->


    <owl:NamedIndividual rdf:about="http://w3id.org/dcri-ont/vocabulary/concept_00252">
        <rdf:type rdf:resource="http://www.w3.org/2004/02/skos/core#Concept"/>
        <skos:broader rdf:resource="http://w3id.org/dcri-ont/vocabulary/concept_00251"/>
        <skos:inScheme rdf:resource="http://w3id.org/dcri-ont/vocabulary/conceptscheme"/>
        <rdfs:label xml:lang="en">Storage location</rdfs:label>
        <rdfs:label xml:lang="el">Θέση αποθήκευσης</rdfs:label>
        <skos:prefLabel xml:lang="en">Storage location</skos:prefLabel>
        <skos:prefLabel xml:lang="el">Θέση αποθήκευσης</skos:prefLabel>
    </owl:NamedIndividual>
    


    <!-- http://w3id.org/dcri-ont/vocabulary/concept_00253 -->


    <owl:NamedIndividual rdf:about="http://w3id.org/dcri-ont/vocabulary/concept_00253">
        <rdf:type rdf:resource="http://www.w3.org/2004/02/skos/core#Concept"/>
        <skos:broader rdf:resource="http://w3id.org/dcri-ont/vocabulary/concept_00251"/>
        <skos:inScheme rdf:resource="http://w3id.org/dcri-ont/vocabulary/conceptscheme"/>
        <rdfs:label xml:lang="en">Exhibition location</rdfs:label>
        <rdfs:label xml:lang="el">Θέση έκθεσης</rdfs:label>
        <skos:prefLabel xml:lang="en">Exhibition location</skos:prefLabel>
        <skos:prefLabel xml:lang="el">Θέση έκθεσης</skos:prefLabel>
    </owl:NamedIndividual>
    


    <!-- http://w3id.org/dcri-ont/vocabulary/concept_00254 -->


    <owl:NamedIndividual rdf:about="http://w3id.org/dcri-ont/vocabulary/concept_00254">
        <rdf:type rdf:resource="http://www.w3.org/2004/02/skos/core#Concept"/>
        <skos:broader rdf:resource="http://w3id.org/dcri-ont/vocabulary/concept_00160"/>
        <skos:inScheme rdf:resource="http://w3id.org/dcri-ont/vocabulary/conceptscheme"/>
        <rdfs:label xml:lang="en">Klucel G</rdfs:label>
        <skos:prefLabel xml:lang="en">Klucel G</skos:prefLabel>
    </owl:NamedIndividual>
    


    <!-- http://w3id.org/dcri-ont/vocabulary/concept_00255 -->


    <owl:NamedIndividual rdf:about="http://w3id.org/dcri-ont/vocabulary/concept_00255">
        <rdf:type rdf:resource="http://www.w3.org/2004/02/skos/core#Concept"/>
        <skos:broader rdf:resource="http://w3id.org/dcri-ont/vocabulary/concept_00158"/>
        <skos:inScheme rdf:resource="http://w3id.org/dcri-ont/vocabulary/conceptscheme"/>
        <rdfs:label xml:lang="en">Propan-2-ol</rdfs:label>
        <rdfs:label xml:lang="el">Ισοπροπανόλη</rdfs:label>
        <skos:prefLabel xml:lang="en">Propan-2-ol</skos:prefLabel>
        <skos:prefLabel xml:lang="el">Ισοπροπανόλη</skos:prefLabel>
    </owl:NamedIndividual>
    


    <!-- http://w3id.org/dcri-ont/vocabulary/concept_00256 -->


    <owl:NamedIndividual rdf:about="http://w3id.org/dcri-ont/vocabulary/concept_00256">
        <rdf:type rdf:resource="http://www.w3.org/2004/02/skos/core#Concept"/>
        <skos:broader rdf:resource="http://w3id.org/dcri-ont/vocabulary/concept_00228"/>
        <skos:inScheme rdf:resource="http://w3id.org/dcri-ont/vocabulary/conceptscheme"/>
        <rdfs:label xml:lang="en">Temperature</rdfs:label>
        <rdfs:label xml:lang="el">Θερμοκρασία</rdfs:label>
        <skos:prefLabel xml:lang="en">Temperature</skos:prefLabel>
        <skos:prefLabel xml:lang="el">Θερμοκρασία</skos:prefLabel>
    </owl:NamedIndividual>
    


    <!-- http://w3id.org/dcri-ont/vocabulary/concept_00257 -->


    <owl:NamedIndividual rdf:about="http://w3id.org/dcri-ont/vocabulary/concept_00257">
        <rdf:type rdf:resource="http://www.w3.org/2004/02/skos/core#Concept"/>
        <skos:broader rdf:resource="http://w3id.org/dcri-ont/vocabulary/concept_00222"/>
        <skos:inScheme rdf:resource="http://w3id.org/dcri-ont/vocabulary/conceptscheme"/>
        <rdfs:label xml:lang="en">Wet cleaning solution</rdfs:label>
        <rdfs:label xml:lang="el">Διάλυμα υγρού καθαρισμού</rdfs:label>
        <skos:prefLabel xml:lang="en">Wet cleaning solution</skos:prefLabel>
        <skos:prefLabel xml:lang="el">Διάλυμα υγρού καθαρισμού</skos:prefLabel>
    </owl:NamedIndividual>
    


    <!-- http://w3id.org/dcri-ont/vocabulary/concept_00258 -->


    <owl:NamedIndividual rdf:about="http://w3id.org/dcri-ont/vocabulary/concept_00258">
        <rdf:type rdf:resource="http://www.w3.org/2004/02/skos/core#Concept"/>
        <skos:broader rdf:resource="http://w3id.org/dcri-ont/vocabulary/concept_00228"/>
        <skos:inScheme rdf:resource="http://w3id.org/dcri-ont/vocabulary/conceptscheme"/>
        <rdfs:label xml:lang="en">Relative humidity</rdfs:label>
        <rdfs:label xml:lang="el">Σχετική υγρασία</rdfs:label>
        <skos:prefLabel xml:lang="en">Relative humidity</skos:prefLabel>
        <skos:prefLabel xml:lang="el">Σχετική υγρασία</skos:prefLabel>
    </owl:NamedIndividual>
    


    <!-- http://w3id.org/dcri-ont/vocabulary/concept_00259 -->


    <owl:NamedIndividual rdf:about="http://w3id.org/dcri-ont/vocabulary/concept_00259">
        <rdf:type rdf:resource="http://www.w3.org/2004/02/skos/core#Concept"/>
        <skos:broader rdf:resource="http://w3id.org/dcri-ont/vocabulary/concept_00226"/>
        <skos:inScheme rdf:resource="http://w3id.org/dcri-ont/vocabulary/conceptscheme"/>
        <rdfs:label xml:lang="en">Percentage</rdfs:label>
        <rdfs:label xml:lang="el">Ποσοστό</rdfs:label>
        <skos:prefLabel xml:lang="en">Percentage</skos:prefLabel>
        <skos:prefLabel xml:lang="el">Ποσοστό</skos:prefLabel>
    </owl:NamedIndividual>
    


    <!-- http://w3id.org/dcri-ont/vocabulary/concept_00260 -->


    <owl:NamedIndividual rdf:about="http://w3id.org/dcri-ont/vocabulary/concept_00260">
        <rdf:type rdf:resource="http://www.w3.org/2004/02/skos/core#Concept"/>
        <skos:broader rdf:resource="http://w3id.org/dcri-ont/vocabulary/concept_00263"/>
        <skos:inScheme rdf:resource="http://w3id.org/dcri-ont/vocabulary/conceptscheme"/>
        <rdfs:label xml:lang="en">Artist</rdfs:label>
        <rdfs:label xml:lang="el">Καλλιτέχνης</rdfs:label>
        <skos:prefLabel xml:lang="en">Artist</skos:prefLabel>
        <skos:prefLabel xml:lang="el">Καλλιτέχνης</skos:prefLabel>
    </owl:NamedIndividual>
    


    <!-- http://w3id.org/dcri-ont/vocabulary/concept_00261 -->


    <owl:NamedIndividual rdf:about="http://w3id.org/dcri-ont/vocabulary/concept_00261">
        <rdf:type rdf:resource="http://www.w3.org/2004/02/skos/core#Concept"/>
        <skos:broader rdf:resource="http://w3id.org/dcri-ont/vocabulary/concept_00263"/>
        <skos:inScheme rdf:resource="http://w3id.org/dcri-ont/vocabulary/conceptscheme"/>
        <rdfs:label xml:lang="en">Conservator</rdfs:label>
        <rdfs:label xml:lang="el">Συντηρητής</rdfs:label>
        <skos:prefLabel xml:lang="en">Conservator</skos:prefLabel>
        <skos:prefLabel xml:lang="el">Συντηρητής</skos:prefLabel>
    </owl:NamedIndividual>
    


    <!-- http://w3id.org/dcri-ont/vocabulary/concept_00262 -->


    <owl:NamedIndividual rdf:about="http://w3id.org/dcri-ont/vocabulary/concept_00262">
        <rdf:type rdf:resource="http://www.w3.org/2004/02/skos/core#Concept"/>
        <skos:broader rdf:resource="http://w3id.org/dcri-ont/vocabulary/concept_00263"/>
        <skos:inScheme rdf:resource="http://w3id.org/dcri-ont/vocabulary/conceptscheme"/>
        <rdfs:label xml:lang="en">Museum</rdfs:label>
        <rdfs:label xml:lang="el">Μουσείο</rdfs:label>
        <skos:prefLabel xml:lang="en">Museum</skos:prefLabel>
        <skos:prefLabel xml:lang="el">Μουσείο</skos:prefLabel>
    </owl:NamedIndividual>
    


    <!-- http://w3id.org/dcri-ont/vocabulary/concept_00263 -->


    <owl:NamedIndividual rdf:about="http://w3id.org/dcri-ont/vocabulary/concept_00263">
        <rdf:type rdf:resource="http://www.w3.org/2004/02/skos/core#Concept"/>
        <skos:inScheme rdf:resource="http://w3id.org/dcri-ont/vocabulary/conceptscheme"/>
        <skos:narrower rdf:resource="http://w3id.org/dcri-ont/vocabulary/concept_00260"/>
        <skos:narrower rdf:resource="http://w3id.org/dcri-ont/vocabulary/concept_00261"/>
        <skos:narrower rdf:resource="http://w3id.org/dcri-ont/vocabulary/concept_00262"/>
        <skos:topConceptOf rdf:resource="http://w3id.org/dcri-ont/vocabulary/conceptscheme"/>
        <rdfs:label xml:lang="en">Actor type (vocabulary top concept)</rdfs:label>
        <rdfs:label xml:lang="el">Τύπος δράστη</rdfs:label>
        <skos:prefLabel xml:lang="en">Actor type (vocabulary top concept)</skos:prefLabel>
        <skos:prefLabel xml:lang="el">Τύπος δράστη</skos:prefLabel>
    </owl:NamedIndividual>
    


    <!-- http://w3id.org/dcri-ont/vocabulary/conceptscheme -->


    <owl:NamedIndividual rdf:about="http://w3id.org/dcri-ont/vocabulary/conceptscheme">
        <rdf:type rdf:resource="http://www.w3.org/2004/02/skos/core#ConceptScheme"/>
        <skos:hasTopConcept rdf:resource="http://w3id.org/dcri-ont/vocabulary/concept_00208"/>
        <skos:hasTopConcept rdf:resource="http://w3id.org/dcri-ont/vocabulary/concept_00222"/>
        <skos:hasTopConcept rdf:resource="http://w3id.org/dcri-ont/vocabulary/concept_00223"/>
        <skos:hasTopConcept rdf:resource="http://w3id.org/dcri-ont/vocabulary/concept_00224"/>
        <skos:hasTopConcept rdf:resource="http://w3id.org/dcri-ont/vocabulary/concept_00226"/>
        <skos:hasTopConcept rdf:resource="http://w3id.org/dcri-ont/vocabulary/concept_00227"/>
        <skos:hasTopConcept rdf:resource="http://w3id.org/dcri-ont/vocabulary/concept_00228"/>
        <skos:hasTopConcept rdf:resource="http://w3id.org/dcri-ont/vocabulary/concept_00251"/>
        <skos:hasTopConcept rdf:resource="http://w3id.org/dcri-ont/vocabulary/concept_00263"/>
        <terms:title xml:lang="en">DCRIO Vocabulary</terms:title>
        <terms:title xml:lang="el">DCRIO Λεξιλόγιο</terms:title>
        <rdfs:label xml:lang="en">DCRIO Vocabulary</rdfs:label>
        <rdfs:label xml:lang="el">DCRIO Λεξιλόγιο</rdfs:label>
        <skos:prefLabel xml:lang="en">DCRIO Vocabulary</skos:prefLabel>
        <skos:prefLabel xml:lang="el">DCRIO Λεξιλόγιο</skos:prefLabel>
    </owl:NamedIndividual>
</rdf:RDF>



<!-- Generated by the OWL API (version 5.1.18) https://github.com/owlcs/owlapi/ -->


